<?xml version="1.0"?>
<rdf:RDF xmlns="http://www.w3id.org/efro/efro/"
     xml:base="http://www.w3id.org/efro/efro/"
     xmlns:cc="http://web.resource.org/cc/"
     xmlns:dc="http://purl.org/dc/elements/1.1/"
     xmlns:ns="http://creativecommons.org/ns#"
     xmlns:ns2="http://www.w3.org/2003/06/sw-vocab-status/ns#"
     xmlns:owl="http://www.w3.org/2002/07/owl#"
     xmlns:rdf="http://www.w3.org/1999/02/22-rdf-syntax-ns#"
     xmlns:wot="http://xmlns.com/wot/0.1/"
     xmlns:xml="http://www.w3.org/XML/1998/namespace"
     xmlns:xsd="http://www.w3.org/2001/XMLSchema#"
     xmlns:EFRO="http://www.w3id.org/efro/efro#"
     xmlns:foaf="http://xmlns.com/foaf/0.1/"
     xmlns:owl1="http://purl.org/cerif/frapo/owl:"
     xmlns:rdfs="http://www.w3.org/2000/01/rdf-schema#"
     xmlns:skos="http://www.w3.org/2004/02/skos/core#"
     xmlns:vann="http://purl.org/vocab/vann/"
     xmlns:cerro="http://purl.org/cerif/cerro/"
     xmlns:frapo="http://purl.org/cerif/frapo/"
     xmlns:schema="http://purl.org/vocab/aiiso/schema#"
     xmlns:dcterms="http://purl.org/dc/terms/"
     xmlns:sw-vocab-status="http://www.w3.org/2003/06/sw-vocab-status/">
    <owl:Ontology rdf:about="http://www.w3id.org/efro/efro">
        <owl:imports rdf:resource="http://purl.org/cerif/frapo/"/>
        <owl:imports rdf:resource="http://purl.org/vocab/aiiso/schema#"/>
        <owl:imports rdf:resource="http://purl.org/vocab/vann/"/>
        <owl:imports rdf:resource="http://www.w3.org/2003/06/sw-vocab-status/ns"/>
        <owl:imports rdf:resource="http://xmlns.com/foaf/0.1/"/>
        <ns:license rdf:resource="https://creativecommons.org/licenses/by/4.0/"/>
        <dc:contributor>Ikechukwu Nkisi-Orji</dc:contributor>
        <dc:coverage>Educational domain including student management, program administration, funding allocation, and assessment tracking.</dc:coverage>
        <dc:rights>This ontology is licensed under the Creative Commons Attribution 4.0 International License (CC-BY 4.0). You are free to share and adapt this ontology, provided that you give appropriate credit. More details: https://creativecommons.org/licenses/by/4.0/</dc:rights>
        <dcterms:contributor>David Corsar</dcterms:contributor>
        <dcterms:creator>Umair Arshad</dcterms:creator>
        <dcterms:description>An ontology for modeling educational institutions&apos; funding, assessment, and student management systems. It captures the relationships between students, educational programs, funding mechanisms, and assessment processes. The ontology supports tracking student statuses, attendance, progression, and funding eligibility while maintaining compliance with educational standards and reporting requirements.</dcterms:description>
        <dcterms:format>rdf/xml</dcterms:format>
        <dcterms:language>en</dcterms:language>
        <dcterms:title>Educational Funding Regulations Ontology (EFRO)</dcterms:title>
        <rdfs:comment>This ontology models:
    1. Student enrollment and status tracking
    2. Educational program structures and requirements
    3. Funding mechanisms and eligibility criteria
    4. Assessment and progression tracking
    5. Attendance monitoring systems
    6. Documentation and compliance requirements
    7. Administrative processes and support systems</rdfs:comment>
        <owl:versionInfo rdf:datatype="http://www.w3.org/2001/XMLSchema#decimal">1.0</owl:versionInfo>
    </owl:Ontology>
    


    <!-- 
    ///////////////////////////////////////////////////////////////////////////////////////
    //
    // Annotation properties
    //
    ///////////////////////////////////////////////////////////////////////////////////////
     -->

    


    <!-- http://creativecommons.org/ns#license -->

    <owl:AnnotationProperty rdf:about="http://creativecommons.org/ns#license"/>
    


    <!-- http://purl.org/dc/elements/1.1/coverage -->

    <owl:AnnotationProperty rdf:about="http://purl.org/dc/elements/1.1/coverage"/>
    


    <!-- http://purl.org/dc/terms/description -->

    <owl:AnnotationProperty rdf:about="http://purl.org/dc/terms/description"/>
    


    <!-- http://www.w3.org/2004/02/skos/core#example -->

    <owl:AnnotationProperty rdf:about="http://www.w3.org/2004/02/skos/core#example"/>
    


    <!-- 
    ///////////////////////////////////////////////////////////////////////////////////////
    //
    // Object Properties
    //
    ///////////////////////////////////////////////////////////////////////////////////////
     -->

    


    <!-- http://www.w3id.org/efro/efro#belongsTo -->

    <owl:ObjectProperty rdf:about="http://www.w3id.org/efro/efro#belongsTo">
        <owl:inverseOf rdf:resource="http://www.w3id.org/efro/efro#includes"/>
        <rdfs:domain>
            <owl:Class>
                <owl:unionOf rdf:parseType="Collection">
                    <rdf:Description rdf:about="http://www.w3id.org/efro/efro#Learning"/>
                    <rdf:Description rdf:about="http://www.w3id.org/efro/efro#Person"/>
                </owl:unionOf>
            </owl:Class>
        </rdfs:domain>
        <dcterms:description xml:lang="en">Indicates an entity&apos;s relationship to a parent entity, such as a student belonging to an institution or a funding scheme.</dcterms:description>
        <rdfs:label>belongsTo</rdfs:label>
    </owl:ObjectProperty>
    


    <!-- http://www.w3id.org/efro/efro#constrains -->

    <owl:ObjectProperty rdf:about="http://www.w3id.org/efro/efro#constrains">
        <rdfs:subPropertyOf rdf:resource="http://www.w3.org/2002/07/owl#topObjectProperty"/>
        <rdfs:domain rdf:resource="http://www.w3id.org/efro/efro#TimeRelated"/>
        <rdfs:range rdf:resource="http://www.w3id.org/efro/efro#Activity"/>
    </owl:ObjectProperty>
    


    <!-- http://www.w3id.org/efro/efro#correspondsToLearningAim -->

    <owl:ObjectProperty rdf:about="http://www.w3id.org/efro/efro#correspondsToLearningAim">
        <rdfs:domain rdf:resource="http://www.w3id.org/efro/efro#ClassRegister"/>
        <rdfs:range rdf:resource="http://www.w3id.org/efro/efro#LearningAim"/>
        <rdfs:label>correspondsToLearningAim</rdfs:label>
    </owl:ObjectProperty>
    


    <!-- http://www.w3id.org/efro/efro#defines -->

    <owl:ObjectProperty rdf:about="http://www.w3id.org/efro/efro#defines">
        <rdfs:domain rdf:resource="http://www.w3id.org/efro/efro#FundingElement"/>
        <rdfs:range rdf:resource="http://www.w3id.org/efro/efro#FundingImpact"/>
        <rdfs:label>defines</rdfs:label>
    </owl:ObjectProperty>
    


    <!-- http://www.w3id.org/efro/efro#enrolledIn -->

    <owl:ObjectProperty rdf:about="http://www.w3id.org/efro/efro#enrolledIn">
        <owl:inverseOf rdf:resource="http://www.w3id.org/efro/efro#hasEnrollee"/>
        <rdfs:domain rdf:resource="http://www.w3id.org/efro/efro#Student"/>
        <rdfs:range rdf:resource="http://www.w3id.org/efro/efro#StudyProgramme"/>
        <dcterms:description xml:lang="en">Represents a student&apos;s enrolment in a specific programme, institution, or funding category​.</dcterms:description>
        <rdfs:label>enrolledIn</rdfs:label>
    </owl:ObjectProperty>
    


    <!-- http://www.w3id.org/efro/efro#evaluates -->

    <owl:ObjectProperty rdf:about="http://www.w3id.org/efro/efro#evaluates">
        <rdfs:domain rdf:resource="http://www.w3id.org/efro/efro#FundingElement"/>
        <rdfs:range rdf:resource="http://www.w3id.org/efro/efro#Activity"/>
    </owl:ObjectProperty>
    


    <!-- http://www.w3id.org/efro/efro#forProgramme -->

    <owl:ObjectProperty rdf:about="http://www.w3id.org/efro/efro#forProgramme">
        <rdfs:domain rdf:resource="http://www.w3id.org/efro/efro#Status"/>
        <rdfs:range rdf:resource="http://www.w3id.org/efro/efro#StudyProgramme"/>
        <rdfs:comment>for programme</rdfs:comment>
    </owl:ObjectProperty>
    


    <!-- http://www.w3id.org/efro/efro#fulfills -->

    <owl:ObjectProperty rdf:about="http://www.w3id.org/efro/efro#fulfills">
        <rdfs:subPropertyOf rdf:resource="http://www.w3.org/2002/07/owl#topObjectProperty"/>
        <rdfs:domain rdf:resource="http://www.w3id.org/efro/efro#Evidence"/>
        <rdfs:range rdf:resource="http://www.w3id.org/efro/efro#Obligation"/>
        <rdfs:label>fulfills</rdfs:label>
    </owl:ObjectProperty>
    


    <!-- http://www.w3id.org/efro/efro#givernedBy -->

    <owl:ObjectProperty rdf:about="http://www.w3id.org/efro/efro#givernedBy">
        <rdfs:domain rdf:resource="http://www.w3id.org/efro/efro#FundingRegulations"/>
        <rdfs:range rdf:resource="http://www.w3id.org/efro/efro#FundingElement"/>
        <rdfs:label>Governed By</rdfs:label>
    </owl:ObjectProperty>
    


    <!-- http://www.w3id.org/efro/efro#hasAchievementStatus -->

    <owl:ObjectProperty rdf:about="http://www.w3id.org/efro/efro#hasAchievementStatus">
        <rdfs:domain rdf:resource="http://www.w3id.org/efro/efro#Student"/>
        <rdfs:range rdf:resource="http://www.w3id.org/efro/efro#AchievementStatus"/>
        <dcterms:description xml:lang="en">Represents the status of a student’s academic or vocational achievement, tracking progress and outcomes.</dcterms:description>
        <rdfs:label>hasAchievementStatus</rdfs:label>
    </owl:ObjectProperty>
    


    <!-- http://www.w3id.org/efro/efro#hasActiveParticipation -->

    <owl:ObjectProperty rdf:about="http://www.w3id.org/efro/efro#hasActiveParticipation">
        <rdfs:subPropertyOf rdf:resource="http://www.w3id.org/efro/efro#hasParticipationStatus"/>
        <rdfs:domain rdf:resource="http://www.w3id.org/efro/efro#Student"/>
        <rdfs:range rdf:resource="http://www.w3id.org/efro/efro#ActiveParticipationStatus"/>
        <dcterms:description xml:lang="en">Indicates that a student is actively engaged in their learning and meets attendance requirements.</dcterms:description>
        <rdfs:label>hasActiveParticipation</rdfs:label>
    </owl:ObjectProperty>
    


    <!-- http://www.w3id.org/efro/efro#hasActualAttendance -->

    <owl:ObjectProperty rdf:about="http://www.w3id.org/efro/efro#hasActualAttendance">
        <rdfs:subPropertyOf rdf:resource="http://www.w3id.org/efro/efro#hasAttendanceRecord"/>
        <rdfs:domain rdf:resource="http://www.w3id.org/efro/efro#Student"/>
        <rdfs:range rdf:resource="http://www.w3id.org/efro/efro#ActualAttendanceActivity"/>
        <dcterms:description xml:lang="en">Tracks the actual attendance hours recorded for a student, ensuring compliance with funding regulations​.</dcterms:description>
        <rdfs:label>hasActualAttendance</rdfs:label>
    </owl:ObjectProperty>
    


    <!-- http://www.w3id.org/efro/efro#hasAdminSystemAccount -->

    <owl:ObjectProperty rdf:about="http://www.w3id.org/efro/efro#hasAdminSystemAccount">
        <rdfs:subPropertyOf rdf:resource="http://www.w3id.org/efro/efro#hasOnlineAccount"/>
        <rdfs:domain rdf:resource="http://www.w3id.org/efro/efro#Staff"/>
        <rdfs:range rdf:resource="http://xmlns.com/foaf/0.1/OnlineAccount"/>
        <rdfs:label>hasAdminSystemAccount</rdfs:label>
    </owl:ObjectProperty>
    


    <!-- http://www.w3id.org/efro/efro#hasAimStatus -->

    <owl:ObjectProperty rdf:about="http://www.w3id.org/efro/efro#hasAimStatus">
        <rdfs:domain rdf:resource="http://www.w3id.org/efro/efro#LearningAim"/>
        <rdfs:range rdf:resource="http://www.w3id.org/efro/efro#Status"/>
        <rdfs:label>has aim status</rdfs:label>
    </owl:ObjectProperty>
    


    <!-- http://www.w3id.org/efro/efro#hasApplicationStatus -->

    <owl:ObjectProperty rdf:about="http://www.w3id.org/efro/efro#hasApplicationStatus">
        <rdfs:subPropertyOf rdf:resource="http://www.w3id.org/efro/efro#hasStatus"/>
        <rdfs:domain rdf:resource="http://purl.org/cerif/frapo/Application"/>
        <rdfs:range rdf:resource="http://www.w3id.org/efro/efro#Status"/>
        <rdfs:label>hasApplicationStatus</rdfs:label>
    </owl:ObjectProperty>
    


    <!-- http://www.w3id.org/efro/efro#hasApplicationType -->

    <owl:ObjectProperty rdf:about="http://www.w3id.org/efro/efro#hasApplicationType">
        <rdfs:domain rdf:resource="http://purl.org/cerif/frapo/Application"/>
        <rdfs:range rdf:resource="http://www.w3id.org/efro/efro#LearningAim"/>
        <rdfs:label>hasApplicationType</rdfs:label>
    </owl:ObjectProperty>
    


    <!-- http://www.w3id.org/efro/efro#hasApprenticeshipFunding -->

    <owl:ObjectProperty rdf:about="http://www.w3id.org/efro/efro#hasApprenticeshipFunding">
        <rdfs:subPropertyOf rdf:resource="http://www.w3id.org/efro/efro#hasFundingElement"/>
        <rdfs:domain>
            <owl:Class>
                <owl:unionOf rdf:parseType="Collection">
                    <rdf:Description rdf:about="http://www.w3id.org/efro/efro#Learning"/>
                    <rdf:Description rdf:about="http://www.w3id.org/efro/efro#Student"/>
                </owl:unionOf>
            </owl:Class>
        </rdfs:domain>
        <rdfs:range rdf:resource="http://www.w3id.org/efro/efro#ApprenticeshipFunding"/>
        <dcterms:description xml:lang="en">Denotes funding specifically allocated for apprenticeship programmes, covering training, assessment, and employer incentives.</dcterms:description>
        <rdfs:label>hasApprenticeshipFunding</rdfs:label>
    </owl:ObjectProperty>
    


    <!-- http://www.w3id.org/efro/efro#hasAssessmentRecord -->

    <owl:ObjectProperty rdf:about="http://www.w3id.org/efro/efro#hasAssessmentRecord">
        <owl:inverseOf rdf:resource="http://www.w3id.org/efro/efro#isAssessmentRecord"/>
        <rdfs:domain rdf:resource="http://www.w3id.org/efro/efro#Student"/>
        <rdfs:range rdf:resource="http://www.w3id.org/efro/efro#AssessmentActivity"/>
        <dcterms:description xml:lang="en">Links a student’s assessment records, such as examinations, assignments, and overall performance tracking.</dcterms:description>
        <rdfs:label>hasAssessmentRecord</rdfs:label>
    </owl:ObjectProperty>
    


    <!-- http://www.w3id.org/efro/efro#hasAssignmentCompletion -->

    <owl:ObjectProperty rdf:about="http://www.w3id.org/efro/efro#hasAssignmentCompletion">
        <rdfs:subPropertyOf rdf:resource="http://www.w3id.org/efro/efro#hasAssessmentRecord"/>
        <rdfs:domain rdf:resource="http://www.w3id.org/efro/efro#Student"/>
        <rdfs:range rdf:resource="http://www.w3id.org/efro/efro#AssignmentActivity"/>
        <dcterms:description xml:lang="en">Indicates that a student has submitted and completed a required assignment as part of their programme​.</dcterms:description>
        <rdfs:label>hasAssignmentCompletion</rdfs:label>
    </owl:ObjectProperty>
    


    <!-- http://www.w3id.org/efro/efro#hasAssociatedDocument -->

    <owl:ObjectProperty rdf:about="http://www.w3id.org/efro/efro#hasAssociatedDocument">
        <rdfs:domain rdf:resource="http://www.w3id.org/efro/efro#Obligation"/>
        <rdfs:range rdf:resource="http://www.w3id.org/efro/efro#Document"/>
        <dcterms:description xml:lang="en">Links an entity (e.g., student, programme, funding application) to a supporting document such as a learning agreement, enrolment form, or funding claim.</dcterms:description>
        <rdfs:label>hasAssociatedDocument</rdfs:label>
    </owl:ObjectProperty>
    


    <!-- http://www.w3id.org/efro/efro#hasAttendanceEvidence -->

    <owl:ObjectProperty rdf:about="http://www.w3id.org/efro/efro#hasAttendanceEvidence">
        <rdfs:domain rdf:resource="http://www.w3id.org/efro/efro#LastAttendanceActivity"/>
        <rdfs:range rdf:resource="http://www.w3id.org/efro/efro#ClassRegister"/>
        <dcterms:description xml:lang="en">Refers to records that demonstrate a student&apos;s attendance in learning activities, which is essential for funding eligibility.</dcterms:description>
        <rdfs:label>hasAttendanceEvidence</rdfs:label>
    </owl:ObjectProperty>
    


    <!-- http://www.w3id.org/efro/efro#hasAttendanceRecord -->

    <owl:ObjectProperty rdf:about="http://www.w3id.org/efro/efro#hasAttendanceRecord">
        <owl:inverseOf rdf:resource="http://www.w3id.org/efro/efro#isAttendanceRecordOf"/>
        <rdfs:domain rdf:resource="http://www.w3id.org/efro/efro#Student"/>
        <rdfs:range rdf:resource="http://www.w3id.org/efro/efro#AttendanceActivity"/>
        <dcterms:description xml:lang="en">Represents a student’s attendance data, used to validate funding claims and student engagement.</dcterms:description>
        <rdfs:label>hasAttendanceRecord</rdfs:label>
    </owl:ObjectProperty>
    


    <!-- http://www.w3id.org/efro/efro#hasClassRegister -->

    <owl:ObjectProperty rdf:about="http://www.w3id.org/efro/efro#hasClassRegister">
        <rdfs:domain rdf:resource="http://www.w3id.org/efro/efro#LastAttendanceActivity"/>
        <rdfs:range rdf:resource="http://www.w3id.org/efro/efro#ClassRegister"/>
        <dcterms:description xml:lang="en">Links a student or programme to an official attendance register used to record participation​.</dcterms:description>
        <rdfs:label>hasClassRegister</rdfs:label>
    </owl:ObjectProperty>
    


    <!-- http://www.w3id.org/efro/efro#hasCompletionStatus -->

    <owl:ObjectProperty rdf:about="http://www.w3id.org/efro/efro#hasCompletionStatus">
        <rdfs:domain>
            <owl:Class>
                <owl:unionOf rdf:parseType="Collection">
                    <rdf:Description rdf:about="http://www.w3id.org/efro/efro#CompletionStatus"/>
                    <rdf:Description rdf:about="http://www.w3id.org/efro/efro#Student"/>
                </owl:unionOf>
            </owl:Class>
        </rdfs:domain>
        <rdfs:range rdf:resource="http://www.w3id.org/efro/efro#CompletionStatus"/>
        <dcterms:description xml:lang="en">Represents the completion status of a student&apos;s learning aim or study programme, whether successful, withdrawn, or incomplete.</dcterms:description>
        <rdfs:label>hasCompletionStatus</rdfs:label>
    </owl:ObjectProperty>
    


    <!-- http://www.w3id.org/efro/efro#hasComplianceRequirement -->

    <owl:ObjectProperty rdf:about="http://www.w3id.org/efro/efro#hasComplianceRequirement">
        <rdfs:subPropertyOf rdf:resource="http://www.w3id.org/efro/efro#hasLegalDuty"/>
        <owl:inverseOf rdf:resource="http://www.w3id.org/efro/efro#isComplianceRequirementFor"/>
        <rdfs:domain rdf:resource="http://www.w3id.org/efro/efro#FundedInstitution"/>
        <rdfs:range rdf:resource="http://www.w3id.org/efro/efro#ComplianceObligation"/>
        <dcterms:description xml:lang="en">Defines the legal and regulatory requirements institutions must meet to receive and maintain funding.</dcterms:description>
        <rdfs:label>hasComplianceRequirement</rdfs:label>
    </owl:ObjectProperty>
    


    <!-- http://www.w3id.org/efro/efro#hasDistanceLearningProvision -->

    <owl:ObjectProperty rdf:about="http://www.w3id.org/efro/efro#hasDistanceLearningProvision">
        <rdfs:subPropertyOf rdf:resource="http://www.w3id.org/efro/efro#hasLearningMode"/>
        <rdfs:domain rdf:resource="http://www.w3id.org/efro/efro#Learning"/>
        <rdfs:range rdf:resource="http://www.w3id.org/efro/efro#DistanceLearningProvision"/>
        <dcterms:description xml:lang="en">Represents learning that occurs remotely, without requiring physical attendance at an institution.</dcterms:description>
        <rdfs:label>hasDistanceLearningProvision</rdfs:label>
    </owl:ObjectProperty>
    


    <!-- http://www.w3id.org/efro/efro#hasDocumentation -->

    <owl:ObjectProperty rdf:about="http://www.w3id.org/efro/efro#hasDocumentation">
        <rdfs:domain rdf:resource="http://www.w3id.org/efro/efro#Reason"/>
        <rdfs:range rdf:resource="http://www.w3id.org/efro/efro#Document"/>
        <dcterms:description xml:lang="en">Indicates the presence of required supporting documents for enrolment, funding applications, or compliance.</dcterms:description>
        <rdfs:label>hasDocumentation</rdfs:label>
    </owl:ObjectProperty>
    


    <!-- http://www.w3id.org/efro/efro#hasDoubleFundingRestriction -->

    <owl:ObjectProperty rdf:about="http://www.w3id.org/efro/efro#hasDoubleFundingRestriction">
        <rdfs:subPropertyOf rdf:resource="http://www.w3id.org/efro/efro#hasFundingCondition"/>
        <rdfs:domain rdf:resource="http://www.w3id.org/efro/efro#FundingElement"/>
        <rdfs:range rdf:resource="http://www.w3id.org/efro/efro#DoubleFundingRestriction"/>
        <dcterms:description xml:lang="en">Prevents a student from being funded simultaneously by multiple programmes or institutions.</dcterms:description>
        <rdfs:label>hasDoubleFundingRestriction</rdfs:label>
    </owl:ObjectProperty>
    


    <!-- http://www.w3id.org/efro/efro#hasESFAFunding -->

    <owl:ObjectProperty rdf:about="http://www.w3id.org/efro/efro#hasESFAFunding">
        <rdfs:subPropertyOf rdf:resource="http://www.w3id.org/efro/efro#hasFundingElement"/>
        <rdfs:domain>
            <owl:Class>
                <owl:unionOf rdf:parseType="Collection">
                    <rdf:Description rdf:about="http://www.w3id.org/efro/efro#Learning"/>
                    <rdf:Description rdf:about="http://www.w3id.org/efro/efro#Student"/>
                </owl:unionOf>
            </owl:Class>
        </rdfs:domain>
        <rdfs:range rdf:resource="http://www.w3id.org/efro/efro#ESFAFunding"/>
        <dcterms:description xml:lang="en">Indicates financial support provided by the Education and Skills Funding Agency (ESFA) for 16-19 education, adult learning, and traineeships.</dcterms:description>
        <rdfs:label>hasESFAFunding</rdfs:label>
    </owl:ObjectProperty>
    


    <!-- http://www.w3id.org/efro/efro#hasEarlyCompletion -->

    <owl:ObjectProperty rdf:about="http://www.w3id.org/efro/efro#hasEarlyCompletion">
        <rdfs:subPropertyOf rdf:resource="http://www.w3id.org/efro/efro#hasAchievementStatus"/>
        <rdfs:domain rdf:resource="http://www.w3id.org/efro/efro#AchievementStatus"/>
        <rdfs:range rdf:resource="http://www.w3id.org/efro/efro#EarlyCompletionStatus"/>
        <dcterms:description xml:lang="en">Indicates that a student has completed their programme earlier than planned, which may impact funding adjustments​.</dcterms:description>
        <rdfs:label>hasEarlyCompletion</rdfs:label>
    </owl:ObjectProperty>
    


    <!-- http://www.w3id.org/efro/efro#hasEarlyCompletionStatus -->

    <owl:ObjectProperty rdf:about="http://www.w3id.org/efro/efro#hasEarlyCompletionStatus">
        <rdfs:subPropertyOf rdf:resource="http://www.w3id.org/efro/efro#hasParticipationStatus"/>
        <rdfs:domain rdf:resource="http://www.w3id.org/efro/efro#Student"/>
        <rdfs:range rdf:resource="http://www.w3id.org/efro/efro#EarlyCompletionStatus"/>
        <dcterms:description xml:lang="en">Captures the status of a student who has completed their programme ahead of the planned schedule.</dcterms:description>
        <rdfs:label>hasEarlyCompletionStatus</rdfs:label>
    </owl:ObjectProperty>
    


    <!-- http://www.w3id.org/efro/efro#hasEnrollee -->

    <owl:ObjectProperty rdf:about="http://www.w3id.org/efro/efro#hasEnrollee">
        <rdfs:domain rdf:resource="http://www.w3id.org/efro/efro#StudyProgramme"/>
        <rdfs:range rdf:resource="http://www.w3id.org/efro/efro#Student"/>
        <dcterms:description xml:lang="en">Links a student to an educational institution or programme in which they are officially enrolled​.</dcterms:description>
        <rdfs:label>hasEnrollee</rdfs:label>
    </owl:ObjectProperty>
    


    <!-- http://www.w3id.org/efro/efro#hasExaminationResult -->

    <owl:ObjectProperty rdf:about="http://www.w3id.org/efro/efro#hasExaminationResult">
        <rdfs:subPropertyOf rdf:resource="http://www.w3id.org/efro/efro#hasAssessmentRecord"/>
        <rdfs:domain rdf:resource="http://www.w3id.org/efro/efro#Student"/>
        <rdfs:range rdf:resource="http://www.w3id.org/efro/efro#ExaminationActivity"/>
        <dcterms:description xml:lang="en">Represents the student’s performance in formal exams, recorded for academic and funding purposes.</dcterms:description>
        <rdfs:label>hasExaminationResult</rdfs:label>
    </owl:ObjectProperty>
    


    <!-- http://www.w3id.org/efro/efro#hasFundedStudent -->

    <owl:ObjectProperty rdf:about="http://www.w3id.org/efro/efro#hasFundedStudent">
        <rdfs:domain rdf:resource="http://www.w3id.org/efro/efro#FundingClaimReport"/>
        <rdfs:range rdf:resource="http://www.w3id.org/efro/efro#Student"/>
        <dcterms:description xml:lang="en">Connects a student to a funding allocation, indicating that they have been approved for financial support​.</dcterms:description>
        <rdfs:label>hasFundedStudent</rdfs:label>
    </owl:ObjectProperty>
    


    <!-- http://www.w3id.org/efro/efro#hasFunding -->

    <owl:ObjectProperty rdf:about="http://www.w3id.org/efro/efro#hasFunding">
        <owl:inverseOf rdf:resource="http://www.w3id.org/efro/efro#isFundedBy"/>
        <rdfs:domain>
            <owl:Class>
                <owl:unionOf rdf:parseType="Collection">
                    <rdf:Description rdf:about="http://www.w3id.org/efro/efro#EducationalEntity"/>
                    <rdf:Description rdf:about="http://www.w3id.org/efro/efro#Learning"/>
                </owl:unionOf>
            </owl:Class>
        </rdfs:domain>
        <rdfs:range rdf:resource="http://www.w3id.org/efro/efro#FundingElement"/>
        <dcterms:description xml:lang="en">Represents the financial resources allocated to a student, programme, or institution.</dcterms:description>
        <rdfs:label>hasFunding</rdfs:label>
    </owl:ObjectProperty>
    


    <!-- http://www.w3id.org/efro/efro#hasFundingBand -->

    <owl:ObjectProperty rdf:about="http://www.w3id.org/efro/efro#hasFundingBand">
        <rdfs:subPropertyOf rdf:resource="http://www.w3id.org/efro/efro#hasFundingElement"/>
        <rdfs:domain>
            <owl:Class>
                <owl:unionOf rdf:parseType="Collection">
                    <rdf:Description rdf:about="http://www.w3id.org/efro/efro#Learning"/>
                    <rdf:Description rdf:about="http://www.w3id.org/efro/efro#Student"/>
                </owl:unionOf>
            </owl:Class>
        </rdfs:domain>
        <rdfs:range rdf:resource="http://www.w3id.org/efro/efro#FundingBand"/>
        <dcterms:description xml:lang="en">Represents the predefined levels or categories that determine funding allocation for specific learning aims.</dcterms:description>
        <rdfs:label>hasFundingBand</rdfs:label>
    </owl:ObjectProperty>
    


    <!-- http://www.w3id.org/efro/efro#hasFundingCondition -->

    <owl:ObjectProperty rdf:about="http://www.w3id.org/efro/efro#hasFundingCondition">
        <rdfs:domain rdf:resource="http://www.w3id.org/efro/efro#FundingElement"/>
        <rdfs:range rdf:resource="http://www.w3id.org/efro/efro#FundingCondition"/>
        <dcterms:description xml:lang="en">Defines the rules and conditions that govern funding eligibility, allocation, and restrictions.</dcterms:description>
        <rdfs:label>hasFundingCondition</rdfs:label>
    </owl:ObjectProperty>
    


    <!-- http://www.w3id.org/efro/efro#hasFundingElement -->

    <owl:ObjectProperty rdf:about="http://www.w3id.org/efro/efro#hasFundingElement">
        <rdfs:domain>
            <owl:Class>
                <owl:unionOf rdf:parseType="Collection">
                    <rdf:Description rdf:about="http://www.w3id.org/efro/efro#Learning"/>
                    <rdf:Description rdf:about="http://www.w3id.org/efro/efro#Student"/>
                </owl:unionOf>
            </owl:Class>
        </rdfs:domain>
        <rdfs:range rdf:resource="http://www.w3id.org/efro/efro#FundingElement"/>
        <dcterms:description xml:lang="en">Represents different components of funding allocated to a student, institution, or programme.</dcterms:description>
        <rdfs:label>hasFundingElement</rdfs:label>
    </owl:ObjectProperty>
    


    <!-- http://www.w3id.org/efro/efro#hasFundingImpact -->

    <owl:ObjectProperty rdf:about="http://www.w3id.org/efro/efro#hasFundingImpact">
        <rdfs:domain rdf:resource="http://www.w3id.org/efro/efro#Activity"/>
        <rdfs:range rdf:resource="http://www.w3id.org/efro/efro#FundingImpact"/>
        <rdfs:label>has funding impact</rdfs:label>
    </owl:ObjectProperty>
    


    <!-- http://www.w3id.org/efro/efro#hasFundingObligation -->

    <owl:ObjectProperty rdf:about="http://www.w3id.org/efro/efro#hasFundingObligation">
        <rdfs:subPropertyOf rdf:resource="http://www.w3id.org/efro/efro#hasLegalDuty"/>
        <owl:inverseOf rdf:resource="http://www.w3id.org/efro/efro#isFundingObligationFor"/>
        <rdfs:domain rdf:resource="http://www.w3id.org/efro/efro#FundedInstitution"/>
        <rdfs:range rdf:resource="http://www.w3id.org/efro/efro#FundingObligation"/>
        <dcterms:description xml:lang="en">Specifies the conditions that institutions must fulfill to qualify for and continue receiving financial support.</dcterms:description>
        <rdfs:label>hasFundingObligation</rdfs:label>
    </owl:ObjectProperty>
    


    <!-- http://www.w3id.org/efro/efro#hasFundingOverlap -->

    <owl:ObjectProperty rdf:about="http://www.w3id.org/efro/efro#hasFundingOverlap">
        <rdfs:subPropertyOf rdf:resource="http://www.w3id.org/efro/efro#hasFundingCondition"/>
        <rdfs:domain rdf:resource="http://www.w3id.org/efro/efro#FundingElement"/>
        <rdfs:range rdf:resource="http://www.w3id.org/efro/efro#FundingOverlap"/>
        <dcterms:description xml:lang="en">Identifies cases where a student’s funding periods overlap, ensuring they do not receive duplicate funding.</dcterms:description>
        <rdfs:label>hasFundingOverlap</rdfs:label>
    </owl:ObjectProperty>
    


    <!-- http://www.w3id.org/efro/efro#hasFundingStartStatus -->

    <owl:ObjectProperty rdf:about="http://www.w3id.org/efro/efro#hasFundingStartStatus">
        <rdfs:domain rdf:resource="http://www.w3id.org/efro/efro#Student"/>
        <rdfs:range rdf:resource="http://www.w3id.org/efro/efro#FundingStartStatus"/>
        <dcterms:description xml:lang="en">Captures the initial status of a student or programme at the beginning of a funding period, ensuring eligibility and compliance​.</dcterms:description>
        <rdfs:label>hasFundingStartStatus</rdfs:label>
    </owl:ObjectProperty>
    


    <!-- http://www.w3id.org/efro/efro#hasGroupStatus -->

    <owl:ObjectProperty rdf:about="http://www.w3id.org/efro/efro#hasGroupStatus">
        <rdfs:subPropertyOf rdf:resource="http://www.w3id.org/efro/efro#hasStatus"/>
        <rdfs:domain rdf:resource="http://xmlns.com/foaf/0.1/Group"/>
        <rdfs:range rdf:resource="http://www.w3id.org/efro/efro#Status"/>
        <rdfs:label>hasGroupStatus</rdfs:label>
    </owl:ObjectProperty>
    


    <!-- http://www.w3id.org/efro/efro#hasGroupType -->

    <owl:ObjectProperty rdf:about="http://www.w3id.org/efro/efro#hasGroupType">
        <rdfs:domain rdf:resource="http://xmlns.com/foaf/0.1/Group"/>
        <rdfs:range rdf:resource="http://www.w3id.org/efro/efro#LearningMode"/>
        <rdfs:label>hasGroupType</rdfs:label>
    </owl:ObjectProperty>
    


    <!-- http://www.w3id.org/efro/efro#hasGuidedLearning -->

    <owl:ObjectProperty rdf:about="http://www.w3id.org/efro/efro#hasGuidedLearning">
        <rdfs:subPropertyOf rdf:resource="http://www.w3id.org/efro/efro#hasLearningMode"/>
        <rdfs:domain rdf:resource="http://www.w3id.org/efro/efro#Learning"/>
        <rdfs:range rdf:resource="http://www.w3id.org/efro/efro#GuidedLearning"/>
        <dcterms:description xml:lang="en">Indicates structured learning activities under the direct supervision of an instructor or tutor.</dcterms:description>
        <rdfs:label>hasGuidedLearning</rdfs:label>
    </owl:ObjectProperty>
    


    <!-- http://www.w3id.org/efro/efro#hasInfrastructureType -->

    <owl:ObjectProperty rdf:about="http://www.w3id.org/efro/efro#hasInfrastructureType">
        <rdfs:domain rdf:resource="http://purl.org/cerif/frapo/InfrastructureEntity"/>
        <rdfs:range rdf:resource="http://www.w3id.org/efro/efro#LearningMode"/>
        <rdfs:label>hasInfrastructureType</rdfs:label>
    </owl:ObjectProperty>
    


    <!-- http://www.w3id.org/efro/efro#hasInitialPlannedHours -->

    <owl:ObjectProperty rdf:about="http://www.w3id.org/efro/efro#hasInitialPlannedHours">
        <rdfs:subPropertyOf rdf:resource="http://www.w3id.org/efro/efro#hasPlannedHoursManagement"/>
        <rdfs:domain rdf:resource="http://www.w3id.org/efro/efro#Learning"/>
        <rdfs:range rdf:resource="http://www.w3id.org/efro/efro#InitialPlannedHours"/>
        <dcterms:description xml:lang="en">Captures the number of learning hours assigned to a student when they first enroll in a study programme.</dcterms:description>
        <rdfs:label>hasInitialPlannedHours</rdfs:label>
    </owl:ObjectProperty>
    


    <!-- http://www.w3id.org/efro/efro#hasInstitutionalAccount -->

    <owl:ObjectProperty rdf:about="http://www.w3id.org/efro/efro#hasInstitutionalAccount">
        <rdfs:subPropertyOf rdf:resource="http://www.w3id.org/efro/efro#hasOnlineAccount"/>
        <rdfs:domain rdf:resource="http://www.w3id.org/efro/efro#EducationalEntity"/>
        <rdfs:range rdf:resource="http://xmlns.com/foaf/0.1/OnlineAccount"/>
        <rdfs:label>hasInstitutionalAccount</rdfs:label>
    </owl:ObjectProperty>
    


    <!-- http://www.w3id.org/efro/efro#hasLastAttendance -->

    <owl:ObjectProperty rdf:about="http://www.w3id.org/efro/efro#hasLastAttendance">
        <rdfs:subPropertyOf rdf:resource="http://www.w3id.org/efro/efro#hasAttendanceRecord"/>
        <rdfs:domain rdf:resource="http://www.w3id.org/efro/efro#Student"/>
        <rdfs:range rdf:resource="http://www.w3id.org/efro/efro#LastAttendanceActivity"/>
        <dcterms:description xml:lang="en">Captures the most recent attendance record before a student withdraws or completes their programme​.</dcterms:description>
        <rdfs:label>hasLastAttendance</rdfs:label>
    </owl:ObjectProperty>
    


    <!-- http://www.w3id.org/efro/efro#hasLearningAim -->

    <owl:ObjectProperty rdf:about="http://www.w3id.org/efro/efro#hasLearningAim">
        <rdfs:domain rdf:resource="http://www.w3id.org/efro/efro#StudyProgramme"/>
        <rdfs:range rdf:resource="http://www.w3id.org/efro/efro#LearningAim"/>
        <dcterms:description xml:lang="en">Defines the objectives or intended outcomes of a student’s learning programme.</dcterms:description>
        <rdfs:label>hasLearningAim</rdfs:label>
    </owl:ObjectProperty>
    


    <!-- http://www.w3id.org/efro/efro#hasLearningMode -->

    <owl:ObjectProperty rdf:about="http://www.w3id.org/efro/efro#hasLearningMode">
        <rdfs:domain rdf:resource="http://www.w3id.org/efro/efro#Learning"/>
        <rdfs:range rdf:resource="http://www.w3id.org/efro/efro#LearningMode"/>
        <dcterms:description xml:lang="en">Specifies the method or format in which learning is delivered.</dcterms:description>
        <rdfs:label>hasLearningMode</rdfs:label>
    </owl:ObjectProperty>
    


    <!-- http://www.w3id.org/efro/efro#hasLearningPlatformAccount -->

    <owl:ObjectProperty rdf:about="http://www.w3id.org/efro/efro#hasLearningPlatformAccount">
        <rdfs:subPropertyOf rdf:resource="http://www.w3id.org/efro/efro#hasOnlineAccount"/>
        <rdfs:domain rdf:resource="http://www.w3id.org/efro/efro#Student"/>
        <rdfs:range rdf:resource="http://xmlns.com/foaf/0.1/OnlineAccount"/>
        <rdfs:label>hasLearningPlatformAccount</rdfs:label>
    </owl:ObjectProperty>
    


    <!-- http://www.w3id.org/efro/efro#hasLegalDuty -->

    <owl:ObjectProperty rdf:about="http://www.w3id.org/efro/efro#hasLegalDuty">
        <rdfs:domain rdf:resource="http://www.w3id.org/efro/efro#EducationalEntity"/>
        <rdfs:range rdf:resource="http://www.w3id.org/efro/efro#Obligation"/>
        <dcterms:description xml:lang="en">Represents legal responsibilities institutions must fulfill regarding funding, student participation, and compliance.</dcterms:description>
        <rdfs:label>hasLegalDuty</rdfs:label>
    </owl:ObjectProperty>
    


    <!-- http://www.w3id.org/efro/efro#hasNonAttendance -->

    <owl:ObjectProperty rdf:about="http://www.w3id.org/efro/efro#hasNonAttendance">
        <rdfs:subPropertyOf rdf:resource="http://www.w3id.org/efro/efro#hasAttendanceRecord"/>
        <rdfs:domain rdf:resource="http://www.w3id.org/efro/efro#Student"/>
        <rdfs:range rdf:resource="http://www.w3id.org/efro/efro#NonAttendanceActivity"/>
        <dcterms:description xml:lang="en">Records instances where a student has failed to attend required sessions, which may impact their funding eligibility.</dcterms:description>
        <rdfs:label>hasNonAttendance</rdfs:label>
    </owl:ObjectProperty>
    


    <!-- http://www.w3id.org/efro/efro#hasNonQualificationAim -->

    <owl:ObjectProperty rdf:about="http://www.w3id.org/efro/efro#hasNonQualificationAim">
        <rdfs:subPropertyOf rdf:resource="http://www.w3id.org/efro/efro#hasLearningAim"/>
        <rdfs:domain rdf:resource="http://www.w3id.org/efro/efro#StudyProgramme"/>
        <rdfs:range rdf:resource="http://www.w3id.org/efro/efro#NonQualificationAim"/>
        <dcterms:description xml:lang="en">Refers to learning activities that do not lead to formal qualifications, such as employability training or enrichment activities.</dcterms:description>
        <rdfs:label>hasNonQualificationAim</rdfs:label>
    </owl:ObjectProperty>
    


    <!-- http://www.w3id.org/efro/efro#hasOnlineAccount -->

    <owl:ObjectProperty rdf:about="http://www.w3id.org/efro/efro#hasOnlineAccount">
        <rdfs:domain rdf:resource="http://www.w3id.org/efro/efro#Person"/>
        <rdfs:range rdf:resource="http://xmlns.com/foaf/0.1/OnlineAccount"/>
        <rdfs:label>hasOnlineAccount</rdfs:label>
    </owl:ObjectProperty>
    


    <!-- http://www.w3id.org/efro/efro#hasOpenLearningProvision -->

    <owl:ObjectProperty rdf:about="http://www.w3id.org/efro/efro#hasOpenLearningProvision">
        <rdfs:subPropertyOf rdf:resource="http://www.w3id.org/efro/efro#hasLearningMode"/>
        <rdfs:domain rdf:resource="http://www.w3id.org/efro/efro#Learning"/>
        <rdfs:range rdf:resource="http://www.w3id.org/efro/efro#OpenLearningProvision"/>
        <dcterms:description xml:lang="en">Refers to flexible learning models that allow students to access materials and progress at their own pace.</dcterms:description>
        <rdfs:label>hasOpenLearningProvision</rdfs:label>
    </owl:ObjectProperty>
    


    <!-- http://www.w3id.org/efro/efro#hasParticipant -->

    <owl:ObjectProperty rdf:about="http://www.w3id.org/efro/efro#hasParticipant">
        <owl:inverseOf rdf:resource="http://www.w3id.org/efro/efro#participatesIn"/>
        <rdfs:domain rdf:resource="http://www.w3id.org/efro/efro#Activity"/>
        <rdfs:range rdf:resource="http://www.w3id.org/efro/efro#Person"/>
        <dcterms:description xml:lang="en">Identifies students or staff involved in a study programme, funding scheme, or learning activity.</dcterms:description>
        <rdfs:label>hasParticipant</rdfs:label>
    </owl:ObjectProperty>
    


    <!-- http://www.w3id.org/efro/efro#hasParticipationStatus -->

    <owl:ObjectProperty rdf:about="http://www.w3id.org/efro/efro#hasParticipationStatus">
        <rdfs:domain rdf:resource="http://www.w3id.org/efro/efro#Student"/>
        <rdfs:range rdf:resource="http://www.w3id.org/efro/efro#ParticipationStatus"/>
        <dcterms:description xml:lang="en">Represents a student&apos;s engagement level in their learning programme.</dcterms:description>
        <rdfs:label>hasParticipationStatus</rdfs:label>
    </owl:ObjectProperty>
    


    <!-- http://www.w3id.org/efro/efro#hasPeriodTotal -->

    <owl:ObjectProperty rdf:about="http://www.w3id.org/efro/efro#hasPeriodTotal">
        <rdfs:domain rdf:resource="http://www.w3id.org/efro/efro#PlannedHours"/>
        <rdfs:range rdf:resource="http://www.w3id.org/efro/efro#PlannedHours"/>
        <dcterms:description xml:lang="en">Represents the total allocated funding, hours, or duration for a specific funding period.</dcterms:description>
        <rdfs:label>hasPeriodTotal</rdfs:label>
    </owl:ObjectProperty>
    


    <!-- http://www.w3id.org/efro/efro#hasPersonalReason -->

    <owl:ObjectProperty rdf:about="http://www.w3id.org/efro/efro#hasPersonalReason">
        <rdfs:subPropertyOf rdf:resource="http://www.w3id.org/efro/efro#hasWithdrawalReason"/>
        <rdfs:domain rdf:resource="http://www.w3id.org/efro/efro#WithdrawalActivity"/>
        <rdfs:range rdf:resource="http://www.w3id.org/efro/efro#PersonalReason"/>
        <dcterms:description xml:lang="en">Indicates withdrawal due to personal circumstances such as health issues, family commitments, or relocation.</dcterms:description>
        <rdfs:label>hasPersonalReason</rdfs:label>
    </owl:ObjectProperty>
    


    <!-- http://www.w3id.org/efro/efro#hasPlannedHours -->

    <owl:ObjectProperty rdf:about="http://www.w3id.org/efro/efro#hasPlannedHours">
        <rdfs:domain>
            <owl:Class>
                <owl:unionOf rdf:parseType="Collection">
                    <rdf:Description rdf:about="http://www.w3id.org/efro/efro#Learning"/>
                    <rdf:Description rdf:about="http://www.w3id.org/efro/efro#StudyProgramme"/>
                </owl:unionOf>
            </owl:Class>
        </rdfs:domain>
        <rdfs:range rdf:resource="http://www.w3id.org/efro/efro#PlannedHours"/>
        <dcterms:description xml:lang="en">Represents the number of learning hours planned for a student at the beginning of the academic year, used for funding calculations.</dcterms:description>
        <rdfs:label>hasPlannedHours</rdfs:label>
    </owl:ObjectProperty>
    


    <!-- http://www.w3id.org/efro/efro#hasPlannedHoursManagement -->

    <owl:ObjectProperty rdf:about="http://www.w3id.org/efro/efro#hasPlannedHoursManagement">
        <rdfs:domain rdf:resource="http://www.w3id.org/efro/efro#Learning"/>
        <rdfs:range rdf:resource="http://www.w3id.org/efro/efro#PlannedHours"/>
        <dcterms:description xml:lang="en">Represents the processes involved in recording, managing, and adjusting planned learning hours.</dcterms:description>
        <rdfs:label>hasPlannedHoursManagement</rdfs:label>
    </owl:ObjectProperty>
    


    <!-- http://www.w3id.org/efro/efro#hasProgression -->

    <owl:ObjectProperty rdf:about="http://www.w3id.org/efro/efro#hasProgression">
        <rdfs:domain rdf:resource="http://www.w3id.org/efro/efro#Student"/>
        <rdfs:range rdf:resource="http://www.w3id.org/efro/efro#ProgressionActivity"/>
        <dcterms:description xml:lang="en">Indicates a student&apos;s movement from one stage of a programme to another, such as transitioning from one qualification level to the next.</dcterms:description>
        <rdfs:label>hasProgression</rdfs:label>
    </owl:ObjectProperty>
    


    <!-- http://www.w3id.org/efro/efro#hasProgressionActivity -->

    <owl:ObjectProperty rdf:about="http://www.w3id.org/efro/efro#hasProgressionActivity">
        <rdfs:domain rdf:resource="http://www.w3id.org/efro/efro#Student"/>
        <rdfs:range rdf:resource="http://www.w3id.org/efro/efro#ProgressionActivity"/>
        <dcterms:description xml:lang="en">Refers to specific activities that support a student&apos;s educational progression, such as additional training, assessments, or workshops.</dcterms:description>
        <rdfs:label>hasProgressionActivity</rdfs:label>
    </owl:ObjectProperty>
    


    <!-- http://www.w3id.org/efro/efro#hasProgressionReason -->

    <owl:ObjectProperty rdf:about="http://www.w3id.org/efro/efro#hasProgressionReason">
        <rdfs:subPropertyOf rdf:resource="http://www.w3id.org/efro/efro#hasWithdrawalReason"/>
        <rdfs:domain rdf:resource="http://www.w3id.org/efro/efro#WithdrawalActivity"/>
        <rdfs:range rdf:resource="http://www.w3id.org/efro/efro#ProgressionReason"/>
        <dcterms:description>Denotes withdrawal due to progression to a higher-level course, employment, or alternative educational opportunities.</dcterms:description>
        <rdfs:label>hasProgressionReason</rdfs:label>
    </owl:ObjectProperty>
    


    <!-- http://www.w3id.org/efro/efro#hasProgressionStatus -->

    <owl:ObjectProperty rdf:about="http://www.w3id.org/efro/efro#hasProgressionStatus">
        <rdfs:subPropertyOf rdf:resource="http://www.w3id.org/efro/efro#hasAssessmentRecord"/>
        <owl:inverseOf rdf:resource="http://www.w3id.org/efro/efro#isProgressionStatusOf"/>
        <rdfs:domain rdf:resource="http://www.w3id.org/efro/efro#Student"/>
        <rdfs:range rdf:resource="http://www.w3id.org/efro/efro#ProgressionActivity"/>
        <dcterms:description xml:lang="en">Captures the progression of a student based on their assessment and qualification achievements.</dcterms:description>
        <rdfs:label>hasProgressionStatus</rdfs:label>
    </owl:ObjectProperty>
    


    <!-- http://www.w3id.org/efro/efro#hasProgressionType -->

    <owl:ObjectProperty rdf:about="http://www.w3id.org/efro/efro#hasProgressionType">
        <rdfs:domain rdf:resource="http://www.w3id.org/efro/efro#ProgressionActivity"/>
        <rdfs:range rdf:resource="http://www.w3id.org/efro/efro#ProgressionType"/>
        <dcterms:description xml:lang="en">Defines the type of progression a student undergoes, such as academic, vocational, or skill-based.</dcterms:description>
        <rdfs:label>hasProgressionType</rdfs:label>
    </owl:ObjectProperty>
    


    <!-- http://www.w3id.org/efro/efro#hasQualificationAim -->

    <owl:ObjectProperty rdf:about="http://www.w3id.org/efro/efro#hasQualificationAim">
        <rdfs:subPropertyOf rdf:resource="http://www.w3id.org/efro/efro#hasLearningAim"/>
        <rdfs:domain rdf:resource="http://www.w3id.org/efro/efro#StudyProgramme"/>
        <rdfs:range rdf:resource="http://www.w3id.org/efro/efro#QualificationAim"/>
        <dcterms:description xml:lang="en">Represents learning that leads to an accredited qualification, such as A-levels, vocational diplomas, or apprenticeships.</dcterms:description>
        <rdfs:label>hasQualificationAim</rdfs:label>
    </owl:ObjectProperty>
    


    <!-- http://www.w3id.org/efro/efro#hasQualifyingPeriod -->

    <owl:ObjectProperty rdf:about="http://www.w3id.org/efro/efro#hasQualifyingPeriod">
        <rdfs:subPropertyOf rdf:resource="http://www.w3id.org/efro/efro#hasFundingCondition"/>
        <rdfs:domain rdf:resource="http://www.w3id.org/efro/efro#StudyProgramme"/>
        <rdfs:range rdf:resource="http://www.w3id.org/efro/efro#QualifyingPeriod"/>
        <dcterms:description xml:lang="en">Specifies the required duration a student must be enrolled before qualifying for funding​.</dcterms:description>
        <rdfs:label>hasQualifyingPeriod</rdfs:label>
    </owl:ObjectProperty>
    


    <!-- http://www.w3id.org/efro/efro#hasQualifyingPeriodAttendance -->

    <owl:ObjectProperty rdf:about="http://www.w3id.org/efro/efro#hasQualifyingPeriodAttendance">
        <rdfs:subPropertyOf rdf:resource="http://www.w3id.org/efro/efro#hasAttendanceRecord"/>
        <rdfs:domain rdf:resource="http://www.w3id.org/efro/efro#FullTimeStudent"/>
        <rdfs:range rdf:resource="http://www.w3id.org/efro/efro#QualifyingAttendanceActivity"/>
        <dcterms:description xml:lang="en">Represents attendance during the initial funding-qualifying period to determine if a student remains eligible for financial support.</dcterms:description>
        <rdfs:label>hasQualifyingPeriodAttendance</rdfs:label>
    </owl:ObjectProperty>
    


    <!-- http://www.w3id.org/efro/efro#hasReason -->

    <owl:ObjectProperty rdf:about="http://www.w3id.org/efro/efro#hasReason">
        <rdfs:domain rdf:resource="http://www.w3id.org/efro/efro#Activity"/>
        <rdfs:range rdf:resource="http://www.w3id.org/efro/efro#Reason"/>
        <rdfs:label>has reason</rdfs:label>
    </owl:ObjectProperty>
    


    <!-- http://www.w3id.org/efro/efro#hasRecordedPlannedHours -->

    <owl:ObjectProperty rdf:about="http://www.w3id.org/efro/efro#hasRecordedPlannedHours">
        <rdfs:subPropertyOf rdf:resource="http://www.w3id.org/efro/efro#hasPlannedHoursManagement"/>
        <rdfs:domain rdf:resource="http://www.w3id.org/efro/efro#Learning"/>
        <rdfs:range rdf:resource="http://www.w3id.org/efro/efro#RecordedPlannedHours"/>
        <dcterms:description xml:lang="en">Represents the hours officially recorded for funding claims, which may differ from initial planned hours due to changes.</dcterms:description>
        <rdfs:label>hasRecordedPlannedHours</rdfs:label>
    </owl:ObjectProperty>
    


    <!-- http://www.w3id.org/efro/efro#hasReplacementActivity -->

    <owl:ObjectProperty rdf:about="http://www.w3id.org/efro/efro#hasReplacementActivity">
        <owl:inverseOf rdf:resource="http://www.w3id.org/efro/efro#isReplacementActivityOf"/>
        <rdfs:domain rdf:resource="http://www.w3id.org/efro/efro#WithdrawalActivity"/>
        <rdfs:range rdf:resource="http://www.w3id.org/efro/efro#LearningAim"/>
        <dcterms:description xml:lang="en">Represents an alternative learning activity assigned when a student cannot complete the originally planned activity​.</dcterms:description>
        <rdfs:label>hasReplacementActivity</rdfs:label>
    </owl:ObjectProperty>
    


    <!-- http://www.w3id.org/efro/efro#hasReportingDuty -->

    <owl:ObjectProperty rdf:about="http://www.w3id.org/efro/efro#hasReportingDuty">
        <rdfs:subPropertyOf rdf:resource="http://www.w3id.org/efro/efro#hasLegalDuty"/>
        <rdfs:domain rdf:resource="http://www.w3id.org/efro/efro#EducationalEntity"/>
        <rdfs:range rdf:resource="http://www.w3id.org/efro/efro#ReportingObligation"/>
        <dcterms:description xml:lang="en">Represents the obligation to submit accurate data and compliance reports to funding bodies.</dcterms:description>
        <rdfs:label>hasReportingDuty</rdfs:label>
    </owl:ObjectProperty>
    


    <!-- http://www.w3id.org/efro/efro#hasRetainedStatus -->

    <owl:ObjectProperty rdf:about="http://www.w3id.org/efro/efro#hasRetainedStatus">
        <rdfs:subPropertyOf rdf:resource="http://www.w3id.org/efro/efro#hasParticipationStatus"/>
        <rdfs:domain rdf:resource="http://www.w3id.org/efro/efro#Student"/>
        <rdfs:range rdf:resource="http://www.w3id.org/efro/efro#RetainedStatus"/>
        <dcterms:description xml:lang="en">Represents a student who has remained enrolled in their programme without withdrawing or failing to meet attendance requirements.</dcterms:description>
        <rdfs:label>hasRetainedStatus</rdfs:label>
    </owl:ObjectProperty>
    


    <!-- http://www.w3id.org/efro/efro#hasRetentionFactor -->

    <owl:ObjectProperty rdf:about="http://www.w3id.org/efro/efro#hasRetentionFactor">
        <rdfs:subPropertyOf rdf:resource="http://www.w3id.org/efro/efro#hasFundingCondition"/>
        <rdfs:domain rdf:resource="http://www.w3id.org/efro/efro#FundingElement"/>
        <rdfs:range rdf:resource="http://www.w3id.org/efro/efro#RetentionFactor"/>
        <dcterms:description xml:lang="en">Represents the funding adjustment based on student retention, incentivizing institutions to support student completion.</dcterms:description>
        <rdfs:label>hasRetentionFactor</rdfs:label>
    </owl:ObjectProperty>
    


    <!-- http://www.w3id.org/efro/efro#hasServiceType -->

    <owl:ObjectProperty rdf:about="http://www.w3id.org/efro/efro#hasServiceType">
        <rdfs:domain rdf:resource="http://purl.org/cerif/frapo/Service"/>
        <rdfs:range rdf:resource="http://www.w3id.org/efro/efro#LearningAspect"/>
        <rdfs:label>hasServiceType</rdfs:label>
    </owl:ObjectProperty>
    


    <!-- http://www.w3id.org/efro/efro#hasStatus -->

    <owl:ObjectProperty rdf:about="http://www.w3id.org/efro/efro#hasStatus">
        <owl:inverseOf rdf:resource="http://www.w3id.org/efro/efro#isStatusOf"/>
        <rdfs:domain>
            <owl:Class>
                <owl:unionOf rdf:parseType="Collection">
                    <rdf:Description rdf:about="http://www.w3id.org/efro/efro#CompletionStatus"/>
                    <rdf:Description rdf:about="http://www.w3id.org/efro/efro#Learning"/>
                    <rdf:Description rdf:about="http://www.w3id.org/efro/efro#Person"/>
                </owl:unionOf>
            </owl:Class>
        </rdfs:domain>
        <rdfs:range rdf:resource="http://www.w3id.org/efro/efro#Status"/>
        <dcterms:description xml:lang="en">Links an entity (student, programme, or funding allocation) to its current operational status​.</dcterms:description>
        <rdfs:label>hasStatus</rdfs:label>
    </owl:ObjectProperty>
    


    <!-- http://www.w3id.org/efro/efro#hasSuccessfulCompletion -->

    <owl:ObjectProperty rdf:about="http://www.w3id.org/efro/efro#hasSuccessfulCompletion">
        <rdfs:subPropertyOf rdf:resource="http://www.w3id.org/efro/efro#hasAchievementStatus"/>
        <rdfs:domain rdf:resource="http://www.w3id.org/efro/efro#AchievementStatus"/>
        <rdfs:range rdf:resource="http://www.w3id.org/efro/efro#SuccessfulCompletionStatus"/>
        <dcterms:description xml:lang="en">Denotes that a student has successfully completed their study programme or qualification as per funding regulations.</dcterms:description>
        <rdfs:label>hasSuccessfulCompletion</rdfs:label>
    </owl:ObjectProperty>
    


    <!-- http://www.w3id.org/efro/efro#hasSustainableEmployment -->

    <owl:ObjectProperty rdf:about="http://www.w3id.org/efro/efro#hasSustainableEmployment">
        <rdfs:subPropertyOf rdf:resource="http://www.w3id.org/efro/efro#hasAchievementStatus"/>
        <rdfs:domain rdf:resource="http://www.w3id.org/efro/efro#AchievementStatus"/>
        <rdfs:range rdf:resource="http://www.w3id.org/efro/efro#SustainableEmploymentStatus"/>
        <dcterms:description xml:lang="en">Represents an outcome where a student transitions into stable employment after completing their educational programme.</dcterms:description>
        <rdfs:label>hasSustainableEmployment</rdfs:label>
    </owl:ObjectProperty>
    


    <!-- http://www.w3id.org/efro/efro#hasTerm -->

    <owl:ObjectProperty rdf:about="http://www.w3id.org/efro/efro#hasTerm">
        <rdfs:domain>
            <owl:Class>
                <owl:unionOf rdf:parseType="Collection">
                    <rdf:Description rdf:about="http://www.w3id.org/efro/efro#LearningAim"/>
                    <rdf:Description rdf:about="http://www.w3id.org/efro/efro#QualificationAim"/>
                </owl:unionOf>
            </owl:Class>
        </rdfs:domain>
        <rdfs:range rdf:resource="http://www.w3id.org/efro/efro#SummerTerm"/>
        <dcterms:description xml:lang="en">Represents the academic or funding term associated with a student’s enrolment and funding eligibility.</dcterms:description>
        <rdfs:label>hasTerm</rdfs:label>
    </owl:ObjectProperty>
    


    <!-- http://www.w3id.org/efro/efro#hasTimePeriod -->

    <owl:ObjectProperty rdf:about="http://www.w3id.org/efro/efro#hasTimePeriod">
        <owl:inverseOf rdf:resource="http://www.w3id.org/efro/efro#isTimePeriodOf"/>
        <rdfs:domain>
            <owl:Class>
                <owl:unionOf rdf:parseType="Collection">
                    <rdf:Description rdf:about="http://www.w3id.org/efro/efro#Activity"/>
                    <rdf:Description rdf:about="http://www.w3id.org/efro/efro#FundingElement"/>
                    <rdf:Description rdf:about="http://www.w3id.org/efro/efro#Learning"/>
                </owl:unionOf>
            </owl:Class>
        </rdfs:domain>
        <rdfs:range rdf:resource="http://www.w3id.org/efro/efro#TimeRelated"/>
        <dcterms:description xml:lang="en">Specifies the duration for which a funding allocation, learning programme, or enrolment is valid.</dcterms:description>
        <rdfs:label>hasTimePeriod</rdfs:label>
    </owl:ObjectProperty>
    


    <!-- http://www.w3id.org/efro/efro#hasTraditionalProvision -->

    <owl:ObjectProperty rdf:about="http://www.w3id.org/efro/efro#hasTraditionalProvision">
        <rdfs:subPropertyOf rdf:resource="http://www.w3id.org/efro/efro#hasLearningMode"/>
        <rdfs:domain>
            <owl:Class>
                <owl:unionOf rdf:parseType="Collection">
                    <rdf:Description rdf:about="http://www.w3id.org/efro/efro#Learning"/>
                    <rdf:Description rdf:about="http://www.w3id.org/efro/efro#Student"/>
                </owl:unionOf>
            </owl:Class>
        </rdfs:domain>
        <rdfs:range>
            <owl:Class>
                <owl:unionOf rdf:parseType="Collection">
                    <rdf:Description rdf:about="http://www.w3id.org/efro/efro#ProgressionActivity"/>
                    <rdf:Description rdf:about="http://www.w3id.org/efro/efro#TraditionalProvision"/>
                </owl:unionOf>
            </owl:Class>
        </rdfs:range>
        <dcterms:description xml:lang="en">Represents in-person, classroom-based learning models with scheduled instruction.</dcterms:description>
        <rdfs:label>hasTraditionalProvision</rdfs:label>
    </owl:ObjectProperty>
    


    <!-- http://www.w3id.org/efro/efro#hasTraineeshipFunding -->

    <owl:ObjectProperty rdf:about="http://www.w3id.org/efro/efro#hasTraineeshipFunding">
        <rdfs:subPropertyOf rdf:resource="http://www.w3id.org/efro/efro#hasFundingElement"/>
        <rdfs:domain>
            <owl:Class>
                <owl:unionOf rdf:parseType="Collection">
                    <rdf:Description rdf:about="http://www.w3id.org/efro/efro#Learning"/>
                    <rdf:Description rdf:about="http://www.w3id.org/efro/efro#Student"/>
                </owl:unionOf>
            </owl:Class>
        </rdfs:domain>
        <rdfs:range rdf:resource="http://www.w3id.org/efro/efro#TraineeshipFunding"/>
        <dcterms:description xml:lang="en">Specifies funding granted for traineeship programmes aimed at preparing students for apprenticeships or employment.</dcterms:description>
        <rdfs:label>hasTraineeshipFunding</rdfs:label>
    </owl:ObjectProperty>
    


    <!-- http://www.w3id.org/efro/efro#hasWeeklyLimit -->

    <owl:ObjectProperty rdf:about="http://www.w3id.org/efro/efro#hasWeeklyLimit">
        <rdfs:domain rdf:resource="http://www.w3id.org/efro/efro#PlannedHours"/>
        <rdfs:range rdf:resource="http://www.w3id.org/efro/efro#PlannedHours"/>
        <dcterms:description xml:lang="en">Defines the maximum allowable study hours per week for funding and enrolment purposes​.</dcterms:description>
        <rdfs:label>hasWeeklyLimit</rdfs:label>
    </owl:ObjectProperty>
    


    <!-- http://www.w3id.org/efro/efro#hasWithdrawalFromLearningAim -->

    <owl:ObjectProperty rdf:about="http://www.w3id.org/efro/efro#hasWithdrawalFromLearningAim">
        <rdfs:subPropertyOf rdf:resource="http://www.w3id.org/efro/efro#hasWithdrawalProcess"/>
        <owl:inverseOf rdf:resource="http://www.w3id.org/efro/efro#isWithdrawalFromLearningAimOf"/>
        <rdfs:domain rdf:resource="http://www.w3id.org/efro/efro#Student"/>
        <rdfs:range rdf:resource="http://www.w3id.org/efro/efro#WithdrawalFromLearningAim"/>
        <dcterms:description xml:lang="en">Denotes withdrawal from a single course or qualification within a broader study programme.</dcterms:description>
        <rdfs:label>hasWithdrawalFromLearningAim</rdfs:label>
    </owl:ObjectProperty>
    


    <!-- http://www.w3id.org/efro/efro#hasWithdrawalFromStudyProgramme -->

    <owl:ObjectProperty rdf:about="http://www.w3id.org/efro/efro#hasWithdrawalFromStudyProgramme">
        <rdfs:subPropertyOf rdf:resource="http://www.w3id.org/efro/efro#hasWithdrawalProcess"/>
        <owl:inverseOf rdf:resource="http://www.w3id.org/efro/efro#isWithdrawalFromStudyProgrammeOf"/>
        <rdfs:domain rdf:resource="http://www.w3id.org/efro/efro#Student"/>
        <rdfs:range rdf:resource="http://www.w3id.org/efro/efro#WithdrawalFromStudyProgramme"/>
        <dcterms:description xml:lang="en">Represents withdrawal from a structured programme that includes multiple learning aims.</dcterms:description>
        <rdfs:label>hasWithdrawalFromStudyProgramme</rdfs:label>
    </owl:ObjectProperty>
    


    <!-- http://www.w3id.org/efro/efro#hasWithdrawalFromWholeProgramme -->

    <owl:ObjectProperty rdf:about="http://www.w3id.org/efro/efro#hasWithdrawalFromWholeProgramme">
        <rdfs:subPropertyOf rdf:resource="http://www.w3id.org/efro/efro#hasWithdrawalProcess"/>
        <owl:inverseOf rdf:resource="http://www.w3id.org/efro/efro#isWithdrawalFromWholeProgrammeOf"/>
        <rdfs:domain rdf:resource="http://www.w3id.org/efro/efro#Student"/>
        <rdfs:range rdf:resource="http://www.w3id.org/efro/efro#WithdrawalFromWholeProgramme"/>
        <dcterms:description xml:lang="en">Indicates complete withdrawal from an institution, ceasing all learning activities.</dcterms:description>
        <rdfs:label>hasWithdrawalFromWholeProgramme</rdfs:label>
    </owl:ObjectProperty>
    


    <!-- http://www.w3id.org/efro/efro#hasWithdrawalProcess -->

    <owl:ObjectProperty rdf:about="http://www.w3id.org/efro/efro#hasWithdrawalProcess">
        <rdfs:domain rdf:resource="http://www.w3id.org/efro/efro#Student"/>
        <rdfs:range rdf:resource="http://www.w3id.org/efro/efro#WithdrawalActivity"/>
        <dcterms:description xml:lang="en">Represents the formal process of student withdrawal from individual learning aims, study programmes, or entire educational enrollment.</dcterms:description>
        <rdfs:label>hasWithdrawalProcess</rdfs:label>
    </owl:ObjectProperty>
    


    <!-- http://www.w3id.org/efro/efro#hasWithdrawalReason -->

    <owl:ObjectProperty rdf:about="http://www.w3id.org/efro/efro#hasWithdrawalReason">
        <owl:inverseOf rdf:resource="http://www.w3id.org/efro/efro#isWithdrawalReasonFor"/>
        <rdfs:domain rdf:resource="http://www.w3id.org/efro/efro#WithdrawalActivity"/>
        <rdfs:range rdf:resource="http://www.w3id.org/efro/efro#WithdrawalReason"/>
        <dcterms:description xml:lang="en">Captures the reasons why a student withdraws from a course, study programme, or institution.</dcterms:description>
        <rdfs:label>hasWithdrawalReason</rdfs:label>
    </owl:ObjectProperty>
    


    <!-- http://www.w3id.org/efro/efro#hasWithdrawnAim -->

    <owl:ObjectProperty rdf:about="http://www.w3id.org/efro/efro#hasWithdrawnAim">
        <rdfs:subPropertyOf rdf:resource="http://www.w3id.org/efro/efro#hasLearningAim"/>
        <owl:inverseOf rdf:resource="http://www.w3id.org/efro/efro#isWithdrawnAimOf"/>
        <rdf:type rdf:resource="http://www.w3.org/2002/07/owl#InverseFunctionalProperty"/>
        <rdfs:domain rdf:resource="http://www.w3id.org/efro/efro#StudyProgramme"/>
        <rdfs:range rdf:resource="http://www.w3id.org/efro/efro#WithdrawnQualification"/>
        <dcterms:description xml:lang="en">Indicates a learning aim that a student started but did not complete, potentially impacting funding eligibility.</dcterms:description>
        <rdfs:label>hasWithdrawnAim</rdfs:label>
    </owl:ObjectProperty>
    


    <!-- http://www.w3id.org/efro/efro#hasWithdrawnFromProgramme -->

    <owl:ObjectProperty rdf:about="http://www.w3id.org/efro/efro#hasWithdrawnFromProgramme">
        <rdfs:domain rdf:resource="http://www.w3id.org/efro/efro#Student"/>
        <rdfs:range rdf:resource="http://www.w3id.org/efro/efro#StudyProgramme"/>
        <dcterms:description xml:lang="en">Represents the relationship between a student and the programme they have withdrawn from, impacting funding eligibility.</dcterms:description>
        <rdfs:label>hasWithdrawnFromProgramme</rdfs:label>
    </owl:ObjectProperty>
    


    <!-- http://www.w3id.org/efro/efro#hasWithdrawnStatus -->

    <owl:ObjectProperty rdf:about="http://www.w3id.org/efro/efro#hasWithdrawnStatus">
        <rdfs:subPropertyOf rdf:resource="http://www.w3id.org/efro/efro#hasParticipationStatus"/>
        <rdfs:domain rdf:resource="http://www.w3id.org/efro/efro#Student"/>
        <rdfs:range rdf:resource="http://www.w3id.org/efro/efro#WithdrawnStatus"/>
        <dcterms:description xml:lang="en">Denotes that a student has withdrawn from their learning programme, which may impact funding retention.</dcterms:description>
        <rdfs:label>hasWithdrawnStatus</rdfs:label>
    </owl:ObjectProperty>
    


    <!-- http://www.w3id.org/efro/efro#includes -->

    <owl:ObjectProperty rdf:about="http://www.w3id.org/efro/efro#includes">
        <rdfs:domain rdf:resource="http://www.w3id.org/efro/efro#EducationalEntity"/>
        <rdfs:range>
            <owl:Class>
                <owl:unionOf rdf:parseType="Collection">
                    <rdf:Description rdf:about="http://www.w3id.org/efro/efro#Learning"/>
                    <rdf:Description rdf:about="http://www.w3id.org/efro/efro#Person"/>
                </owl:unionOf>
            </owl:Class>
        </rdfs:range>
        <dcterms:description xml:lang="en">Indicates that a programme, funding scheme, or learning activity contains certain components or sub-programmes​.</dcterms:description>
        <rdfs:label>includes</rdfs:label>
    </owl:ObjectProperty>
    


    <!-- http://www.w3id.org/efro/efro#isAssessmentRecord -->

    <owl:ObjectProperty rdf:about="http://www.w3id.org/efro/efro#isAssessmentRecord">
        <rdfs:subPropertyOf rdf:resource="http://www.w3id.org/efro/efro#hasAssessmentRecord"/>
        <rdf:type rdf:resource="http://www.w3.org/2002/07/owl#FunctionalProperty"/>
        <rdfs:domain rdf:resource="http://www.w3id.org/efro/efro#AssessmentActivity"/>
        <rdfs:range rdf:resource="http://www.w3id.org/efro/efro#Student"/>
        <dcterms:description xml:lang="en">Defines a particular record as an official assessment document related to a student’s academic performance​.</dcterms:description>
        <rdfs:label>isAssessmentRecord</rdfs:label>
    </owl:ObjectProperty>
    


    <!-- http://www.w3id.org/efro/efro#isAssistanceProvidedBy -->

    <owl:ObjectProperty rdf:about="http://www.w3id.org/efro/efro#isAssistanceProvidedBy">
        <rdfs:subPropertyOf rdf:resource="http://www.w3id.org/efro/efro#providesAssistance"/>
        <owl:inverseOf rdf:resource="http://www.w3id.org/efro/efro#providesAssistance"/>
        <rdfs:domain rdf:resource="http://www.w3id.org/efro/efro#Activity"/>
        <rdfs:range rdf:resource="http://www.w3id.org/efro/efro#EducationalEntity"/>
        <dcterms:description xml:lang="en">Identifies the entity (e.g., institution, funding body, support service) responsible for providing assistance.</dcterms:description>
        <rdfs:label>isAssistanceProvidedBy</rdfs:label>
    </owl:ObjectProperty>
    


    <!-- http://www.w3id.org/efro/efro#isAttendanceRecordOf -->

    <owl:ObjectProperty rdf:about="http://www.w3id.org/efro/efro#isAttendanceRecordOf">
        <rdfs:subPropertyOf rdf:resource="http://www.w3id.org/efro/efro#hasAttendanceRecord"/>
        <rdf:type rdf:resource="http://www.w3.org/2002/07/owl#InverseFunctionalProperty"/>
        <rdfs:domain rdf:resource="http://www.w3id.org/efro/efro#AttendanceActivity"/>
        <rdfs:range rdf:resource="http://www.w3id.org/efro/efro#Student"/>
        <dcterms:description xml:lang="en">Establishes that an attendance record belongs to a particular student or study programme.</dcterms:description>
        <rdfs:label>isAttendanceRecordOf</rdfs:label>
    </owl:ObjectProperty>
    


    <!-- http://www.w3id.org/efro/efro#isComplianceRequirementFor -->

    <owl:ObjectProperty rdf:about="http://www.w3id.org/efro/efro#isComplianceRequirementFor">
        <rdfs:subPropertyOf rdf:resource="http://www.w3id.org/efro/efro#hasLegalDuty"/>
        <rdfs:domain rdf:resource="http://www.w3id.org/efro/efro#ComplianceObligation"/>
        <rdfs:range rdf:resource="http://www.w3id.org/efro/efro#FundedInstitution"/>
        <dcterms:description xml:lang="en">Establishes a relationship between compliance requirements and the specific funding schemes they apply to.</dcterms:description>
        <rdfs:label>isComplianceRequirementFor</rdfs:label>
    </owl:ObjectProperty>
    


    <!-- http://www.w3id.org/efro/efro#isDocumentationRequiredBy -->

    <owl:ObjectProperty rdf:about="http://www.w3id.org/efro/efro#isDocumentationRequiredBy">
        <owl:inverseOf rdf:resource="http://www.w3id.org/efro/efro#requiresDocumentation"/>
        <rdfs:domain rdf:resource="http://www.w3id.org/efro/efro#Document"/>
        <rdfs:range rdf:resource="http://www.w3id.org/efro/efro#Obligation"/>
        <dcterms:description xml:lang="en">Specifies the entity (e.g., funding agency, institution) that requires specific documentation for compliance or audit purposes​.</dcterms:description>
        <rdfs:label>isDocumentationRequiredBy</rdfs:label>
    </owl:ObjectProperty>
    


    <!-- http://www.w3id.org/efro/efro#isFundedBy -->

    <owl:ObjectProperty rdf:about="http://www.w3id.org/efro/efro#isFundedBy">
        <rdfs:domain rdf:resource="http://www.w3id.org/efro/efro#FundingElement"/>
        <rdfs:range>
            <owl:Class>
                <owl:unionOf rdf:parseType="Collection">
                    <rdf:Description rdf:about="http://www.w3id.org/efro/efro#EducationalEntity"/>
                    <rdf:Description rdf:about="http://www.w3id.org/efro/efro#Learning"/>
                </owl:unionOf>
            </owl:Class>
        </rdfs:range>
        <dcterms:description xml:lang="en">Represents the funding source that provides financial support to a student, institution, or programme​.</dcterms:description>
        <rdfs:label>isFundedBy</rdfs:label>
    </owl:ObjectProperty>
    


    <!-- http://www.w3id.org/efro/efro#isFundingObligationFor -->

    <owl:ObjectProperty rdf:about="http://www.w3id.org/efro/efro#isFundingObligationFor">
        <rdfs:subPropertyOf rdf:resource="http://www.w3id.org/efro/efro#hasLegalDuty"/>
        <rdfs:domain rdf:resource="http://www.w3id.org/efro/efro#FundingObligation"/>
        <rdfs:range rdf:resource="http://www.w3id.org/efro/efro#FundedInstitution"/>
        <dcterms:description xml:lang="en">Links funding obligations to the specific programmes or institutions that must meet them.</dcterms:description>
        <rdfs:label>isFundingObligationFor</rdfs:label>
    </owl:ObjectProperty>
    


    <!-- http://www.w3id.org/efro/efro#isProgressionStatusOf -->

    <owl:ObjectProperty rdf:about="http://www.w3id.org/efro/efro#isProgressionStatusOf">
        <rdfs:subPropertyOf rdf:resource="http://www.w3id.org/efro/efro#isAssessmentRecord"/>
        <rdf:type rdf:resource="http://www.w3.org/2002/07/owl#FunctionalProperty"/>
        <rdfs:domain rdf:resource="http://www.w3id.org/efro/efro#ProgressionActivity"/>
        <rdfs:range rdf:resource="http://www.w3id.org/efro/efro#Student"/>
        <dcterms:description xml:lang="en">Establishes a link between a student’s academic status and their overall progression in the learning programme.</dcterms:description>
        <rdfs:label>isProgressionStatusOf</rdfs:label>
    </owl:ObjectProperty>
    


    <!-- http://www.w3id.org/efro/efro#isReasonFor -->

    <owl:ObjectProperty rdf:about="http://www.w3id.org/efro/efro#isReasonFor">
        <rdfs:domain rdf:resource="http://www.w3id.org/efro/efro#Reason"/>
        <rdfs:range rdf:resource="http://www.w3id.org/efro/efro#Activity"/>
        <dcterms:description xml:lang="en">Indicates a cause-and-effect relationship where a specific condition (e.g., attendance issues) is the reason for an outcome (e.g., funding reduction).</dcterms:description>
        <rdfs:label>isReasonFor</rdfs:label>
    </owl:ObjectProperty>
    


    <!-- http://www.w3id.org/efro/efro#isReplacementActivityOf -->

    <owl:ObjectProperty rdf:about="http://www.w3id.org/efro/efro#isReplacementActivityOf">
        <rdfs:domain rdf:resource="http://www.w3id.org/efro/efro#LearningAim"/>
        <rdfs:range rdf:resource="http://www.w3id.org/efro/efro#WithdrawalActivity"/>
        <dcterms:description xml:lang="en">Identifies the original activity that has been replaced by an alternative due to changes in student circumstances​.</dcterms:description>
        <rdfs:label>isReplacementActivityOf</rdfs:label>
    </owl:ObjectProperty>
    


    <!-- http://www.w3id.org/efro/efro#isStatusOf -->

    <owl:ObjectProperty rdf:about="http://www.w3id.org/efro/efro#isStatusOf">
        <rdfs:domain rdf:resource="http://www.w3id.org/efro/efro#Status"/>
        <rdfs:range>
            <owl:Class>
                <owl:unionOf rdf:parseType="Collection">
                    <rdf:Description rdf:about="http://www.w3id.org/efro/efro#CompletionStatus"/>
                    <rdf:Description rdf:about="http://www.w3id.org/efro/efro#Learning"/>
                    <rdf:Description rdf:about="http://www.w3id.org/efro/efro#Person"/>
                </owl:unionOf>
            </owl:Class>
        </rdfs:range>
        <dcterms:description xml:lang="en">Defines the status of an entity, such as funding eligibility, enrolment, or completion status​.</dcterms:description>
        <rdfs:label>isStatusOf</rdfs:label>
    </owl:ObjectProperty>
    


    <!-- http://www.w3id.org/efro/efro#isStatusResultingFrom -->

    <owl:ObjectProperty rdf:about="http://www.w3id.org/efro/efro#isStatusResultingFrom">
        <owl:inverseOf rdf:resource="http://www.w3id.org/efro/efro#resultsInStatus"/>
        <rdfs:domain rdf:resource="http://www.w3id.org/efro/efro#Status"/>
        <rdfs:range rdf:resource="http://www.w3id.org/efro/efro#Reason"/>
        <dcterms:description xml:lang="en">Captures the cause of a status change, such as withdrawal due to non-attendance.</dcterms:description>
        <rdfs:label>isStatusResultingFrom</rdfs:label>
    </owl:ObjectProperty>
    


    <!-- http://www.w3id.org/efro/efro#isTimePeriodOf -->

    <owl:ObjectProperty rdf:about="http://www.w3id.org/efro/efro#isTimePeriodOf">
        <rdfs:domain rdf:resource="http://www.w3id.org/efro/efro#TimeRelated"/>
        <rdfs:range>
            <owl:Class>
                <owl:unionOf rdf:parseType="Collection">
                    <rdf:Description rdf:about="http://www.w3id.org/efro/efro#Activity"/>
                    <rdf:Description rdf:about="http://www.w3id.org/efro/efro#FundingElement"/>
                    <rdf:Description rdf:about="http://www.w3id.org/efro/efro#Learning"/>
                </owl:unionOf>
            </owl:Class>
        </rdfs:range>
        <dcterms:description xml:lang="en">Links a time period to the entity it applies to, such as a funding year or academic term​.</dcterms:description>
        <rdfs:label>isTimePeriodOf</rdfs:label>
    </owl:ObjectProperty>
    


    <!-- http://www.w3id.org/efro/efro#isWithdrawalFromLearningAimOf -->

    <owl:ObjectProperty rdf:about="http://www.w3id.org/efro/efro#isWithdrawalFromLearningAimOf">
        <rdfs:subPropertyOf rdf:resource="http://www.w3id.org/efro/efro#hasWithdrawalProcess"/>
        <rdfs:domain rdf:resource="http://www.w3id.org/efro/efro#WithdrawalFromLearningAim"/>
        <rdfs:range rdf:resource="http://www.w3id.org/efro/efro#Student"/>
        <dcterms:description xml:lang="en">Establishes a link between a withdrawal process and the specific learning aim it applies to.</dcterms:description>
        <rdfs:label>isWithdrawalFromLearningAimOf</rdfs:label>
    </owl:ObjectProperty>
    


    <!-- http://www.w3id.org/efro/efro#isWithdrawalFromStudyProgrammeOf -->

    <owl:ObjectProperty rdf:about="http://www.w3id.org/efro/efro#isWithdrawalFromStudyProgrammeOf">
        <rdfs:subPropertyOf rdf:resource="http://www.w3id.org/efro/efro#hasWithdrawalProcess"/>
        <rdfs:domain rdf:resource="http://www.w3id.org/efro/efro#WithdrawalFromStudyProgramme"/>
        <rdfs:range rdf:resource="http://www.w3id.org/efro/efro#Student"/>
        <dcterms:description xml:lang="en">Associates a withdrawal process with the study programme it affects.</dcterms:description>
        <rdfs:label>isWithdrawalFromStudyProgrammeOf</rdfs:label>
    </owl:ObjectProperty>
    


    <!-- http://www.w3id.org/efro/efro#isWithdrawalFromWholeProgrammeOf -->

    <owl:ObjectProperty rdf:about="http://www.w3id.org/efro/efro#isWithdrawalFromWholeProgrammeOf">
        <rdfs:subPropertyOf rdf:resource="http://www.w3id.org/efro/efro#hasWithdrawalProcess"/>
        <rdfs:domain rdf:resource="http://www.w3id.org/efro/efro#WithdrawalFromWholeProgramme"/>
        <rdfs:range rdf:resource="http://www.w3id.org/efro/efro#Student"/>
        <dcterms:description xml:lang="en">Links a withdrawal process to the entire programme or institution.</dcterms:description>
        <rdfs:label>isWithdrawalFromWholeProgrammeOf</rdfs:label>
    </owl:ObjectProperty>
    


    <!-- http://www.w3id.org/efro/efro#isWithdrawalReasonFor -->

    <owl:ObjectProperty rdf:about="http://www.w3id.org/efro/efro#isWithdrawalReasonFor">
        <rdfs:subPropertyOf rdf:resource="http://www.w3id.org/efro/efro#hasWithdrawalReason"/>
        <rdfs:domain rdf:resource="http://www.w3id.org/efro/efro#WithdrawalReason"/>
        <rdfs:range rdf:resource="http://www.w3id.org/efro/efro#WithdrawalActivity"/>
        <dcterms:description xml:lang="en">Establishes a link between a specific reason and the withdrawal decision it influenced.</dcterms:description>
        <rdfs:label>isWithdrawalReasonFor</rdfs:label>
    </owl:ObjectProperty>
    


    <!-- http://www.w3id.org/efro/efro#isWithdrawnAimOf -->

    <owl:ObjectProperty rdf:about="http://www.w3id.org/efro/efro#isWithdrawnAimOf">
        <rdfs:subPropertyOf rdf:resource="http://www.w3id.org/efro/efro#hasLearningAim"/>
        <rdf:type rdf:resource="http://www.w3.org/2002/07/owl#FunctionalProperty"/>
        <rdfs:domain rdf:resource="http://www.w3id.org/efro/efro#WithdrawnQualification"/>
        <rdfs:range rdf:resource="http://www.w3id.org/efro/efro#StudyProgramme"/>
        <dcterms:description xml:lang="en">Establishes a relationship between a withdrawn learning aim and the specific student or programme it was part of.</dcterms:description>
        <rdfs:label>isWithdrawnAimOf</rdfs:label>
    </owl:ObjectProperty>
    


    <!-- http://www.w3id.org/efro/efro#modifies -->

    <owl:ObjectProperty rdf:about="http://www.w3id.org/efro/efro#modifies">
        <rdfs:domain rdf:resource="http://www.w3id.org/efro/efro#Status"/>
        <rdfs:range rdf:resource="http://www.w3id.org/efro/efro#FundingElement"/>
        <rdfs:label>modifies</rdfs:label>
    </owl:ObjectProperty>
    


    <!-- http://www.w3id.org/efro/efro#participatesIn -->

    <owl:ObjectProperty rdf:about="http://www.w3id.org/efro/efro#participatesIn">
        <rdfs:domain rdf:resource="http://www.w3id.org/efro/efro#Person"/>
        <rdfs:range rdf:resource="http://www.w3id.org/efro/efro#Activity"/>
        <dcterms:description xml:lang="en">Represents a student&apos;s or institution&apos;s involvement in a funded study programme or activity​.</dcterms:description>
        <rdfs:label>participatesIn</rdfs:label>
    </owl:ObjectProperty>
    


    <!-- http://www.w3id.org/efro/efro#performs -->

    <owl:ObjectProperty rdf:about="http://www.w3id.org/efro/efro#performs">
        <rdfs:label>performs</rdfs:label>
    </owl:ObjectProperty>
    


    <!-- http://www.w3id.org/efro/efro#progressedFrom -->

    <owl:ObjectProperty rdf:about="http://www.w3id.org/efro/efro#progressedFrom">
        <rdfs:domain rdf:resource="http://www.w3id.org/efro/efro#ProgressionActivity"/>
        <rdfs:range rdf:resource="http://www.w3id.org/efro/efro#StudyProgramme"/>
        <rdfs:comment>progressed from</rdfs:comment>
    </owl:ObjectProperty>
    


    <!-- http://www.w3id.org/efro/efro#progressedTo -->

    <owl:ObjectProperty rdf:about="http://www.w3id.org/efro/efro#progressedTo">
        <rdfs:domain rdf:resource="http://www.w3id.org/efro/efro#ProgressionActivity"/>
        <rdfs:comment>progressed to</rdfs:comment>
    </owl:ObjectProperty>
    


    <!-- http://www.w3id.org/efro/efro#providesAdministrativeAssistance -->

    <owl:ObjectProperty rdf:about="http://www.w3id.org/efro/efro#providesAdministrativeAssistance">
        <rdfs:subPropertyOf rdf:resource="http://www.w3id.org/efro/efro#providesAssistance"/>
        <owl:inverseOf rdf:resource="http://www.w3id.org/efro/efro#receivesAdministrativeAssistanceFrom"/>
        <rdfs:domain rdf:resource="http://www.w3id.org/efro/efro#EducationalEntity"/>
        <rdfs:range rdf:resource="http://www.w3id.org/efro/efro#AdministrativeActivity"/>
        <dcterms:description xml:lang="en">Covers support related to funding applications, enrollment processing, and compliance with regulations.</dcterms:description>
        <rdfs:label>providesAdministrativeAssistance</rdfs:label>
    </owl:ObjectProperty>
    


    <!-- http://www.w3id.org/efro/efro#providesAssistance -->

    <owl:ObjectProperty rdf:about="http://www.w3id.org/efro/efro#providesAssistance">
        <rdfs:domain rdf:resource="http://www.w3id.org/efro/efro#EducationalEntity"/>
        <rdfs:range rdf:resource="http://www.w3id.org/efro/efro#Activity"/>
        <dcterms:description xml:lang="en">Represents the various forms of support provided to students, institutions, or staff in relation to educational funding and study programmes.</dcterms:description>
        <rdfs:label>providesAssistance</rdfs:label>
    </owl:ObjectProperty>
    


    <!-- http://www.w3id.org/efro/efro#providesGeneralAssistance -->

    <owl:ObjectProperty rdf:about="http://www.w3id.org/efro/efro#providesGeneralAssistance">
        <rdfs:subPropertyOf rdf:resource="http://www.w3id.org/efro/efro#providesAssistance"/>
        <owl:inverseOf rdf:resource="http://www.w3id.org/efro/efro#receivesGeneralAssistanceFrom"/>
        <rdfs:domain rdf:resource="http://www.w3id.org/efro/efro#EducationalEntity"/>
        <rdfs:range rdf:resource="http://www.w3id.org/efro/efro#GeneralAdministrativeActivity"/>
        <dcterms:description xml:lang="en">Represents non-specialized support offered to students, such as academic guidance or welfare services.</dcterms:description>
        <rdfs:label>providesGeneralAssistance</rdfs:label>
    </owl:ObjectProperty>
    


    <!-- http://www.w3id.org/efro/efro#providesService -->

    <owl:ObjectProperty rdf:about="http://www.w3id.org/efro/efro#providesService">
        <rdfs:domain rdf:resource="http://purl.org/cerif/frapo/Service"/>
        <rdfs:range rdf:resource="http://www.w3id.org/efro/efro#Activity"/>
        <rdfs:label>providesService</rdfs:label>
    </owl:ObjectProperty>
    


    <!-- http://www.w3id.org/efro/efro#providesStudentSupport -->

    <owl:ObjectProperty rdf:about="http://www.w3id.org/efro/efro#providesStudentSupport">
        <rdfs:subPropertyOf rdf:resource="http://www.w3id.org/efro/efro#providesAssistance"/>
        <owl:inverseOf rdf:resource="http://www.w3id.org/efro/efro#receivesStudentSupportfrom"/>
        <rdfs:domain rdf:resource="http://www.w3id.org/efro/efro#EducationalEntity"/>
        <rdfs:range rdf:resource="http://www.w3id.org/efro/efro#SupportActivity"/>
        <dcterms:description>Denotes specific assistance aimed at students, including financial aid, learning accommodations, and career counseling.</dcterms:description>
        <rdfs:label>providesStudentSupport</rdfs:label>
    </owl:ObjectProperty>
    


    <!-- http://www.w3id.org/efro/efro#receivesAdministrativeAssistanceFrom -->

    <owl:ObjectProperty rdf:about="http://www.w3id.org/efro/efro#receivesAdministrativeAssistanceFrom">
        <rdfs:subPropertyOf rdf:resource="http://www.w3id.org/efro/efro#isAssistanceProvidedBy"/>
        <rdfs:domain rdf:resource="http://www.w3id.org/efro/efro#AdministrativeActivity"/>
        <rdfs:range rdf:resource="http://www.w3id.org/efro/efro#EducationalEntity"/>
        <dcterms:description xml:lang="en">Indicates that an institution, staff member, or student receives administrative support from a specific entity, such as a funding body, educational provider, or government agency.</dcterms:description>
        <rdfs:label>receivesAdministrativeAssistanceFrom</rdfs:label>
    </owl:ObjectProperty>
    


    <!-- http://www.w3id.org/efro/efro#receivesGeneralAssistanceFrom -->

    <owl:ObjectProperty rdf:about="http://www.w3id.org/efro/efro#receivesGeneralAssistanceFrom">
        <rdfs:subPropertyOf rdf:resource="http://www.w3id.org/efro/efro#isAssistanceProvidedBy"/>
        <rdfs:domain rdf:resource="http://www.w3id.org/efro/efro#GeneralAdministrativeActivity"/>
        <rdfs:range rdf:resource="http://www.w3id.org/efro/efro#EducationalEntity"/>
        <dcterms:description xml:lang="en">Represents the receipt of general, non-specialized support from an external source, which may include academic advice, career counseling, or general welfare services.</dcterms:description>
        <rdfs:label>receivesGeneralAssistanceFrom</rdfs:label>
    </owl:ObjectProperty>
    


    <!-- http://www.w3id.org/efro/efro#receivesStudentSupportfrom -->

    <owl:ObjectProperty rdf:about="http://www.w3id.org/efro/efro#receivesStudentSupportfrom">
        <rdfs:subPropertyOf rdf:resource="http://www.w3id.org/efro/efro#isAssistanceProvidedBy"/>
        <rdfs:domain rdf:resource="http://www.w3id.org/efro/efro#SupportActivity"/>
        <rdfs:range rdf:resource="http://www.w3id.org/efro/efro#EducationalEntity"/>
        <dcterms:description xml:lang="en">Specifies that a student receives targeted support from a designated entity, such as financial aid offices, learning support teams, or mental health services.</dcterms:description>
        <rdfs:label>receivesStudentSupportfrom</rdfs:label>
    </owl:ObjectProperty>
    


    <!-- http://www.w3id.org/efro/efro#recordedIn -->

    <owl:ObjectProperty rdf:about="http://www.w3id.org/efro/efro#recordedIn">
        <rdfs:subPropertyOf rdf:resource="http://www.w3.org/2002/07/owl#topObjectProperty"/>
        <rdfs:domain rdf:resource="http://www.w3id.org/efro/efro#Activity"/>
        <rdfs:range rdf:resource="http://www.w3id.org/efro/efro#Evidence"/>
    </owl:ObjectProperty>
    


    <!-- http://www.w3id.org/efro/efro#relatedToAdjustedPlannedHours -->

    <owl:ObjectProperty rdf:about="http://www.w3id.org/efro/efro#relatedToAdjustedPlannedHours">
        <rdfs:subPropertyOf rdf:resource="http://www.w3id.org/efro/efro#hasPlannedHours"/>
        <rdfs:domain>
            <owl:Class>
                <owl:unionOf rdf:parseType="Collection">
                    <rdf:Description rdf:about="http://www.w3id.org/efro/efro#Learning"/>
                    <rdf:Description rdf:about="http://www.w3id.org/efro/efro#StudyProgramme"/>
                </owl:unionOf>
            </owl:Class>
        </rdfs:domain>
        <rdfs:range rdf:resource="http://www.w3id.org/efro/efro#AdjustedPlannedHours"/>
        <dcterms:description xml:lang="en">Establishes a relationship between the initially planned hours and any adjustments made due to changes in student circumstances (e.g., withdrawals, reduced study load).</dcterms:description>
        <rdfs:label>relatedToAdjustedPlannedHours</rdfs:label>
    </owl:ObjectProperty>
    


    <!-- http://www.w3id.org/efro/efro#relatedToExcludedHours -->

    <owl:ObjectProperty rdf:about="http://www.w3id.org/efro/efro#relatedToExcludedHours">
        <rdfs:subPropertyOf rdf:resource="http://www.w3id.org/efro/efro#hasPlannedHoursManagement"/>
        <rdfs:domain>
            <owl:Class>
                <owl:unionOf rdf:parseType="Collection">
                    <rdf:Description rdf:about="http://www.w3id.org/efro/efro#Learning"/>
                    <rdf:Description rdf:about="http://www.w3id.org/efro/efro#PlannedHours"/>
                </owl:unionOf>
            </owl:Class>
        </rdfs:domain>
        <rdfs:range rdf:resource="http://www.w3id.org/efro/efro#ExcludedHours"/>
        <dcterms:description xml:lang="en">Links planned hours to those excluded from funding eligibility, such as non-qualifying activities or voluntary study sessions.</dcterms:description>
        <rdfs:label>relatedToExcludedHours</rdfs:label>
    </owl:ObjectProperty>
    


    <!-- http://www.w3id.org/efro/efro#relatedToFundingStatus -->

    <owl:ObjectProperty rdf:about="http://www.w3id.org/efro/efro#relatedToFundingStatus">
        <rdfs:domain>
            <owl:Class>
                <owl:unionOf rdf:parseType="Collection">
                    <rdf:Description rdf:about="http://www.w3id.org/efro/efro#FundingStatus"/>
                    <rdf:Description rdf:about="http://www.w3id.org/efro/efro#Student"/>
                </owl:unionOf>
            </owl:Class>
        </rdfs:domain>
        <rdfs:range rdf:resource="http://www.w3id.org/efro/efro#FundingStatus"/>
        <dcterms:description xml:lang="en">Links an entity to its funding status, such as active, pending, or withdrawn​.</dcterms:description>
        <rdfs:label>relatedToFundingStatus</rdfs:label>
    </owl:ObjectProperty>
    


    <!-- http://www.w3id.org/efro/efro#relatedToNonAttendanceReason -->

    <owl:ObjectProperty rdf:about="http://www.w3id.org/efro/efro#relatedToNonAttendanceReason">
        <rdfs:subPropertyOf rdf:resource="http://www.w3id.org/efro/efro#hasWithdrawalReason"/>
        <rdf:type rdf:resource="http://www.w3.org/2002/07/owl#FunctionalProperty"/>
        <rdfs:domain>
            <owl:Class>
                <owl:unionOf rdf:parseType="Collection">
                    <rdf:Description rdf:about="http://www.w3id.org/efro/efro#NonAttendanceActivity"/>
                    <rdf:Description rdf:about="http://www.w3id.org/efro/efro#WithdrawalActivity"/>
                </owl:unionOf>
            </owl:Class>
        </rdfs:domain>
        <rdfs:range rdf:resource="http://www.w3id.org/efro/efro#NonAttendanceReason"/>
        <dcterms:description xml:lang="en">Connects withdrawal reasons to non-attendance patterns that may have led to the withdrawal decision.</dcterms:description>
        <rdfs:label>relatedToNonAttendanceReason</rdfs:label>
    </owl:ObjectProperty>
    


    <!-- http://www.w3id.org/efro/efro#requires -->

    <owl:ObjectProperty rdf:about="http://www.w3id.org/efro/efro#requires">
        <rdfs:domain rdf:resource="http://www.w3id.org/efro/efro#FundingElement"/>
        <rdfs:range rdf:resource="http://www.w3id.org/efro/efro#Evidence"/>
    </owl:ObjectProperty>
    


    <!-- http://www.w3id.org/efro/efro#requiresDocumentation -->

    <owl:ObjectProperty rdf:about="http://www.w3id.org/efro/efro#requiresDocumentation">
        <rdfs:domain rdf:resource="http://www.w3id.org/efro/efro#Obligation"/>
        <rdfs:range rdf:resource="http://www.w3id.org/efro/efro#Document"/>
        <dcterms:description xml:lang="en">Specifies that a funding application, enrolment process, or audit requires specific documentation.</dcterms:description>
        <rdfs:label>requiresDocumentation</rdfs:label>
    </owl:ObjectProperty>


    <!-- http://www.w3id.org/efro/efro#regulatedBy -->

    <owl:ObjectProperty rdf:about="http://www.w3id.org/efro/efro#regulatedBy">
        <owl:inverseOf rdf:resource="http://www.w3id.org/efro/efro#regulates"/>
        <rdfs:domain rdf:resource="http://purl.org/vocab/aiiso/schema#Programme"/>
        <rdfs:range rdf:resource="http://www.w3id.org/efro/efro#FundingRegulations"/>
        <dcterms:description xml:lang="en">Links educational programmes to the funding regulations that govern their delivery, compliance requirements, and funding eligibility criteria.</dcterms:description>
        <rdfs:label>regulatedBy</rdfs:label>
    </owl:ObjectProperty>
    


    <!-- http://www.w3id.org/efro/efro#regulates -->

    <owl:ObjectProperty rdf:about="http://www.w3id.org/efro/efro#regulates">
        <owl:inverseOf rdf:resource="http://www.w3id.org/efro/efro#regulatedBy"/>
        <rdfs:domain rdf:resource="http://www.w3id.org/efro/efro#FundingRegulations"/>
        <rdfs:range rdf:resource="http://purl.org/vocab/aiiso/schema#Programme"/>
        <dcterms:description xml:lang="en">Indicates which educational programmes are governed by this funding regulation.</dcterms:description>
        <rdfs:label>regulates</rdfs:label>
    </owl:ObjectProperty>


    <!-- http://www.w3id.org/efro/efro#resets -->

    <owl:ObjectProperty rdf:about="http://www.w3id.org/efro/efro#resets">
        <rdfs:domain rdf:resource="http://www.w3id.org/efro/efro#Activity"/>
        <rdfs:range rdf:resource="http://www.w3id.org/efro/efro#LearningAim"/>
        <rdfs:label>resets</rdfs:label>
    </owl:ObjectProperty>
    


    <!-- http://www.w3id.org/efro/efro#resultsIn -->

    <owl:ObjectProperty rdf:about="http://www.w3id.org/efro/efro#resultsIn">
        <rdfs:domain rdf:resource="http://www.w3id.org/efro/efro#Activity"/>
        <rdfs:label>results in</rdfs:label>
    </owl:ObjectProperty>
    


    <!-- http://www.w3id.org/efro/efro#resultsInStatus -->

    <owl:ObjectProperty rdf:about="http://www.w3id.org/efro/efro#resultsInStatus">
        <rdfs:domain rdf:resource="http://www.w3id.org/efro/efro#Reason"/>
        <rdfs:range rdf:resource="http://www.w3id.org/efro/efro#Status"/>
        <dcterms:description xml:lang="en">Represents the outcome of a process, such as how non-attendance results in funding suspension.</dcterms:description>
        <rdfs:label>resultsInStatus</rdfs:label>
    </owl:ObjectProperty>
    


    <!-- http://www.w3id.org/efro/efro#supportsActivity -->

    <owl:ObjectProperty rdf:about="http://www.w3id.org/efro/efro#supportsActivity">
        <rdfs:domain rdf:resource="http://purl.org/cerif/frapo/Endeavour"/>
        <rdfs:range rdf:resource="http://www.w3id.org/efro/efro#Activity"/>
        <rdfs:label>supportsActivity</rdfs:label>
    </owl:ObjectProperty>
    


    <!-- http://www.w3id.org/efro/efro#supportsLearning -->

    <owl:ObjectProperty rdf:about="http://www.w3id.org/efro/efro#supportsLearning">
        <rdfs:domain rdf:resource="http://purl.org/cerif/frapo/InfrastructureEntity"/>
        <rdfs:range rdf:resource="http://www.w3id.org/efro/efro#Learning"/>
        <rdfs:label>supportsLearning</rdfs:label>
    </owl:ObjectProperty>
    


    <!-- http://www.w3id.org/efro/efro#tracksProgress -->

    <owl:ObjectProperty rdf:about="http://www.w3id.org/efro/efro#tracksProgress">
        <rdfs:domain rdf:resource="http://purl.org/cerif/frapo/Endeavour"/>
        <rdfs:range rdf:resource="http://www.w3id.org/efro/efro#Status"/>
        <rdfs:label>tracksProgress</rdfs:label>
    </owl:ObjectProperty>
    


    <!-- http://www.w3id.org/efro/efro#verifies -->

    <owl:ObjectProperty rdf:about="http://www.w3id.org/efro/efro#verifies"/>
    


    <!-- http://www.w3id.org/efro/efro#withdrawnFrom -->

    <owl:ObjectProperty rdf:about="http://www.w3id.org/efro/efro#withdrawnFrom">
        <rdfs:domain rdf:resource="http://www.w3id.org/efro/efro#WithdrawalActivity"/>
        <rdfs:range rdf:resource="http://www.w3id.org/efro/efro#LearningAim"/>
        <dcterms:description>Links withdrawal process to the specific learning aim being withdrawn from.</dcterms:description>
        <rdfs:label>withdrawnFrom</rdfs:label>
    </owl:ObjectProperty>
    


    <!-- 
    ///////////////////////////////////////////////////////////////////////////////////////
    //
    // Data properties
    //
    ///////////////////////////////////////////////////////////////////////////////////////
     -->

    


    <!-- http://purl.org/cerif/frapo/hasDegreeSuffix -->

    <owl:DatatypeProperty rdf:about="http://purl.org/cerif/frapo/hasDegreeSuffix">
        <rdfs:domain rdf:resource="http://www.w3id.org/efro/efro#Person"/>
        <rdfs:range rdf:resource="http://www.w3.org/2001/XMLSchema#string"/>
        <rdfs:comment xml:lang="en">The letters that should be displayed after a person&apos;s name to indicate an academic degree, e.g. BA, BVSc, PhD, DSc.</rdfs:comment>
        <rdfs:label xml:lang="en">has degrees</rdfs:label>
    </owl:DatatypeProperty>
    


    <!-- http://purl.org/cerif/frapo/hasPersonalInformation -->

    <owl:DatatypeProperty rdf:about="http://purl.org/cerif/frapo/hasPersonalInformation">
        <rdfs:subPropertyOf rdf:resource="http://purl.org/cerif/frapo/hasAgentInformation"/>
        <rdfs:domain>
            <owl:Class>
                <owl:unionOf rdf:parseType="Collection">
                    <rdf:Description rdf:about="http://www.w3id.org/efro/efro#EducationalEntity"/>
                    <rdf:Description rdf:about="http://xmlns.com/foaf/0.1/Agent"/>
                </owl:unionOf>
            </owl:Class>
        </rdfs:domain>
        <rdfs:range rdf:resource="http://www.w3.org/2001/XMLSchema#string"/>
        <rdfs:comment xml:lang="en">A data property linking a person to information about that person.</rdfs:comment>
        <rdfs:label xml:lang="en">has contact information</rdfs:label>
    </owl:DatatypeProperty>
    


    <!-- http://purl.org/cerif/frapo/hasPhoneNumber -->

    <owl:DatatypeProperty rdf:about="http://purl.org/cerif/frapo/hasPhoneNumber">
        <rdfs:subPropertyOf rdf:resource="http://purl.org/cerif/frapo/hasAgentInformation"/>
        <rdfs:domain>
            <owl:Class>
                <owl:unionOf rdf:parseType="Collection">
                    <rdf:Description rdf:about="http://www.w3id.org/efro/efro#EducationalEntity"/>
                    <rdf:Description rdf:about="http://xmlns.com/foaf/0.1/Agent"/>
                </owl:unionOf>
            </owl:Class>
        </rdfs:domain>
        <rdfs:range rdf:resource="http://www.w3.org/2001/XMLSchema#string"/>
        <rdfs:comment xml:lang="en">A data property identifying a telephone number for an agent.</rdfs:comment>
        <rdfs:label xml:lang="en">has phone number</rdfs:label>
    </owl:DatatypeProperty>
    


    <!-- http://purl.org/cerif/frapo/hasQualification -->

    <owl:DatatypeProperty rdf:about="http://purl.org/cerif/frapo/hasQualification">
        <rdfs:subPropertyOf rdf:resource="http://purl.org/cerif/frapo/hasPersonalInformation"/>
        <rdfs:domain rdf:resource="http://www.w3id.org/efro/efro#Person"/>
        <rdfs:range rdf:resource="http://www.w3.org/2001/XMLSchema#string"/>
        <rdfs:comment xml:lang="en">A data property permitting specification of the qualification held by a person.</rdfs:comment>
        <rdfs:label xml:lang="en">has qualification</rdfs:label>
    </owl:DatatypeProperty>
    


    <!-- http://purl.org/cerif/frapo/hasRegistrationDeadline -->

    <owl:DatatypeProperty rdf:about="http://purl.org/cerif/frapo/hasRegistrationDeadline">
        <rdf:type rdf:resource="http://www.w3.org/2002/07/owl#FunctionalProperty"/>
        <rdfs:domain rdf:resource="http://www.w3id.org/efro/efro#Person"/>
        <rdfs:range rdf:resource="http://www.w3.org/2001/XMLSchema#dateTime"/>
        <rdfs:comment xml:lang="en">The date by which registration must be made, for example renewal of an internet domain name.</rdfs:comment>
        <rdfs:label xml:lang="en">has registration deadline</rdfs:label>
    </owl:DatatypeProperty>
    


    <!-- http://www.w3id.org/efro/efro#assistanceType -->

    <owl:DatatypeProperty rdf:about="http://www.w3id.org/efro/efro#assistanceType">
        <rdfs:domain rdf:resource="http://www.w3id.org/efro/efro#Activity"/>
        <rdfs:range rdf:resource="http://www.w3.org/2001/XMLSchema#string"/>
        <dcterms:description xml:lang="en">Defines the type of support provided to students, such as financial aid, educational support, or guidance services.</dcterms:description>
        <rdfs:label xml:lang="en">assistanceType</rdfs:label>
    </owl:DatatypeProperty>
    


    <!-- http://www.w3id.org/efro/efro#canBeUsedAsWithdrawalDate -->

    <owl:DatatypeProperty rdf:about="http://www.w3id.org/efro/efro#canBeUsedAsWithdrawalDate">
        <rdfs:domain rdf:resource="http://www.w3id.org/efro/efro#Activity"/>
        <rdfs:range rdf:resource="http://www.w3.org/2001/XMLSchema#boolean"/>
        <dcterms:description xml:lang="en">Refers to a date that can be used to determine when a student is officially considered withdrawn from a study programme.</dcterms:description>
        <rdfs:label xml:lang="en">canBeUsedAsWithdrawalDate</rdfs:label>
    </owl:DatatypeProperty>
    


    <!-- http://www.w3id.org/efro/efro#hasActualDeliveredHours -->

    <owl:DatatypeProperty rdf:about="http://www.w3id.org/efro/efro#hasActualDeliveredHours">
        <rdfs:subPropertyOf rdf:resource="http://www.w3id.org/efro/efro#hasHoursValue"/>
        <rdfs:domain rdf:resource="http://www.w3id.org/efro/efro#PlannedHours"/>
        <rdfs:range>
            <rdfs:Datatype>
                <owl:onDatatype rdf:resource="http://www.w3.org/2001/XMLSchema#integer"/>
                <owl:withRestrictions rdf:parseType="Collection">
                    <rdf:Description>
                        <xsd:minInclusive rdf:datatype="http://www.w3.org/2001/XMLSchema#integer">0</xsd:minInclusive>
                    </rdf:Description>
                    <rdf:Description>
                        <xsd:maxInclusive rdf:datatype="http://www.w3.org/2001/XMLSchema#integer">40</xsd:maxInclusive>
                    </rdf:Description>
                </owl:withRestrictions>
            </rdfs:Datatype>
        </rdfs:range>
        <dcterms:description xml:lang="en">Captures the total hours of learning actually delivered to the student, including guided learning and supervised study.</dcterms:description>
        <rdfs:label>hasActualDeliveredHours</rdfs:label>
    </owl:DatatypeProperty>
    


    <!-- http://www.w3id.org/efro/efro#hasActualDuration -->

    <owl:DatatypeProperty rdf:about="http://www.w3id.org/efro/efro#hasActualDuration">
        <rdfs:subPropertyOf rdf:resource="http://www.w3id.org/efro/efro#hasDurationValue"/>
        <rdfs:domain rdf:resource="http://www.w3id.org/efro/efro#Learning"/>
        <rdfs:range>
            <rdfs:Datatype>
                <owl:onDatatype rdf:resource="http://www.w3.org/2001/XMLSchema#integer"/>
                <owl:withRestrictions rdf:parseType="Collection">
                    <rdf:Description>
                        <xsd:minInclusive rdf:datatype="http://www.w3.org/2001/XMLSchema#integer">0</xsd:minInclusive>
                    </rdf:Description>
                </owl:withRestrictions>
            </rdfs:Datatype>
        </rdfs:range>
        <dcterms:description xml:lang="en">Defines the actual time a student remained enrolled in a programme or learning aim before completion, transfer, or withdrawal​.</dcterms:description>
        <rdfs:label>hasActualDuration</rdfs:label>
    </owl:DatatypeProperty>
    


    <!-- http://www.w3id.org/efro/efro#hasAdjustedAmount -->

    <owl:DatatypeProperty rdf:about="http://www.w3id.org/efro/efro#hasAdjustedAmount">
        <rdfs:subPropertyOf rdf:resource="http://www.w3id.org/efro/efro#hasFundingValue"/>
        <rdfs:domain rdf:resource="http://www.w3id.org/efro/efro#FundingElement"/>
        <rdfs:range>
            <rdfs:Datatype>
                <owl:onDatatype rdf:resource="http://www.w3.org/2001/XMLSchema#decimal"/>
                <owl:withRestrictions rdf:parseType="Collection">
                    <rdf:Description>
                        <xsd:minInclusive rdf:datatype="http://www.w3.org/2001/XMLSchema#decimal">0.00</xsd:minInclusive>
                    </rdf:Description>
                </owl:withRestrictions>
            </rdfs:Datatype>
        </rdfs:range>
        <dcterms:description xml:lang="en">Specifies an updated funding amount that reflects adjustments due to changes in planned hours, withdrawals, or other funding criteria​</dcterms:description>
        <rdfs:label>hasAdjustedAmount</rdfs:label>
    </owl:DatatypeProperty>
    


    <!-- http://www.w3id.org/efro/efro#hasAdjustedHours -->

    <owl:DatatypeProperty rdf:about="http://www.w3id.org/efro/efro#hasAdjustedHours">
        <rdfs:subPropertyOf rdf:resource="http://www.w3id.org/efro/efro#hasHoursValue"/>
        <rdfs:domain rdf:resource="http://www.w3id.org/efro/efro#PlannedHours"/>
        <rdfs:range>
            <rdfs:Datatype>
                <owl:onDatatype rdf:resource="http://www.w3.org/2001/XMLSchema#integer"/>
                <owl:withRestrictions rdf:parseType="Collection">
                    <rdf:Description>
                        <xsd:minInclusive rdf:datatype="http://www.w3.org/2001/XMLSchema#integer">0</xsd:minInclusive>
                    </rdf:Description>
                    <rdf:Description>
                        <xsd:maxInclusive rdf:datatype="http://www.w3.org/2001/XMLSchema#integer">40</xsd:maxInclusive>
                    </rdf:Description>
                </owl:withRestrictions>
            </rdfs:Datatype>
        </rdfs:range>
        <dcterms:description xml:lang="en">Reflects any modifications made to planned learning hours due to changes in student participation, programme alterations, or withdrawals.</dcterms:description>
        <rdfs:label>hasAdjustedHours</rdfs:label>
    </owl:DatatypeProperty>
    


    <!-- http://www.w3id.org/efro/efro#hasAdjustedPlannedHours -->

    <owl:DatatypeProperty rdf:about="http://www.w3id.org/efro/efro#hasAdjustedPlannedHours">
        <rdfs:domain rdf:resource="http://www.w3id.org/efro/efro#AdjustedPlannedHours"/>
        <rdfs:range rdf:resource="http://www.w3.org/2001/XMLSchema#integer"/>
        <dcterms:description xml:lang="en">Represents the number of planned learning hours that have been modified due to changes in the student’s study plan, withdrawals, or adjustments.</dcterms:description>
        <rdfs:label xml:lang="en">hasAdjustedPlannedHours</rdfs:label>
    </owl:DatatypeProperty>
    


    <!-- http://www.w3id.org/efro/efro#hasAdjustmentReason -->

    <owl:DatatypeProperty rdf:about="http://www.w3id.org/efro/efro#hasAdjustmentReason">
        <rdfs:subPropertyOf rdf:resource="http://www.w3id.org/efro/efro#hasDescription"/>
        <rdf:type rdf:resource="http://www.w3.org/2002/07/owl#FunctionalProperty"/>
        <rdfs:domain>
            <owl:Class>
                <owl:unionOf rdf:parseType="Collection">
                    <rdf:Description rdf:about="http://www.w3id.org/efro/efro#FundingElement"/>
                    <rdf:Description rdf:about="http://www.w3id.org/efro/efro#PlannedHours"/>
                </owl:unionOf>
            </owl:Class>
        </rdfs:domain>
        <rdfs:range rdf:resource="http://www.w3.org/2001/XMLSchema#string"/>
        <dcterms:description xml:lang="en">Specifies the reason for adjusting planned hours, funding allocations, or student records, such as changes in study plans, withdrawals, or exceptional circumstances.</dcterms:description>
        <rdfs:label>hasAdjustmentReason</rdfs:label>
    </owl:DatatypeProperty>
    


    <!-- http://www.w3id.org/efro/efro#hasAimReference -->

    <owl:DatatypeProperty rdf:about="http://www.w3id.org/efro/efro#hasAimReference">
        <rdfs:domain rdf:resource="http://www.w3id.org/efro/efro#QualificationAim"/>
        <rdfs:range rdf:resource="http://www.w3.org/2001/XMLSchema#string"/>
        <dcterms:description xml:lang="en">Identifies a reference code or identifier for a specific learning aim in the educational programme, often used in funding records​.</dcterms:description>
        <rdfs:label xml:lang="en">hasAimReference</rdfs:label>
    </owl:DatatypeProperty>
    


    <!-- http://www.w3id.org/efro/efro#hasAllocatedAmount -->

    <owl:DatatypeProperty rdf:about="http://www.w3id.org/efro/efro#hasAllocatedAmount">
        <rdfs:subPropertyOf rdf:resource="http://www.w3id.org/efro/efro#hasFundingValue"/>
        <rdfs:domain rdf:resource="http://www.w3id.org/efro/efro#FundingElement"/>
        <rdfs:range>
            <rdfs:Datatype>
                <owl:onDatatype rdf:resource="http://www.w3.org/2001/XMLSchema#decimal"/>
                <owl:withRestrictions rdf:parseType="Collection">
                    <rdf:Description>
                        <xsd:minInclusive rdf:datatype="http://www.w3.org/2001/XMLSchema#decimal">0.00</xsd:minInclusive>
                    </rdf:Description>
                </owl:withRestrictions>
            </rdfs:Datatype>
        </rdfs:range>
        <dcterms:description xml:lang="en">Represents the initially assigned funding amount for a student or programme before any modifications​.</dcterms:description>
        <rdfs:label>hasAllocatedAmount</rdfs:label>
    </owl:DatatypeProperty>
    


    <!-- http://www.w3id.org/efro/efro#hasAttendanceStatus -->

    <owl:DatatypeProperty rdf:about="http://www.w3id.org/efro/efro#hasAttendanceStatus">
        <rdfs:subPropertyOf rdf:resource="http://www.w3id.org/efro/efro#hasStatusValue"/>
        <rdfs:domain rdf:resource="http://www.w3id.org/efro/efro#AttendanceStatus"/>
        <rdfs:range>
            <rdfs:Datatype>
                <owl:oneOf>
                    <rdf:Description>
                        <rdf:type rdf:resource="http://www.w3.org/1999/02/22-rdf-syntax-ns#List"/>
                        <rdf:first>Absent</rdf:first>
                        <rdf:rest>
                            <rdf:Description>
                                <rdf:type rdf:resource="http://www.w3.org/1999/02/22-rdf-syntax-ns#List"/>
                                <rdf:first>Authorized</rdf:first>
                                <rdf:rest>
                                    <rdf:Description>
                                        <rdf:type rdf:resource="http://www.w3.org/1999/02/22-rdf-syntax-ns#List"/>
                                        <rdf:first>Present</rdf:first>
                                        <rdf:rest>
                                            <rdf:Description>
                                                <rdf:type rdf:resource="http://www.w3.org/1999/02/22-rdf-syntax-ns#List"/>
                                                <rdf:first>Unauthorized</rdf:first>
                                                <rdf:rest rdf:resource="http://www.w3.org/1999/02/22-rdf-syntax-ns#nil"/>
                                            </rdf:Description>
                                        </rdf:rest>
                                    </rdf:Description>
                                </rdf:rest>
                            </rdf:Description>
                        </rdf:rest>
                    </rdf:Description>
                </owl:oneOf>
            </rdfs:Datatype>
        </rdfs:range>
        <dcterms:description xml:lang="en">Indicates whether a student is actively attending, absent, or has irregular attendance, affecting funding eligibility.</dcterms:description>
        <rdfs:label>hasAttendanceStatus</rdfs:label>
    </owl:DatatypeProperty>
    


    <!-- http://www.w3id.org/efro/efro#hasCompleteStatus -->

    <owl:DatatypeProperty rdf:about="http://www.w3id.org/efro/efro#hasCompleteStatus">
        <rdfs:subPropertyOf rdf:resource="http://www.w3id.org/efro/efro#hasStatusValue"/>
        <rdfs:domain rdf:resource="http://www.w3id.org/efro/efro#CompletionStatus"/>
        <rdfs:range>
            <rdfs:Datatype>
                <owl:oneOf>
                    <rdf:Description>
                        <rdf:type rdf:resource="http://www.w3.org/1999/02/22-rdf-syntax-ns#List"/>
                        <rdf:first>Complete</rdf:first>
                        <rdf:rest>
                            <rdf:Description>
                                <rdf:type rdf:resource="http://www.w3.org/1999/02/22-rdf-syntax-ns#List"/>
                                <rdf:first>EarlyCompletion</rdf:first>
                                <rdf:rest>
                                    <rdf:Description>
                                        <rdf:type rdf:resource="http://www.w3.org/1999/02/22-rdf-syntax-ns#List"/>
                                        <rdf:first>Incomplete</rdf:first>
                                        <rdf:rest rdf:resource="http://www.w3.org/1999/02/22-rdf-syntax-ns#nil"/>
                                    </rdf:Description>
                                </rdf:rest>
                            </rdf:Description>
                        </rdf:rest>
                    </rdf:Description>
                </owl:oneOf>
            </rdfs:Datatype>
        </rdfs:range>
        <dcterms:description xml:lang="en">Specifies whether a student has completed their learning aim successfully, failed, or left the course before completion​.</dcterms:description>
        <rdfs:label>hasCompleteStatus</rdfs:label>
    </owl:DatatypeProperty>
    


    <!-- http://www.w3id.org/efro/efro#hasCompletionDate -->

    <owl:DatatypeProperty rdf:about="http://www.w3id.org/efro/efro#hasCompletionDate">
        <rdfs:subPropertyOf rdf:resource="http://www.w3id.org/efro/efro#hasTemporalValue"/>
        <rdfs:domain>
            <owl:Class>
                <owl:unionOf rdf:parseType="Collection">
                    <rdf:Description rdf:about="http://www.w3id.org/efro/efro#CompletionActivity"/>
                    <rdf:Description rdf:about="http://www.w3id.org/efro/efro#Learning"/>
                </owl:unionOf>
            </owl:Class>
        </rdfs:domain>
        <rdfs:range rdf:resource="http://www.w3.org/2001/XMLSchema#dateTime"/>
        <dcterms:description xml:lang="en">Specifies the official date when a student successfully completes a learning aim or study programme​.</dcterms:description>
        <rdfs:label>hasCompletionDate</rdfs:label>
    </owl:DatatypeProperty>
    


    <!-- http://www.w3id.org/efro/efro#hasCompletionDetails -->

    <owl:DatatypeProperty rdf:about="http://www.w3id.org/efro/efro#hasCompletionDetails">
        <rdfs:subPropertyOf rdf:resource="http://www.w3id.org/efro/efro#hasDescription"/>
        <rdf:type rdf:resource="http://www.w3.org/2002/07/owl#FunctionalProperty"/>
        <rdfs:domain rdf:resource="http://www.w3id.org/efro/efro#CompletionActivity"/>
        <rdfs:range rdf:resource="http://www.w3.org/2001/XMLSchema#string"/>
        <dcterms:description xml:lang="en">Captures details about how and when a student has completed a learning aim or programme, including whether they met the qualifying period​.</dcterms:description>
        <rdfs:label>hasCompletionDetails</rdfs:label>
    </owl:DatatypeProperty>
    


    <!-- http://www.w3id.org/efro/efro#hasDate -->

    <owl:DatatypeProperty rdf:about="http://www.w3id.org/efro/efro#hasDate">
        <rdfs:domain>
            <owl:Class>
                <owl:unionOf rdf:parseType="Collection">
                    <rdf:Description rdf:about="http://www.w3id.org/efro/efro#Activity"/>
                    <rdf:Description rdf:about="http://www.w3id.org/efro/efro#TimeRelated"/>
                </owl:unionOf>
            </owl:Class>
        </rdfs:domain>
        <rdfs:range rdf:resource="http://www.w3.org/2001/XMLSchema#dateTime"/>
        <dcterms:description xml:lang="en">A generic property representing any relevant date associated with funding, learning activities, enrolment, or withdrawal.</dcterms:description>
        <rdfs:label xml:lang="en">hasDate</rdfs:label>
    </owl:DatatypeProperty>
    


    <!-- http://www.w3id.org/efro/efro#hasDescription -->

    <owl:DatatypeProperty rdf:about="http://www.w3id.org/efro/efro#hasDescription">
        <rdfs:domain>
            <owl:Class>
                <owl:unionOf rdf:parseType="Collection">
                    <rdf:Description rdf:about="http://www.w3id.org/efro/efro#Activity"/>
                    <rdf:Description rdf:about="http://www.w3id.org/efro/efro#Document"/>
                    <rdf:Description rdf:about="http://www.w3id.org/efro/efro#EducationalEntity"/>
                    <rdf:Description rdf:about="http://www.w3id.org/efro/efro#FundingElement"/>
                    <rdf:Description rdf:about="http://www.w3id.org/efro/efro#Learning"/>
                    <rdf:Description rdf:about="http://www.w3id.org/efro/efro#Obligation"/>
                    <rdf:Description rdf:about="http://www.w3id.org/efro/efro#Person"/>
                    <rdf:Description rdf:about="http://www.w3id.org/efro/efro#Reason"/>
                    <rdf:Description rdf:about="http://www.w3id.org/efro/efro#Status"/>
                    <rdf:Description rdf:about="http://www.w3id.org/efro/efro#TimeRelated"/>
                </owl:unionOf>
            </owl:Class>
        </rdfs:domain>
        <rdfs:range rdf:resource="http://www.w3.org/2001/XMLSchema#string"/>
        <dcterms:description xml:lang="en">Provides a textual explanation or detailed information about a particular funding-related concept, activity, or rule within the educational funding framework.</dcterms:description>
        <rdfs:label>hasDescription</rdfs:label>
    </owl:DatatypeProperty>
    


    <!-- http://www.w3id.org/efro/efro#hasDurationValue -->

    <owl:DatatypeProperty rdf:about="http://www.w3id.org/efro/efro#hasDurationValue">
        <rdfs:domain rdf:resource="http://www.w3id.org/efro/efro#TimeRelated"/>
        <rdfs:range rdf:resource="http://www.w3.org/2001/XMLSchema#integer"/>
        <dcterms:description xml:lang="en">Represents the time-related aspects of a study programme, learning aim, or funding period.</dcterms:description>
        <rdfs:label>hasDurationValue</rdfs:label>
    </owl:DatatypeProperty>
    


    <!-- http://www.w3id.org/efro/efro#hasEarliestStartDate -->

    <owl:DatatypeProperty rdf:about="http://www.w3id.org/efro/efro#hasEarliestStartDate">
        <rdfs:subPropertyOf rdf:resource="http://www.w3id.org/efro/efro#hasTemporalValue"/>
        <rdfs:domain rdf:resource="http://www.w3id.org/efro/efro#LearningAim"/>
        <rdfs:range rdf:resource="http://www.w3.org/2001/XMLSchema#dateTime"/>
        <dcterms:description xml:lang="en">Represents the first possible start date for a study programme, determining the qualifying period for funding eligibility.</dcterms:description>
        <rdfs:label>hasEarliestStartDate</rdfs:label>
    </owl:DatatypeProperty>
    


    <!-- http://www.w3id.org/efro/efro#hasEndDate -->

    <owl:DatatypeProperty rdf:about="http://www.w3id.org/efro/efro#hasEndDate">
        <rdfs:subPropertyOf rdf:resource="http://www.w3id.org/efro/efro#hasTemporalValue"/>
        <rdfs:domain rdf:resource="http://www.w3id.org/efro/efro#FundingYear"/>
        <rdfs:range rdf:resource="http://www.w3.org/2001/XMLSchema#dateTime"/>
        <dcterms:description xml:lang="en">The official or anticipated end date of a student&apos;s learning aim, used for funding and tracking progression​.</dcterms:description>
        <rdfs:label>hasEndDate</rdfs:label>
    </owl:DatatypeProperty>
    


    <!-- http://www.w3id.org/efro/efro#hasEnrollmentStatus -->

    <owl:DatatypeProperty rdf:about="http://www.w3id.org/efro/efro#hasEnrollmentStatus">
        <rdfs:subPropertyOf rdf:resource="http://www.w3id.org/efro/efro#hasStatusValue"/>
        <rdfs:domain rdf:resource="http://www.w3id.org/efro/efro#EnrollmentStatus"/>
        <rdfs:range>
            <rdfs:Datatype>
                <owl:oneOf>
                    <rdf:Description>
                        <rdf:type rdf:resource="http://www.w3.org/1999/02/22-rdf-syntax-ns#List"/>
                        <rdf:first>Active</rdf:first>
                        <rdf:rest>
                            <rdf:Description>
                                <rdf:type rdf:resource="http://www.w3.org/1999/02/22-rdf-syntax-ns#List"/>
                                <rdf:first>Completed</rdf:first>
                                <rdf:rest>
                                    <rdf:Description>
                                        <rdf:type rdf:resource="http://www.w3.org/1999/02/22-rdf-syntax-ns#List"/>
                                        <rdf:first>Withdrawn</rdf:first>
                                        <rdf:rest rdf:resource="http://www.w3.org/1999/02/22-rdf-syntax-ns#nil"/>
                                    </rdf:Description>
                                </rdf:rest>
                            </rdf:Description>
                        </rdf:rest>
                    </rdf:Description>
                </owl:oneOf>
            </rdfs:Datatype>
        </rdfs:range>
        <dcterms:description xml:lang="en">Denotes whether a student is currently enrolled, deferred, or has withdrawn from the programme.</dcterms:description>
        <rdfs:label>hasEnrollmentStatus</rdfs:label>
    </owl:DatatypeProperty>
    


    <!-- http://www.w3id.org/efro/efro#hasExcludedHours -->

    <owl:DatatypeProperty rdf:about="http://www.w3id.org/efro/efro#hasExcludedHours">
        <rdfs:subPropertyOf rdf:resource="http://www.w3id.org/efro/efro#hasHoursValue"/>
        <rdfs:domain rdf:resource="http://www.w3id.org/efro/efro#ExcludedHours"/>
        <rdfs:range rdf:resource="http://www.w3.org/2001/XMLSchema#integer"/>
        <dcterms:description xml:lang="en">Represents learning hours that are excluded from funding claims due to non-qualification activities, self-study, or ineligible activities.</dcterms:description>
        <rdfs:label>hasExcludedHours</rdfs:label>
    </owl:DatatypeProperty>
    


    <!-- http://www.w3id.org/efro/efro#hasFundingID -->

    <owl:DatatypeProperty rdf:about="http://www.w3id.org/efro/efro#hasFundingID">
        <rdfs:subPropertyOf rdf:resource="http://www.w3id.org/efro/efro#hasIdentifier"/>
        <rdfs:domain rdf:resource="http://www.w3id.org/efro/efro#FundingElement"/>
        <rdfs:range rdf:resource="http://www.w3.org/2001/XMLSchema#string"/>
        <dcterms:description xml:lang="en">Identifies the unique funding reference number assigned to a specific student or programme for tracking financial allocations.</dcterms:description>
        <rdfs:label>hasFundingID</rdfs:label>
    </owl:DatatypeProperty>
    


    <!-- http://www.w3id.org/efro/efro#hasFundingStatus -->

    <owl:DatatypeProperty rdf:about="http://www.w3id.org/efro/efro#hasFundingStatus">
        <rdfs:subPropertyOf rdf:resource="http://www.w3id.org/efro/efro#hasStatusValue"/>
        <rdfs:domain rdf:resource="http://www.w3id.org/efro/efro#FundingStatus"/>
        <rdfs:range>
            <rdfs:Datatype>
                <owl:oneOf>
                    <rdf:Description>
                        <rdf:type rdf:resource="http://www.w3.org/1999/02/22-rdf-syntax-ns#List"/>
                        <rdf:first>Funded</rdf:first>
                        <rdf:rest>
                            <rdf:Description>
                                <rdf:type rdf:resource="http://www.w3.org/1999/02/22-rdf-syntax-ns#List"/>
                                <rdf:first>NotFunded</rdf:first>
                                <rdf:rest>
                                    <rdf:Description>
                                        <rdf:type rdf:resource="http://www.w3.org/1999/02/22-rdf-syntax-ns#List"/>
                                        <rdf:first>PartiallyFunded</rdf:first>
                                        <rdf:rest rdf:resource="http://www.w3.org/1999/02/22-rdf-syntax-ns#nil"/>
                                    </rdf:Description>
                                </rdf:rest>
                            </rdf:Description>
                        </rdf:rest>
                    </rdf:Description>
                </owl:oneOf>
            </rdfs:Datatype>
        </rdfs:range>
        <dcterms:description xml:lang="en">Reflects whether a student’s funding is active, suspended, reduced, or withdrawn based on their participation and eligibility.</dcterms:description>
        <rdfs:label>hasFundingStatus</rdfs:label>
    </owl:DatatypeProperty>
    


    <!-- http://www.w3id.org/efro/efro#hasFundingValue -->

    <owl:DatatypeProperty rdf:about="http://www.w3id.org/efro/efro#hasFundingValue">
        <rdfs:domain rdf:resource="http://www.w3id.org/efro/efro#FundingElement"/>
        <rdfs:range rdf:resource="http://www.w3.org/2001/XMLSchema#decimal"/>
        <dcterms:description xml:lang="en">Represents monetary allocations related to student enrolment, learning aims, and retention for funding purposes.</dcterms:description>
        <rdfs:label>hasFundingValue</rdfs:label>
    </owl:DatatypeProperty>
    


    <!-- http://www.w3id.org/efro/efro#hasHoursPlanned -->

    <owl:DatatypeProperty rdf:about="http://www.w3id.org/efro/efro#hasHoursPlanned">
        <rdfs:subPropertyOf rdf:resource="http://www.w3id.org/efro/efro#hasHoursValue"/>
        <rdfs:domain rdf:resource="http://www.w3id.org/efro/efro#PlannedHours"/>
        <rdfs:range rdf:resource="http://www.w3.org/2001/XMLSchema#integer"/>
        <dcterms:description xml:lang="en">Defines the expected learning hours allocated to a study programme at the start of the academic year​.</dcterms:description>
        <rdfs:label>hasHoursPlanned</rdfs:label>
    </owl:DatatypeProperty>
    


    <!-- http://www.w3id.org/efro/efro#hasHoursValue -->

    <owl:DatatypeProperty rdf:about="http://www.w3id.org/efro/efro#hasHoursValue">
        <rdfs:domain rdf:resource="http://www.w3id.org/efro/efro#PlannedHours"/>
        <rdfs:range rdf:resource="http://www.w3.org/2001/XMLSchema#integer"/>
        <dcterms:description xml:lang="en">Represents the number of learning hours recorded for funding purposes, including planned, adjusted, or excluded hours.</dcterms:description>
        <rdfs:label>hasHoursValue</rdfs:label>
    </owl:DatatypeProperty>
    


    <!-- http://www.w3id.org/efro/efro#hasIdentifier -->

    <owl:DatatypeProperty rdf:about="http://www.w3id.org/efro/efro#hasIdentifier">
        <rdfs:domain>
            <owl:Class>
                <owl:unionOf rdf:parseType="Collection">
                    <rdf:Description rdf:about="http://www.w3id.org/efro/efro#Activity"/>
                    <rdf:Description rdf:about="http://www.w3id.org/efro/efro#Document"/>
                    <rdf:Description rdf:about="http://www.w3id.org/efro/efro#EducationalEntity"/>
                    <rdf:Description rdf:about="http://www.w3id.org/efro/efro#FundingElement"/>
                    <rdf:Description rdf:about="http://www.w3id.org/efro/efro#Learning"/>
                    <rdf:Description rdf:about="http://www.w3id.org/efro/efro#Obligation"/>
                    <rdf:Description rdf:about="http://www.w3id.org/efro/efro#Person"/>
                    <rdf:Description rdf:about="http://www.w3id.org/efro/efro#Reason"/>
                    <rdf:Description rdf:about="http://www.w3id.org/efro/efro#Status"/>
                    <rdf:Description rdf:about="http://www.w3id.org/efro/efro#TimeRelated"/>
                </owl:unionOf>
            </owl:Class>
        </rdfs:domain>
        <rdfs:range rdf:resource="http://www.w3.org/2001/XMLSchema#string"/>
        <dcterms:description xml:lang="en">Represents unique identifiers assigned to various entities within the educational funding framework.</dcterms:description>
        <rdfs:label>hasIdentifier</rdfs:label>
    </owl:DatatypeProperty>
    


    <!-- http://www.w3id.org/efro/efro#hasInstitutionID -->

    <owl:DatatypeProperty rdf:about="http://www.w3id.org/efro/efro#hasInstitutionID">
        <rdfs:subPropertyOf rdf:resource="http://www.w3id.org/efro/efro#hasIdentifier"/>
        <rdfs:domain rdf:resource="http://www.w3id.org/efro/efro#EducationalEntity"/>
        <rdfs:range rdf:resource="http://www.w3.org/2001/XMLSchema#string"/>
        <dcterms:description xml:lang="en">Specifies the unique identifier for an educational institution, used in funding and regulatory reporting​.</dcterms:description>
        <rdfs:label>hasInstitutionID</rdfs:label>
    </owl:DatatypeProperty>
    


    <!-- http://www.w3id.org/efro/efro#hasLastAttendanceDate -->

    <owl:DatatypeProperty rdf:about="http://www.w3id.org/efro/efro#hasLastAttendanceDate">
        <rdfs:subPropertyOf rdf:resource="http://www.w3id.org/efro/efro#hasTemporalValue"/>
        <rdfs:domain>
            <owl:Class>
                <owl:unionOf rdf:parseType="Collection">
                    <rdf:Description rdf:about="http://www.w3id.org/efro/efro#LastAttendanceActivity"/>
                    <rdf:Description rdf:about="http://www.w3id.org/efro/efro#Student"/>
                </owl:unionOf>
            </owl:Class>
        </rdfs:domain>
        <rdfs:range rdf:resource="http://www.w3.org/2001/XMLSchema#dateTime"/>
        <dcterms:description xml:lang="en">Captures the last recorded date a student attended a learning activity before withdrawal, completion, or absence​.</dcterms:description>
        <rdfs:label>hasLastAttendanceDate</rdfs:label>
    </owl:DatatypeProperty>
    


    <!-- http://www.w3id.org/efro/efro#hasMetFundingCriteria -->

    <owl:DatatypeProperty rdf:about="http://www.w3id.org/efro/efro#hasMetFundingCriteria">
        <rdfs:domain rdf:resource="http://www.w3id.org/efro/efro#Student"/>
        <rdfs:range rdf:resource="http://www.w3.org/2001/XMLSchema#boolean"/>
        <dcterms:description xml:lang="en">Indicates whether a student or programme has met the eligibility criteria for funding, based on the ESFA guidelines​.</dcterms:description>
        <rdfs:label xml:lang="en">hasMetFundingCriteria</rdfs:label>
    </owl:DatatypeProperty>
    


    <!-- http://www.w3id.org/efro/efro#hasNonAttendanceReason -->

    <owl:DatatypeProperty rdf:about="http://www.w3id.org/efro/efro#hasNonAttendanceReason">
        <rdfs:subPropertyOf rdf:resource="http://www.w3id.org/efro/efro#hasDescription"/>
        <rdf:type rdf:resource="http://www.w3.org/2002/07/owl#FunctionalProperty"/>
        <rdfs:domain rdf:resource="http://www.w3id.org/efro/efro#NonAttendanceReason"/>
        <rdfs:range rdf:resource="http://www.w3.org/2001/XMLSchema#string"/>
        <dcterms:description xml:lang="en">Describes the reason for a student’s absence from their study programme, which may impact funding eligibility, retention, or planned hours.</dcterms:description>
        <rdfs:label>hasNonAttendanceReason</rdfs:label>
    </owl:DatatypeProperty>
    


    <!-- http://www.w3id.org/efro/efro#hasOriginalPlannedHours -->

    <owl:DatatypeProperty rdf:about="http://www.w3id.org/efro/efro#hasOriginalPlannedHours">
        <rdfs:domain rdf:resource="http://www.w3id.org/efro/efro#PlannedHours"/>
        <rdfs:range rdf:resource="http://www.w3.org/2001/XMLSchema#integer"/>
        <dcterms:description xml:lang="en">Captures the initial number of planned learning hours assigned to a student before any adjustments​.</dcterms:description>
        <rdfs:label>hasOriginalPlannedHours</rdfs:label>
    </owl:DatatypeProperty>
    


    <!-- http://www.w3id.org/efro/efro#hasPlannedDuration -->

    <owl:DatatypeProperty rdf:about="http://www.w3id.org/efro/efro#hasPlannedDuration">
        <rdfs:subPropertyOf rdf:resource="http://www.w3id.org/efro/efro#hasDurationValue"/>
        <rdfs:domain rdf:resource="http://www.w3id.org/efro/efro#Learning"/>
        <rdfs:range>
            <rdfs:Datatype>
                <owl:onDatatype rdf:resource="http://www.w3.org/2001/XMLSchema#integer"/>
                <owl:withRestrictions rdf:parseType="Collection">
                    <rdf:Description>
                        <xsd:minInclusive rdf:datatype="http://www.w3.org/2001/XMLSchema#integer">1</xsd:minInclusive>
                    </rdf:Description>
                </owl:withRestrictions>
            </rdfs:Datatype>
        </rdfs:range>
        <dcterms:description xml:lang="en">Specifies the expected length of a programme or course as originally planned and recorded in funding records​.</dcterms:description>
        <rdfs:label>hasPlannedDuration</rdfs:label>
    </owl:DatatypeProperty>
    


    <!-- http://www.w3id.org/efro/efro#hasPlannedEndDate -->

    <owl:DatatypeProperty rdf:about="http://www.w3id.org/efro/efro#hasPlannedEndDate">
        <rdfs:subPropertyOf rdf:resource="http://www.w3id.org/efro/efro#hasTemporalValue"/>
        <rdfs:domain>
            <owl:Class>
                <owl:unionOf rdf:parseType="Collection">
                    <rdf:Description rdf:about="http://www.w3id.org/efro/efro#LearningAim"/>
                    <rdf:Description rdf:about="http://www.w3id.org/efro/efro#StudyProgramme"/>
                </owl:unionOf>
            </owl:Class>
        </rdfs:domain>
        <rdfs:range rdf:resource="http://www.w3.org/2001/XMLSchema#dateTime"/>
        <dcterms:description xml:lang="en">Indicates the expected completion date set at the start of the study programme, which may differ from the actual end date</dcterms:description>
        <rdfs:label>hasPlannedEndDate</rdfs:label>
    </owl:DatatypeProperty>
    


    <!-- http://www.w3id.org/efro/efro#hasProgrammeID -->

    <owl:DatatypeProperty rdf:about="http://www.w3id.org/efro/efro#hasProgrammeID">
        <rdfs:subPropertyOf rdf:resource="http://www.w3id.org/efro/efro#hasIdentifier"/>
        <rdfs:domain rdf:resource="http://www.w3id.org/efro/efro#StudyProgramme"/>
        <rdfs:range rdf:resource="http://www.w3.org/2001/XMLSchema#string"/>
        <dcterms:description xml:lang="en">Represents the identifier assigned to a specific study programme or qualification pathway​.</dcterms:description>
        <rdfs:label>hasProgrammeID</rdfs:label>
    </owl:DatatypeProperty>
    


    <!-- http://www.w3id.org/efro/efro#hasProgressionDate -->

    <owl:DatatypeProperty rdf:about="http://www.w3id.org/efro/efro#hasProgressionDate">
        <rdfs:subPropertyOf rdf:resource="http://www.w3id.org/efro/efro#hasTemporalValue"/>
        <rdfs:domain rdf:resource="http://www.w3id.org/efro/efro#ProgressionActivity"/>
        <rdfs:range rdf:resource="http://www.w3.org/2001/XMLSchema#dateTime"/>
        <dcterms:description xml:lang="en">Records the date a student progresses to the next stage of their learning pathway, such as transitioning from one qualification to another.</dcterms:description>
        <rdfs:label>hasProgressionDate</rdfs:label>
    </owl:DatatypeProperty>
    


    <!-- http://www.w3id.org/efro/efro#hasQualifyingDate -->

    <owl:DatatypeProperty rdf:about="http://www.w3id.org/efro/efro#hasQualifyingDate">
        <rdfs:subPropertyOf rdf:resource="http://www.w3id.org/efro/efro#hasTemporalValue"/>
        <rdfs:domain rdf:resource="http://www.w3id.org/efro/efro#QualifyingPeriod"/>
        <rdfs:range rdf:resource="http://www.w3.org/2001/XMLSchema#dateTime"/>
        <dcterms:description xml:lang="en">Defines the date when a student becomes eligible for funding by meeting attendance and participation requirements​.</dcterms:description>
        <rdfs:label>hasQualifyingDate</rdfs:label>
    </owl:DatatypeProperty>
    


    <!-- http://www.w3id.org/efro/efro#hasQualifyingPeriodDuration -->

    <owl:DatatypeProperty rdf:about="http://www.w3id.org/efro/efro#hasQualifyingPeriodDuration">
        <rdfs:subPropertyOf rdf:resource="http://www.w3id.org/efro/efro#hasDurationValue"/>
        <rdfs:domain rdf:resource="http://www.w3id.org/efro/efro#QualifyingPeriod"/>
        <rdfs:range>
            <rdfs:Datatype>
                <owl:onDatatype rdf:resource="http://www.w3.org/2001/XMLSchema#integer"/>
                <owl:withRestrictions rdf:parseType="Collection">
                    <rdf:Description>
                        <xsd:minInclusive rdf:datatype="http://www.w3.org/2001/XMLSchema#integer">6</xsd:minInclusive>
                    </rdf:Description>
                </owl:withRestrictions>
            </rdfs:Datatype>
        </rdfs:range>
        <dcterms:description xml:lang="en">Represents the minimum period a student must remain enrolled to qualify for funding, ensuring institutions receive appropriate allocations.</dcterms:description>
        <rdfs:label>hasQualifyingPeriodDuration</rdfs:label>
    </owl:DatatypeProperty>
    


    <!-- http://www.w3id.org/efro/efro#hasReductionAmount -->

    <owl:DatatypeProperty rdf:about="http://www.w3id.org/efro/efro#hasReductionAmount">
        <rdfs:subPropertyOf rdf:resource="http://www.w3id.org/efro/efro#hasFundingValue"/>
        <rdfs:domain rdf:resource="http://www.w3id.org/efro/efro#FundingElement"/>
        <rdfs:range>
            <rdfs:Datatype>
                <owl:onDatatype rdf:resource="http://www.w3.org/2001/XMLSchema#decimal"/>
                <owl:withRestrictions rdf:parseType="Collection">
                    <rdf:Description>
                        <xsd:minInclusive rdf:datatype="http://www.w3.org/2001/XMLSchema#decimal">0.00</xsd:minInclusive>
                    </rdf:Description>
                </owl:withRestrictions>
            </rdfs:Datatype>
        </rdfs:range>
        <dcterms:description xml:lang="en">Captures the amount deducted from an allocated funding value due to early withdrawals, non-completion, or ineligible hours​.</dcterms:description>
        <rdfs:label>hasReductionAmount</rdfs:label>
    </owl:DatatypeProperty>
    


    <!-- http://www.w3id.org/efro/efro#hasReference -->

    <owl:DatatypeProperty rdf:about="http://www.w3id.org/efro/efro#hasReference">
        <rdfs:domain rdf:resource="http://www.w3id.org/efro/efro#Obligation"/>
        <rdfs:range rdf:resource="http://www.w3.org/2001/XMLSchema#string"/>
        <dcterms:description xml:lang="en">Provides a unique identifier or reference number for records, learning aims, or funding-related documentation.</dcterms:description>
        <rdfs:label>hasReference</rdfs:label>
    </owl:DatatypeProperty>
    


    <!-- http://www.w3id.org/efro/efro#hasRetentionValue -->

    <owl:DatatypeProperty rdf:about="http://www.w3id.org/efro/efro#hasRetentionValue">
        <rdfs:subPropertyOf rdf:resource="http://www.w3id.org/efro/efro#hasFundingValue"/>
        <rdfs:domain rdf:resource="http://www.w3id.org/efro/efro#FundingElement"/>
        <rdfs:range>
            <rdfs:Datatype>
                <owl:onDatatype rdf:resource="http://www.w3.org/2001/XMLSchema#decimal"/>
                <owl:withRestrictions rdf:parseType="Collection">
                    <rdf:Description>
                        <xsd:minInclusive rdf:datatype="http://www.w3.org/2001/XMLSchema#decimal">0.00</xsd:minInclusive>
                    </rdf:Description>
                    <rdf:Description>
                        <xsd:maxInclusive rdf:datatype="http://www.w3.org/2001/XMLSchema#decimal">1.00</xsd:maxInclusive>
                    </rdf:Description>
                </owl:withRestrictions>
            </rdfs:Datatype>
        </rdfs:range>
        <dcterms:description xml:lang="en">Indicates the funding value assigned for students who meet retention criteria and complete the required duration of study.</dcterms:description>
        <rdfs:label>hasRetentionValue</rdfs:label>
    </owl:DatatypeProperty>
    


    <!-- http://www.w3id.org/efro/efro#hasStaffID -->

    <owl:DatatypeProperty rdf:about="http://www.w3id.org/efro/efro#hasStaffID">
        <rdfs:subPropertyOf rdf:resource="http://www.w3id.org/efro/efro#hasIdentifier"/>
        <rdfs:domain rdf:resource="http://www.w3id.org/efro/efro#Staff"/>
        <rdfs:range rdf:resource="http://www.w3.org/2001/XMLSchema#string"/>
        <dcterms:description xml:lang="en">Denotes a unique identifier for staff members involved in delivering funded study programmes​.</dcterms:description>
        <rdfs:label>hasStaffID</rdfs:label>
    </owl:DatatypeProperty>
    


    <!-- http://www.w3id.org/efro/efro#hasStartDate -->

    <owl:DatatypeProperty rdf:about="http://www.w3id.org/efro/efro#hasStartDate">
        <rdfs:subPropertyOf rdf:resource="http://www.w3id.org/efro/efro#hasTemporalValue"/>
        <rdfs:domain>
            <owl:Class>
                <owl:unionOf rdf:parseType="Collection">
                    <rdf:Description rdf:about="http://www.w3id.org/efro/efro#Activity"/>
                    <rdf:Description rdf:about="http://www.w3id.org/efro/efro#Learning"/>
                    <rdf:Description rdf:about="http://www.w3id.org/efro/efro#StudyProgramme"/>
                </owl:unionOf>
            </owl:Class>
        </rdfs:domain>
        <rdfs:range rdf:resource="http://www.w3.org/2001/XMLSchema#dateTime"/>
        <dcterms:description xml:lang="en">The official commencement date of a student&apos;s learning aim or study programme​.</dcterms:description>
        <rdfs:label>hasStartDate</rdfs:label>
    </owl:DatatypeProperty>
    


    <!-- http://www.w3id.org/efro/efro#hasStatusValue -->

    <owl:DatatypeProperty rdf:about="http://www.w3id.org/efro/efro#hasStatusValue">
        <rdfs:domain rdf:resource="http://www.w3id.org/efro/efro#Status"/>
        <rdfs:range rdf:resource="http://www.w3.org/2001/XMLSchema#string"/>
        <dcterms:description xml:lang="en">Represents the current status of a student&apos;s enrolment, funding, or participation in a learning programme.</dcterms:description>
        <rdfs:label>hasStatusValue</rdfs:label>
    </owl:DatatypeProperty>
    


    <!-- http://www.w3id.org/efro/efro#hasStudentID -->

    <owl:DatatypeProperty rdf:about="http://www.w3id.org/efro/efro#hasStudentID">
        <rdfs:subPropertyOf rdf:resource="http://www.w3id.org/efro/efro#hasIdentifier"/>
        <rdfs:domain rdf:resource="http://www.w3id.org/efro/efro#Student"/>
        <rdfs:range rdf:resource="http://www.w3.org/2001/XMLSchema#string"/>
        <dcterms:description xml:lang="en">Provides a unique reference number for students enrolled in funded programmes, ensuring accurate tracking of learning progress and funding eligibility.</dcterms:description>
        <rdfs:label>hasStudentID</rdfs:label>
    </owl:DatatypeProperty>
    


    <!-- http://www.w3id.org/efro/efro#hasTemporalValue -->

    <owl:DatatypeProperty rdf:about="http://www.w3id.org/efro/efro#hasTemporalValue">
        <rdfs:domain rdf:resource="http://www.w3id.org/efro/efro#TimeRelated"/>
        <rdfs:range rdf:resource="http://www.w3.org/2001/XMLSchema#dateTime"/>
        <dcterms:description xml:lang="en">Represents date-related aspects of a student’s learning journey, including start, end, and milestone dates.</dcterms:description>
        <rdfs:label>hasTemporalValue</rdfs:label>
    </owl:DatatypeProperty>
    


    <!-- http://www.w3id.org/efro/efro#hasTotalPlannedHours -->

    <owl:DatatypeProperty rdf:about="http://www.w3id.org/efro/efro#hasTotalPlannedHours">
        <rdfs:subPropertyOf rdf:resource="http://www.w3id.org/efro/efro#hasHoursValue"/>
        <rdfs:domain rdf:resource="http://www.w3id.org/efro/efro#PlannedHours"/>
        <rdfs:range>
            <rdfs:Datatype>
                <owl:onDatatype rdf:resource="http://www.w3.org/2001/XMLSchema#integer"/>
                <owl:withRestrictions rdf:parseType="Collection">
                    <rdf:Description>
                        <xsd:minInclusive rdf:datatype="http://www.w3.org/2001/XMLSchema#integer">0</xsd:minInclusive>
                    </rdf:Description>
                    <rdf:Description>
                        <xsd:maxInclusive rdf:datatype="http://www.w3.org/2001/XMLSchema#integer">40</xsd:maxInclusive>
                    </rdf:Description>
                </owl:withRestrictions>
            </rdfs:Datatype>
        </rdfs:range>
        <dcterms:description xml:lang="en">Denotes the cumulative planned hours for a student’s study programme, including all qualification and eligible non-qualification activities​.</dcterms:description>
        <rdfs:label>hasTotalPlannedHours</rdfs:label>
    </owl:DatatypeProperty>
    


    <!-- http://www.w3id.org/efro/efro#hasWeeksDuration -->

    <owl:DatatypeProperty rdf:about="http://www.w3id.org/efro/efro#hasWeeksDuration">
        <rdfs:subPropertyOf rdf:resource="http://www.w3id.org/efro/efro#hasDurationValue"/>
        <rdfs:domain rdf:resource="http://www.w3id.org/efro/efro#TimeRelated"/>
        <rdfs:range>
            <rdfs:Datatype>
                <owl:onDatatype rdf:resource="http://www.w3.org/2001/XMLSchema#integer"/>
                <owl:withRestrictions rdf:parseType="Collection">
                    <rdf:Description>
                        <xsd:minInclusive rdf:datatype="http://www.w3.org/2001/XMLSchema#integer">1</xsd:minInclusive>
                    </rdf:Description>
                </owl:withRestrictions>
            </rdfs:Datatype>
        </rdfs:range>
        <dcterms:description xml:lang="en">Indicates the duration of a learning aim or study programme in terms of weeks, often used in eligibility and funding calculations.</dcterms:description>
        <rdfs:label>hasWeeksDuration</rdfs:label>
    </owl:DatatypeProperty>
    


    <!-- http://www.w3id.org/efro/efro#hasWithdrawReason -->

    <owl:DatatypeProperty rdf:about="http://www.w3id.org/efro/efro#hasWithdrawReason">
        <rdfs:subPropertyOf rdf:resource="http://www.w3id.org/efro/efro#hasDescription"/>
        <rdf:type rdf:resource="http://www.w3.org/2002/07/owl#FunctionalProperty"/>
        <rdfs:domain rdf:resource="http://www.w3id.org/efro/efro#WithdrawalReason"/>
        <rdfs:range rdf:resource="http://www.w3.org/2001/XMLSchema#string"/>
        <dcterms:description xml:lang="en">Indicates why a student has withdrawn from a study programme, such as financial difficulties, personal reasons, or transfer to another institution.</dcterms:description>
        <rdfs:label>hasWithdrawReason</rdfs:label>
    </owl:DatatypeProperty>
    


    <!-- http://www.w3id.org/efro/efro#hasWithdrawalDate -->

    <owl:DatatypeProperty rdf:about="http://www.w3id.org/efro/efro#hasWithdrawalDate">
        <rdfs:subPropertyOf rdf:resource="http://www.w3id.org/efro/efro#hasTemporalValue"/>
        <rdfs:domain rdf:resource="http://www.w3id.org/efro/efro#WithdrawalActivity"/>
        <rdfs:range rdf:resource="http://www.w3.org/2001/XMLSchema#dateTime"/>
        <dcterms:description xml:lang="en">Specifies the date when a student officially withdraws from a study programme, impacting funding calculations​.</dcterms:description>
        <rdfs:label>hasWithdrawalDate</rdfs:label>
    </owl:DatatypeProperty>
    


    <!-- http://www.w3id.org/efro/efro#hasWithdrawalFromProgrammeDate -->

    <owl:DatatypeProperty rdf:about="http://www.w3id.org/efro/efro#hasWithdrawalFromProgrammeDate">
        <rdfs:domain rdf:resource="http://www.w3id.org/efro/efro#Student"/>
        <rdfs:range rdf:resource="http://www.w3.org/2001/XMLSchema#dateTime"/>
        <dcterms:description xml:lang="en">Specifies the date when a student officially withdraws from a study programme​.</dcterms:description>
        <rdfs:label>hasWithdrawalFromProgrammeDate</rdfs:label>
    </owl:DatatypeProperty>
    


    <!-- http://www.w3id.org/efro/efro#hasWithdrawnFromEntireProgramme -->

    <owl:DatatypeProperty rdf:about="http://www.w3id.org/efro/efro#hasWithdrawnFromEntireProgramme">
        <rdfs:domain rdf:resource="http://www.w3id.org/efro/efro#Student"/>
        <rdfs:range rdf:resource="http://www.w3.org/2001/XMLSchema#boolean"/>
        <dcterms:description xml:lang="en">A boolean property that denotes whether a student has withdrawn from all learning aims within their study programme​.</dcterms:description>
        <rdfs:label>hasWithdrawnFromEntireProgramme</rdfs:label>
    </owl:DatatypeProperty>
    


    <!-- http://www.w3id.org/efro/efro#isCountedAsGuidedLearning -->

    <owl:DatatypeProperty rdf:about="http://www.w3id.org/efro/efro#isCountedAsGuidedLearning">
        <rdf:type rdf:resource="http://www.w3.org/2002/07/owl#FunctionalProperty"/>
        <rdfs:domain rdf:resource="http://www.w3id.org/efro/efro#Activity"/>
        <rdfs:range rdf:resource="http://www.w3.org/2001/XMLSchema#boolean"/>
        <dcterms:description xml:lang="en">Identifies whether a learning activity qualifies as guided learning hours (GLH) for funding purposes​.</dcterms:description>
        <rdfs:label>isCountedAsGuidedLearning</rdfs:label>
    </owl:DatatypeProperty>
    


    <!-- http://www.w3id.org/efro/efro#isCountedAsPlannedHours -->

    <owl:DatatypeProperty rdf:about="http://www.w3id.org/efro/efro#isCountedAsPlannedHours">
        <rdf:type rdf:resource="http://www.w3.org/2002/07/owl#FunctionalProperty"/>
        <rdfs:domain rdf:resource="http://www.w3id.org/efro/efro#Activity"/>
        <rdfs:range rdf:resource="http://www.w3.org/2001/XMLSchema#boolean"/>
        <dcterms:description xml:lang="en">Determines whether a specific learning activity is included in the total planned hours recorded for funding​.</dcterms:description>
        <rdfs:label>isCountedAsPlannedHours</rdfs:label>
    </owl:DatatypeProperty>
    


    <!-- http://www.w3id.org/efro/efro#isValidLearningActivity -->

    <owl:DatatypeProperty rdf:about="http://www.w3id.org/efro/efro#isValidLearningActivity">
        <rdf:type rdf:resource="http://www.w3.org/2002/07/owl#FunctionalProperty"/>
        <rdfs:domain rdf:resource="http://www.w3id.org/efro/efro#ExaminationActivity"/>
        <rdfs:range rdf:resource="http://www.w3.org/2001/XMLSchema#boolean"/>
        <dcterms:description xml:lang="en">Specifies whether an activity meets the funding body’s criteria for a valid learning activity, ensuring eligibility for funding​.</dcterms:description>
        <rdfs:label>isValidLearningActivity</rdfs:label>
    </owl:DatatypeProperty>
    


    <!-- http://www.w3id.org/efro/efro#progressedInWeek -->

    <owl:DatatypeProperty rdf:about="http://www.w3id.org/efro/efro#progressedInWeek">
        <rdfs:domain rdf:resource="http://www.w3id.org/efro/efro#ProgressionActivity"/>
        <rdfs:range rdf:resource="http://www.w3.org/2001/XMLSchema#integer"/>
    </owl:DatatypeProperty>
    


    <!-- 
    ///////////////////////////////////////////////////////////////////////////////////////
    //
    // Classes
    //
    ///////////////////////////////////////////////////////////////////////////////////////
     -->

    


    <!-- http://purl.org/cerif/frapo/College -->

    <owl:Class rdf:about="http://purl.org/cerif/frapo/College">
        <rdfs:subClassOf rdf:resource="http://www.w3id.org/efro/efro#EducationalInstitution"/>
        <rdfs:subClassOf rdf:resource="http://xmlns.com/foaf/0.1/Organization"/>
    </owl:Class>
    


    <!-- http://purl.org/cerif/frapo/Funding -->

    <owl:Class rdf:about="http://purl.org/cerif/frapo/Funding">
        <rdfs:subClassOf rdf:resource="http://www.w3id.org/efro/efro#FundingElement"/>
    </owl:Class>
    


    <!-- http://purl.org/cerif/frapo/FundingProgramme -->

    <owl:Class rdf:about="http://purl.org/cerif/frapo/FundingProgramme">
        <rdfs:subClassOf rdf:resource="http://www.w3id.org/efro/efro#FundingElement"/>
    </owl:Class>
    


    <!-- http://purl.org/cerif/frapo/ResearchInstitute -->

    <owl:Class rdf:about="http://purl.org/cerif/frapo/ResearchInstitute">
        <owl:equivalentClass rdf:resource="http://purl.org/vocab/aiiso/schema#ResearchGroup"/>
        <rdfs:subClassOf rdf:resource="http://www.w3id.org/efro/efro#EducationalInstitution"/>
        <rdfs:subClassOf rdf:resource="http://xmlns.com/foaf/0.1/Organization"/>
    </owl:Class>
    


    <!-- http://purl.org/cerif/frapo/Status -->

    <owl:Class rdf:about="http://purl.org/cerif/frapo/Status">
        <owl:equivalentClass rdf:resource="http://www.w3id.org/efro/efro#Status"/>
        <rdfs:subClassOf rdf:resource="http://www.w3.org/2002/07/owl#Thing"/>
        <rdfs:comment xml:lang="en">The status of something such as an application, an investigation or a project.</rdfs:comment>
        <rdfs:label xml:lang="en">status</rdfs:label>
    </owl:Class>
    


    <!-- http://purl.org/cerif/frapo/University -->

    <owl:Class rdf:about="http://purl.org/cerif/frapo/University">
        <rdfs:subClassOf rdf:resource="http://www.w3id.org/efro/efro#EducationalInstitution"/>
        <rdfs:subClassOf rdf:resource="http://xmlns.com/foaf/0.1/Organization"/>
    </owl:Class>
    


    <!-- http://purl.org/vocab/aiiso/schema#KnowledgeGrouping -->

    <owl:Class rdf:about="http://purl.org/vocab/aiiso/schema#KnowledgeGrouping"/>
    


    <!-- http://purl.org/vocab/aiiso/schema#Programme -->

    <owl:Class rdf:about="http://purl.org/vocab/aiiso/schema#Programme"/>
    


    <!-- http://purl.org/vocab/aiiso/schema#ResearchGroup -->

    <owl:Class rdf:about="http://purl.org/vocab/aiiso/schema#ResearchGroup"/>
    


    <!-- http://purl.org/vocab/aiiso/schema#School -->

    <owl:Class rdf:about="http://purl.org/vocab/aiiso/schema#School">
        <rdfs:subClassOf rdf:resource="http://www.w3id.org/efro/efro#EducationalInstitution"/>
        <rdfs:subClassOf rdf:resource="http://xmlns.com/foaf/0.1/Organization"/>
    </owl:Class>
    


    <!-- http://www.w3id.org/efro/efro#ASLevel -->

    <owl:Class rdf:about="http://www.w3id.org/efro/efro#ASLevel">
        <rdfs:subClassOf rdf:resource="http://www.w3id.org/efro/efro#Qualification"/>
        <dcterms:description>A standalone qualification representing the first year of A Level study.</dcterms:description>
        <rdfs:label>ASLevel</rdfs:label>
        <skos:example>AS Level qualifications in Mathematics or English.</skos:example>
    </owl:Class>
    


    <!-- http://www.w3id.org/efro/efro#AcademicProgressionActivity -->

    <owl:Class rdf:about="http://www.w3id.org/efro/efro#AcademicProgressionActivity">
        <rdfs:subClassOf rdf:resource="http://www.w3id.org/efro/efro#ProgressionActivity"/>
        <dcterms:description>Progression activities focusing on advancing a student’s academic qualifications or study program.</dcterms:description>
        <rdfs:label>AcademicProgressionActivity</rdfs:label>
    </owl:Class>
    


    <!-- http://www.w3id.org/efro/efro#AcademicYear -->

    <owl:Class rdf:about="http://www.w3id.org/efro/efro#AcademicYear">
        <rdfs:subClassOf rdf:resource="http://www.w3id.org/efro/efro#TimePeriod"/>
        <dcterms:description>A standard 12-month period during which educational activities occur, typically running from September to August.</dcterms:description>
        <rdfs:label>AcademicYear</rdfs:label>
        <skos:example>The academic year structure used to plan funding, timetables, and reporting for study programs​.</skos:example>
    </owl:Class>
    


    <!-- http://www.w3id.org/efro/efro#AchievementStatus -->

    <owl:Class rdf:about="http://www.w3id.org/efro/efro#AchievementStatus">
        <rdfs:subClassOf rdf:resource="http://www.w3id.org/efro/efro#Status"/>
        <dcterms:description>The status reflecting whether a student has achieved the intended outcomes of their study program or qualification.</dcterms:description>
        <rdfs:label>AchievementStatus</rdfs:label>
    </owl:Class>
    


    <!-- http://www.w3id.org/efro/efro#ActiveParticipationStatus -->

    <owl:Class rdf:about="http://www.w3id.org/efro/efro#ActiveParticipationStatus">
        <rdfs:subClassOf rdf:resource="http://www.w3id.org/efro/efro#ParticipationStatus"/>
        <dcterms:description>Indicates that the student is actively engaging in their study program.</dcterms:description>
        <rdfs:label>ActiveParticipationStatus</rdfs:label>
        <skos:example>Active participation demonstrated through attendance and assignment submissions​.</skos:example>
    </owl:Class>
    


    <!-- http://www.w3id.org/efro/efro#ActiveStatus -->

    <owl:Class rdf:about="http://www.w3id.org/efro/efro#ActiveStatus">
        <rdfs:subClassOf rdf:resource="http://www.w3id.org/efro/efro#EnrollmentStatus"/>
        <owl:disjointWith rdf:resource="http://www.w3id.org/efro/efro#WithdrawnStatus"/>
        <dcterms:description>Indicates that the student is actively enrolled and participating in their study program.</dcterms:description>
        <rdfs:label>ActiveStatus</rdfs:label>
        <skos:example>Students attending planned hours and meeting progression milestones.</skos:example>
    </owl:Class>
    


    <!-- http://www.w3id.org/efro/efro#Activity -->

    <owl:Class rdf:about="http://www.w3id.org/efro/efro#Activity">
        <dcterms:description xml:lang="en">Represents any task, process, or event associated with administering, managing, or supporting educational programs and funding compliance. It serves as the parent class for specialized activities related to attendance, progression, recording, withdrawal, and enrollment.</dcterms:description>
        <rdfs:label>Activity</rdfs:label>
    </owl:Class>
    


    <!-- http://www.w3id.org/efro/efro#ActualAttendanceActivity -->

    <owl:Class rdf:about="http://www.w3id.org/efro/efro#ActualAttendanceActivity">
        <rdfs:subClassOf rdf:resource="http://www.w3id.org/efro/efro#AttendanceActivity"/>
        <dcterms:description>The actual participation or presence of a student in scheduled study programs or activities.</dcterms:description>
        <rdfs:label>ActualAttendanceActivity</rdfs:label>
        <skos:example>Weekly attendance logs submitted for ESFA compliance.</skos:example>
    </owl:Class>
    


    <!-- http://www.w3id.org/efro/efro#ActualAttendancePeriod -->

    <owl:Class rdf:about="http://www.w3id.org/efro/efro#ActualAttendancePeriod">
        <rdfs:subClassOf rdf:resource="http://www.w3id.org/efro/efro#LearningAspect"/>
        <dcterms:description>The period during which a student has actively participated in their study program.</dcterms:description>
        <rdfs:label>ActualAttendancePeriod</rdfs:label>
        <skos:example>Attendance records used for funding validation​.</skos:example>
    </owl:Class>
    


    <!-- http://www.w3id.org/efro/efro#AdjustedPlannedHours -->

    <owl:Class rdf:about="http://www.w3id.org/efro/efro#AdjustedPlannedHours">
        <rdfs:subClassOf rdf:resource="http://www.w3id.org/efro/efro#PlannedHours"/>
        <dcterms:description>Revised planned hours to reflect changes in the student’s program, such as early completion or withdrawal.</dcterms:description>
        <rdfs:label>AdjustedPlannedHours</rdfs:label>
        <skos:example>Reduced hours due to a student completing a program early​.</skos:example>
    </owl:Class>
    


    <!-- http://www.w3id.org/efro/efro#AdministrativeActivity -->

    <owl:Class rdf:about="http://www.w3id.org/efro/efro#AdministrativeActivity">
        <rdfs:subClassOf rdf:resource="http://www.w3id.org/efro/efro#Activity"/>
        <dcterms:description xml:lang="en">Covers activities related to the management and administration of funding compliance, institutional governance, and student records.en</dcterms:description>
        <rdfs:label>AdministrativeActivity</rdfs:label>
    </owl:Class>
    


    <!-- http://www.w3id.org/efro/efro#AdministrativeMeeting -->

    <owl:Class rdf:about="http://www.w3id.org/efro/efro#AdministrativeMeeting">
        <rdfs:subClassOf rdf:resource="http://www.w3id.org/efro/efro#GeneralAssistanceActivity"/>
        <owl:disjointWith rdf:resource="http://www.w3id.org/efro/efro#GuidedLearning"/>
        <rdfs:comment>Meeting for general administrative or attendance discussion that cannot be counted as planned hours or used as withdrawal date.</rdfs:comment>
        <rdfs:label>AdministrativeMeeting</rdfs:label>
    </owl:Class>
    


    <!-- http://www.w3id.org/efro/efro#AdministrativeStaff -->

    <owl:Class rdf:about="http://www.w3id.org/efro/efro#AdministrativeStaff">
        <rdfs:subClassOf rdf:resource="http://www.w3id.org/efro/efro#Staff"/>
        <dcterms:description>Staff responsible for managing records, compliance, and administrative tasks to meet ESFA funding and reporting requirements.</dcterms:description>
        <rdfs:label>AdministrativeStaff</rdfs:label>
        <skos:example>Staff members responsible for submitting ILR data and maintaining attendance records.</skos:example>
    </owl:Class>
    


    <!-- http://www.w3id.org/efro/efro#AfterInitialSixWeeks -->

    <owl:Class rdf:about="http://www.w3id.org/efro/efro#AfterInitialSixWeeks">
        <rdfs:subClassOf rdf:resource="http://www.w3id.org/efro/efro#TimeCondition"/>
        <dcterms:description>A time condition indicating the period after the initial six weeks of a program. This is often used to determine funding eligibility, as students retained beyond this period qualify for funding.</dcterms:description>
        <rdfs:label>AfterInitialSixWeeks</rdfs:label>
        <skos:example>Funding claims are validated for students continuing their study program after the initial six-week period.</skos:example>
    </owl:Class>
    


    <!-- http://www.w3id.org/efro/efro#Apprentice -->

    <owl:Class rdf:about="http://www.w3id.org/efro/efro#Apprentice">
        <rdfs:subClassOf rdf:resource="http://www.w3id.org/efro/efro#Participant"/>
        <dcterms:description>A participant enrolled in an apprenticeship program that combines work-based training with classroom instruction, funded through apprenticeship standards.</dcterms:description>
        <rdfs:label>Apprentice</rdfs:label>
        <skos:example>A digital marketing apprentice completing an ESFA-funded apprenticeship​.</skos:example>
    </owl:Class>
    


    <!-- http://www.w3id.org/efro/efro#ApprenticeshipFunding -->

    <owl:Class rdf:about="http://www.w3id.org/efro/efro#ApprenticeshipFunding">
        <rdfs:subClassOf rdf:resource="http://www.w3id.org/efro/efro#FundingType"/>
        <dcterms:description>Funding allocated for apprenticeship programs, which combine on-the-job training with classroom learning.</dcterms:description>
        <rdfs:label>ApprenticeshipFunding</rdfs:label>
        <skos:example>Funding caps and bands specific to apprenticeship standards and frameworks.</skos:example>
    </owl:Class>
    


    <!-- http://www.w3id.org/efro/efro#ApprenticeshipProgramme -->

    <owl:Class rdf:about="http://www.w3id.org/efro/efro#ApprenticeshipProgramme">
        <rdfs:subClassOf rdf:resource="http://www.w3id.org/efro/efro#StudyProgramme"/>
        <dcterms:description>A study program that combines on-the-job training with classroom learning, leading to recognized apprenticeship qualifications.</dcterms:description>
        <rdfs:label>ApprenticeshipProgramme</rdfs:label>
        <skos:example>Apprenticeships in digital marketing or construction.</skos:example>
    </owl:Class>
    


    <!-- http://www.w3id.org/efro/efro#ApprenticeshipProgression -->

    <owl:Class rdf:about="http://www.w3id.org/efro/efro#ApprenticeshipProgression">
        <rdfs:subClassOf rdf:resource="http://www.w3id.org/efro/efro#ProgressionType"/>
        <dcterms:description xml:lang="en">Represents a student&apos;s transition from a study programme to an apprenticeship scheme.</dcterms:description>
        <rdfs:label>ApprenticeshipProgression</rdfs:label>
    </owl:Class>
    


    <!-- http://www.w3id.org/efro/efro#ApprenticeshipProvider -->

    <owl:Class rdf:about="http://www.w3id.org/efro/efro#ApprenticeshipProvider">
        <rdfs:subClassOf rdf:resource="http://www.w3id.org/efro/efro#EducationProvider"/>
        <dcterms:description>A provider specializing in delivering apprenticeship programs that combine workplace training with educational components. These providers must comply with ESFA funding rules for apprenticeships.</dcterms:description>
        <rdfs:label>ApprenticeshipProvider</rdfs:label>
        <skos:example>Apprenticeship providers must ensure that work placements and educational content meet compliance standards for funding​</skos:example>
    </owl:Class>
    


    <!-- http://www.w3id.org/efro/efro#ApprenticeshipQualification -->

    <owl:Class rdf:about="http://www.w3id.org/efro/efro#ApprenticeshipQualification">
        <rdfs:subClassOf rdf:resource="http://www.w3id.org/efro/efro#Qualification"/>
        <dcterms:description>Qualifications awarded for completing apprenticeship standards or frameworks.</dcterms:description>
        <rdfs:label>ApprenticeshipQualification</rdfs:label>
        <skos:example>Level 3 Engineering Technician Standard​.</skos:example>
    </owl:Class>
    


    <!-- http://www.w3id.org/efro/efro#AssessmentActivity -->

    <owl:Class rdf:about="http://www.w3id.org/efro/efro#AssessmentActivity">
        <rdfs:subClassOf rdf:resource="http://www.w3id.org/efro/efro#Activity"/>
        <dcterms:description xml:lang="en">Covers activities related to evaluating student progress, performance, and completion of educational aims.</dcterms:description>
        <rdfs:label>AssessmentActivity</rdfs:label>
    </owl:Class>
    


    <!-- http://www.w3id.org/efro/efro#AssignmentActivity -->

    <owl:Class rdf:about="http://www.w3id.org/efro/efro#AssignmentActivity">
        <rdfs:subClassOf rdf:resource="http://www.w3id.org/efro/efro#AssessmentActivity"/>
        <dcterms:description xml:lang="en">Involves the planning, submission, and grading of assignments as part of a student’s learning or qualification aim.</dcterms:description>
        <rdfs:label>AssignmentActivity</rdfs:label>
        <skos:example xml:lang="en">A marked essay that contributes to the student’s qualification​.</skos:example>
    </owl:Class>
    


    <!-- http://www.w3id.org/efro/efro#AttendanceActivity -->

    <owl:Class rdf:about="http://www.w3id.org/efro/efro#AttendanceActivity">
        <rdfs:subClassOf rdf:resource="http://www.w3id.org/efro/efro#Activity"/>
        <dcterms:description>Covers activities related to tracking, recording, and managing student attendance for compliance and funding purposes.</dcterms:description>
        <rdfs:label>AttendanceActivity</rdfs:label>
    </owl:Class>
    


    <!-- http://www.w3id.org/efro/efro#AttendanceReport -->

    <owl:Class rdf:about="http://www.w3id.org/efro/efro#AttendanceReport">
        <rdfs:subClassOf rdf:resource="http://www.w3id.org/efro/efro#ReportDocument"/>
        <dcterms:description>A document summarizing student attendance over a defined period. It serves as evidence of engagement and retention for funding purposes.</dcterms:description>
        <rdfs:label>AttendanceReport</rdfs:label>
        <skos:example>Reports generated from class registers or attendance monitoring systems for audit purposes.</skos:example>
    </owl:Class>
    


    <!-- http://www.w3id.org/efro/efro#AttendanceStatus -->

    <owl:Class rdf:about="http://www.w3id.org/efro/efro#AttendanceStatus">
        <rdfs:subClassOf rdf:resource="http://www.w3id.org/efro/efro#Status"/>
        <dcterms:description>Reflects the attendance record of a student, including periods of active participation and absences.</dcterms:description>
        <rdfs:label>AttendanceStatus</rdfs:label>
        <skos:example>Students with attendance below the threshold may not qualify for full funding.</skos:example>
    </owl:Class>
    


    <!-- http://www.w3id.org/efro/efro#AuditDocument -->

    <owl:Class rdf:about="http://www.w3id.org/efro/efro#AuditDocument">
        <rdfs:subClassOf rdf:resource="http://www.w3id.org/efro/efro#ComplianceDocument"/>
        <dcterms:description>A document produced for or during an audit to validate compliance with ESFA funding regulations. It includes records that justify funding claims, attendance, planned hours, and other institutional obligations as outlined in the guidance.</dcterms:description>
        <rdfs:label>AuditDocument</rdfs:label>
        <skos:example>Documents demonstrating compliance with planned hours or evidence of student eligibility during audits.</skos:example>
    </owl:Class>
    


    <!-- http://www.w3id.org/efro/efro#Authority -->

    <owl:Class rdf:about="http://www.w3id.org/efro/efro#Authority">
        <rdfs:subClassOf rdf:resource="http://www.w3id.org/efro/efro#EducationalEntity"/>
        <dcterms:description>A governing or administrative entity responsible for overseeing and ensuring compliance with educational policies, funding regulations, and operational standards.</dcterms:description>
        <rdfs:label>Authority</rdfs:label>
    </owl:Class>
    


    <!-- http://www.w3id.org/efro/efro#BeforeQualifyingStartPeriod -->

    <owl:Class rdf:about="http://www.w3id.org/efro/efro#BeforeQualifyingStartPeriod">
        <rdfs:subClassOf rdf:resource="http://www.w3id.org/efro/efro#TimeCondition"/>
        <dcterms:description>A time condition representing activities or periods that occur before the qualifying start period. This period does not count towards funding eligibility or compliance.</dcterms:description>
        <rdfs:label>BeforeQualifyingStartPeriod</rdfs:label>
        <skos:example>Activities undertaken by a student before their formal enrollment or qualifying attendance period.</skos:example>
    </owl:Class>
    


    <!-- http://www.w3id.org/efro/efro#ClassRegister -->

    <owl:Class rdf:about="http://www.w3id.org/efro/efro#ClassRegister">
        <rdfs:subClassOf rdf:resource="http://www.w3id.org/efro/efro#RecordDocument"/>
        <dcterms:description>A document recording student attendance for specific sessions, including details like the date, time, duration, and tutor information. This is key evidence for compliance with funding regulations.</dcterms:description>
        <rdfs:label>ClassRegister</rdfs:label>
        <skos:example>Registers showing attendance during in-person or virtual sessions, signed by tutors or verified electronically.</skos:example>
    </owl:Class>
    


    <!-- http://www.w3id.org/efro/efro#CollegeStaff -->

    <owl:Class rdf:about="http://www.w3id.org/efro/efro#CollegeStaff">
        <rdfs:subClassOf rdf:resource="http://www.w3id.org/efro/efro#Staff"/>
        <dcterms:description>Employees working in a college setting, including administrative, teaching, and support staff, who ensure compliance with ESFA regulations.</dcterms:description>
        <rdfs:label>CollegeStaff</rdfs:label>
        <skos:example>compliance officer ensuring adherence to planned hours and funding requirements in a college​.</skos:example>
    </owl:Class>
    


    <!-- http://www.w3id.org/efro/efro#CompletedEarlyStatus -->

    <owl:Class rdf:about="http://www.w3id.org/efro/efro#CompletedEarlyStatus">
        <rdfs:subClassOf rdf:resource="http://www.w3id.org/efro/efro#CompletionStatus"/>
        <dcterms:description>Status showing the student completed their study program ahead of the planned schedule.</dcterms:description>
        <rdfs:label>CompletedEarlyStatus</rdfs:label>
        <skos:example>Early completion adjustments are applied to funding in such cases​.</skos:example>
    </owl:Class>
    


    <!-- http://www.w3id.org/efro/efro#CompletedSuccessfullyStatus -->

    <owl:Class rdf:about="http://www.w3id.org/efro/efro#CompletedSuccessfullyStatus">
        <rdfs:subClassOf rdf:resource="http://www.w3id.org/efro/efro#CompletionStatus"/>
        <dcterms:description>Indicates the successful completion of the program, including achieving all learning aims.</dcterms:description>
        <rdfs:label>CompletedSuccessfullyStatus</rdfs:label>
        <skos:example>Students completing their qualifications with satisfactory attendance and assessment completion.</skos:example>
    </owl:Class>
    


    <!-- http://www.w3id.org/efro/efro#CompletionActivity -->

    <owl:Class rdf:about="http://www.w3id.org/efro/efro#CompletionActivity">
        <rdfs:subClassOf rdf:resource="http://www.w3id.org/efro/efro#Activity"/>
        <dcterms:description>Activities related to the successful or partial completion of a study program or educational objective.</dcterms:description>
        <rdfs:label>CompletionActivity</rdfs:label>
    </owl:Class>
    


    <!-- http://www.w3id.org/efro/efro#CompletionStatus -->

    <owl:Class rdf:about="http://www.w3id.org/efro/efro#CompletionStatus">
        <rdfs:subClassOf rdf:resource="http://www.w3id.org/efro/efro#Status"/>
        <dcterms:description>Indicates whether a student has completed their study program as planned, early, or not at all.</dcterms:description>
        <rdfs:label>CompletionStatus</rdfs:label>
    </owl:Class>
    


    <!-- http://www.w3id.org/efro/efro#ComplianceCriterion -->

    <owl:Class rdf:about="http://www.w3id.org/efro/efro#ComplianceCriterion">
        <rdfs:label>Compliance Criterion</rdfs:label>
    </owl:Class>
    


    <!-- http://www.w3id.org/efro/efro#ComplianceDocument -->

    <owl:Class rdf:about="http://www.w3id.org/efro/efro#ComplianceDocument">
        <rdfs:subClassOf rdf:resource="http://www.w3id.org/efro/efro#Document"/>
        <dcterms:description>A category of documents specifically focused on meeting regulatory, legal, and funding requirements. These documents ensure adherence to the ESFA guidelines and audit standards.</dcterms:description>
        <rdfs:label>ComplianceDocument</rdfs:label>
    </owl:Class>
    


    <!-- http://www.w3id.org/efro/efro#ComplianceObligation -->

    <owl:Class rdf:about="http://www.w3id.org/efro/efro#ComplianceObligation">
        <rdfs:subClassOf rdf:resource="http://www.w3id.org/efro/efro#Obligation"/>
        <dcterms:description>A requirement to adhere to funding and regulatory guidelines to ensure that funding is used appropriately and that study programs meet the required standards.</dcterms:description>
        <rdfs:label>ComplianceObligation</rdfs:label>
        <skos:example>Ensuring planned hours are accurately recorded, students meet qualifying criteria, and institutions adhere to audit requirements​.</skos:example>
    </owl:Class>
    


    <!-- http://www.w3id.org/efro/efro#ContinueFunding -->

    <owl:Class rdf:about="http://www.w3id.org/efro/efro#ContinueFunding">
        <rdfs:subClassOf rdf:resource="http://www.w3id.org/efro/efro#FundingImpact"/>
        <rdfs:label>Continue Funding</rdfs:label>
    </owl:Class>
    


    <!-- http://www.w3id.org/efro/efro#ContinuingStatus -->

    <owl:Class rdf:about="http://www.w3id.org/efro/efro#ContinuingStatus">
        <rdfs:subClassOf rdf:resource="http://www.w3id.org/efro/efro#ProgressionStatus"/>
        <dcterms:description>Indicates that the student is progressing as planned within their current study program.</dcterms:description>
        <rdfs:label>ContinuingStatus</rdfs:label>
        <skos:example>A student moving from Year 1 to Year 2 of their T Level program.</skos:example>
    </owl:Class>
    


    <!-- http://www.w3id.org/efro/efro#DateOfWithdrawal -->

    <owl:Class rdf:about="http://www.w3id.org/efro/efro#DateOfWithdrawal">
        <rdfs:subClassOf rdf:resource="http://www.w3id.org/efro/efro#TimePoint"/>
        <dcterms:description>The specific date on which a student withdraws from their study program. This date is critical for recalculating funding claims.</dcterms:description>
        <rdfs:label>DateOfWithdrawal</rdfs:label>
        <skos:example>Withdrawal forms must specify the official date of withdrawal for funding adjustments.</skos:example>
    </owl:Class>
    


    <!-- http://www.w3id.org/efro/efro#DistanceLearningProvision -->

    <owl:Class rdf:about="http://www.w3id.org/efro/efro#DistanceLearningProvision">
        <rdfs:subClassOf rdf:resource="http://www.w3id.org/efro/efro#LearningMode"/>
        <owl:disjointWith rdf:resource="http://www.w3id.org/efro/efro#TraditionalProvision"/>
        <dcterms:description>Learning activities delivered remotely, typically through online platforms, without the need for physical attendance.</dcterms:description>
        <rdfs:label>DistanceLearningProvision</rdfs:label>
        <skos:example>Online modules for students unable to attend in person​.</skos:example>
    </owl:Class>
    


    <!-- http://www.w3id.org/efro/efro#Document -->

    <owl:Class rdf:about="http://www.w3id.org/efro/efro#Document">
        <owl:equivalentClass rdf:resource="http://xmlns.com/foaf/0.1/Document"/>
        <rdfs:subClassOf rdf:resource="http://www.w3id.org/efro/efro#Evidence"/>
        <dcterms:description>Represents any formal written, electronic, or recorded material used to support compliance, funding, audit, and administrative processes. Documents in this hierarchy serve as evidence, records, or reports within the educational context.</dcterms:description>
        <rdfs:label>Document</rdfs:label>
    </owl:Class>
    


    <!-- http://www.w3id.org/efro/efro#DocumentationActivity -->

    <owl:Class rdf:about="http://www.w3id.org/efro/efro#DocumentationActivity">
        <rdfs:subClassOf rdf:resource="http://www.w3id.org/efro/efro#AdministrativeActivity"/>
        <dcterms:description xml:lang="en">The process of creating, collecting, and maintaining records and documents to support compliance with funding, attendance, and progression requirements.</dcterms:description>
        <rdfs:label>DocumentationActivity</rdfs:label>
        <skos:example xml:lang="en">Maintaining funding evidence documents for audits.</skos:example>
    </owl:Class>
    


    <!-- http://www.w3id.org/efro/efro#DoubleFundingRestriction -->

    <owl:Class rdf:about="http://www.w3id.org/efro/efro#DoubleFundingRestriction">
        <rdfs:subClassOf rdf:resource="http://www.w3id.org/efro/efro#FundingCondition"/>
        <dcterms:description>A restriction preventing institutions from claiming funding for the same student or activity from multiple sources.</dcterms:description>
        <rdfs:label>DoubleFundingRestriction</rdfs:label>
        <skos:example>Restrictions ensuring that students enrolled in apprenticeship programs are not double-funded through other ESFA-funded programs​.</skos:example>
    </owl:Class>
    


    <!-- http://www.w3id.org/efro/efro#ESFAFunding -->

    <owl:Class rdf:about="http://www.w3id.org/efro/efro#ESFAFunding">
        <rdfs:subClassOf rdf:resource="http://www.w3id.org/efro/efro#FundingType"/>
        <dcterms:description>General funding provided by the ESFA for study programs, qualifications, and institutional support.</dcterms:description>
        <rdfs:label>ESFAFunding</rdfs:label>
        <skos:example>16-19 study program funding, including high-needs student allocations​.</skos:example>
    </owl:Class>
    


    <!-- http://www.w3id.org/efro/efro#EarlyCompletionActivity -->

    <owl:Class rdf:about="http://www.w3id.org/efro/efro#EarlyCompletionActivity">
        <rdfs:subClassOf rdf:resource="http://www.w3id.org/efro/efro#CompletionActivity"/>
        <dcterms:description>An activity involving the completion of a program or objective earlier than the planned schedule.</dcterms:description>
        <rdfs:label>EarlyCompletionActivity</rdfs:label>
        <skos:example>Adjusting funding claims for students who complete qualifications ahead of schedule​.</skos:example>
    </owl:Class>
    


    <!-- http://www.w3id.org/efro/efro#EarlyCompletionAdjustment -->

    <owl:Class rdf:about="http://www.w3id.org/efro/efro#EarlyCompletionAdjustment">
        <rdfs:subClassOf rdf:resource="http://www.w3id.org/efro/efro#FundingAdjustment"/>
        <dcterms:description>An adjustment applied when a student completes their program earlier than planned. Funding is recalculated based on the actual duration of attendance and the completion criteria.</dcterms:description>
        <rdfs:label>EarlyCompletionAdjustment</rdfs:label>
        <skos:example>A reduced funding claim if a student achieves their qualification ahead of schedule without completing the planned hours​.</skos:example>
    </owl:Class>
    


    <!-- http://www.w3id.org/efro/efro#EarlyCompletionStatus -->

    <owl:Class rdf:about="http://www.w3id.org/efro/efro#EarlyCompletionStatus">
        <rdfs:subClassOf rdf:resource="http://www.w3id.org/efro/efro#AchievementStatus"/>
        <dcterms:description>Indicates that a student has completed their qualification or study program earlier than the planned duration.</dcterms:description>
        <rdfs:label>EarlyCompletionStatus</rdfs:label>
        <skos:example>A student completing their apprenticeship program ahead of schedule​.</skos:example>
    </owl:Class>
    


    <!-- http://www.w3id.org/efro/efro#EducationProvider -->

    <owl:Class rdf:about="http://www.w3id.org/efro/efro#EducationProvider">
        <rdfs:subClassOf rdf:resource="http://www.w3id.org/efro/efro#EducationalEntity"/>
        <rdfs:subClassOf rdf:resource="http://xmlns.com/foaf/0.1/Organization"/>
        <dcterms:description>An organization that delivers educational programs, apprenticeships, or training services. Providers are responsible for meeting funding conditions and delivering high-quality education.</dcterms:description>
        <rdfs:label>Education Provider</rdfs:label>
    </owl:Class>
    


    <!-- http://www.w3id.org/efro/efro#EducationalEntity -->

    <owl:Class rdf:about="http://www.w3id.org/efro/efro#EducationalEntity">
        <owl:equivalentClass rdf:resource="http://xmlns.com/foaf/0.1/Organization"/>
        <dcterms:description>Represents any organization, body, or institution involved in the delivery, regulation, or oversight of education, training, and funding processes.</dcterms:description>
        <rdfs:label>EducationalEntity</rdfs:label>
    </owl:Class>
    


    <!-- http://www.w3id.org/efro/efro#EducationalInstitution -->

    <owl:Class rdf:about="http://www.w3id.org/efro/efro#EducationalInstitution">
        <rdfs:subClassOf rdf:resource="http://www.w3id.org/efro/efro#Institution"/>
        <rdfs:label>EducationalInstitution</rdfs:label>
    </owl:Class>
    


    <!-- http://www.w3id.org/efro/efro#EducationalProvider -->

    <owl:Class rdf:about="http://www.w3id.org/efro/efro#EducationalProvider">
        <rdfs:subClassOf rdf:resource="http://www.w3id.org/efro/efro#EducationProvider"/>
        <dcterms:description>A provider delivering general education programs, including study programs for students aged 16 to 19 or those with Education, Health, and Care (EHC) plans.</dcterms:description>
        <rdfs:label>EducationalProvider</rdfs:label>
        <skos:example>Colleges offering T Level programs or academic qualifications such as A Levels​</skos:example>
    </owl:Class>
    


    <!-- http://www.w3id.org/efro/efro#EmploymentProgressionActivity -->

    <owl:Class rdf:about="http://www.w3id.org/efro/efro#EmploymentProgressionActivity">
        <rdfs:subClassOf rdf:resource="http://www.w3id.org/efro/efro#ProgressionActivity"/>
        <dcterms:description>Activities that facilitate transitioning into employment, including work-based training.</dcterms:description>
        <rdfs:label>EmploymentProgressionActivity</rdfs:label>
    </owl:Class>
    


    <!-- http://www.w3id.org/efro/efro#EnrollmentActivity -->

    <owl:Class rdf:about="http://www.w3id.org/efro/efro#EnrollmentActivity">
        <rdfs:subClassOf rdf:resource="http://www.w3id.org/efro/efro#Activity"/>
        <dcterms:description>Covers all activities associated with registering or enrolling students into educational programs.</dcterms:description>
        <rdfs:label>EnrollmentActivity</rdfs:label>
    </owl:Class>
    


    <!-- http://www.w3id.org/efro/efro#EnrollmentStatus -->

    <owl:Class rdf:about="http://www.w3id.org/efro/efro#EnrollmentStatus">
        <rdfs:subClassOf rdf:resource="http://www.w3id.org/efro/efro#Status"/>
        <dcterms:description>Reflects the enrollment state of a student within a study program.</dcterms:description>
        <rdfs:label>EnrollmentStatus</rdfs:label>
    </owl:Class>
    


    <!-- http://www.w3id.org/efro/efro#Evidence -->

    <owl:Class rdf:about="http://www.w3id.org/efro/efro#Evidence">
        <rdfs:label>Evidence</rdfs:label>
    </owl:Class>
    


    <!-- http://www.w3id.org/efro/efro#ExaminationActivity -->

    <owl:Class rdf:about="http://www.w3id.org/efro/efro#ExaminationActivity">
        <rdfs:subClassOf rdf:resource="http://www.w3id.org/efro/efro#AssessmentActivity"/>
        <dcterms:description xml:lang="en">Activities related to administering, grading, and recording examinations.en</dcterms:description>
        <rdfs:comment>Assessment of student achievement that counts as learning activity</rdfs:comment>
        <rdfs:label>ExaminationActivity</rdfs:label>
        <skos:example xml:lang="en">Formal assessments conducted for qualifications such as GCSEs or vocational qualifications.</skos:example>
    </owl:Class>
    


    <!-- http://www.w3id.org/efro/efro#ExaminationDate -->

    <owl:Class rdf:about="http://www.w3id.org/efro/efro#ExaminationDate">
        <rdfs:subClassOf rdf:resource="http://www.w3id.org/efro/efro#TimePoint"/>
        <dcterms:description>The date on which a student completes a formal examination as part of their study program.</dcterms:description>
        <rdfs:label>ExaminationDate</rdfs:label>
        <skos:example>Institutions report examination dates for students completing final assessments​.</skos:example>
    </owl:Class>
    


    <!-- http://www.w3id.org/efro/efro#ExcludedHours -->

    <owl:Class rdf:about="http://www.w3id.org/efro/efro#ExcludedHours">
        <rdfs:subClassOf rdf:resource="http://www.w3id.org/efro/efro#PlannedHours"/>
        <dcterms:description>ours excluded from funding calculations, such as breaks or activities not eligible for funding.</dcterms:description>
        <rdfs:label>ExcludedHours</rdfs:label>
        <skos:example>Meal breaks or voluntary extracurricular activities​.</skos:example>
    </owl:Class>
    


    <!-- http://www.w3id.org/efro/efro#ExitedStatus -->

    <owl:Class rdf:about="http://www.w3id.org/efro/efro#ExitedStatus">
        <rdfs:subClassOf rdf:resource="http://www.w3id.org/efro/efro#ProgressionStatus"/>
        <dcterms:description>Indicates that the student has exited the program before completion, potentially for personal reasons, employment, or transfer.</dcterms:description>
        <rdfs:label>ExitedStatus</rdfs:label>
        <skos:example>A student leaving to join an apprenticeship before completing their current program​.</skos:example>
    </owl:Class>
    


    <!-- http://www.w3id.org/efro/efro#FinanciallyRelatedInstitution -->

    <owl:Class rdf:about="http://www.w3id.org/efro/efro#FinanciallyRelatedInstitution">
        <rdfs:subClassOf rdf:resource="http://www.w3id.org/efro/efro#Institution"/>
        <dcterms:description>An institution with financial relationships tied to funding agreements, including direct funding from the ESFA or through subcontracting arrangements.</dcterms:description>
        <rdfs:label>FinanciallyRelatedInstitution</rdfs:label>
        <skos:example>Colleges or academies receiving ESFA funding for study programs</skos:example>
    </owl:Class>
    


    <!-- http://www.w3id.org/efro/efro#FirstDateOfAttendance -->

    <owl:Class rdf:about="http://www.w3id.org/efro/efro#FirstDateOfAttendance">
        <rdfs:subClassOf rdf:resource="http://www.w3id.org/efro/efro#TimePoint"/>
        <dcterms:description>The date when a student first attends their study program, marking the start of their qualifying attendance period.</dcterms:description>
        <rdfs:label>FirstDateOfAttendance</rdfs:label>
        <skos:example>The first date of attendance must align with the planned program start for funding validation​.</skos:example>
    </owl:Class>
    


    <!-- http://www.w3id.org/efro/efro#FullTimeEducationProgression -->

    <owl:Class rdf:about="http://www.w3id.org/efro/efro#FullTimeEducationProgression">
        <rdfs:subClassOf rdf:resource="http://www.w3id.org/efro/efro#ProgressionType"/>
        <dcterms:description xml:lang="en">Represents a student&apos;s transition from one level of full-time education to another, such as moving from secondary education to further education or higher education.</dcterms:description>
        <rdfs:label>FullTimeEducationProgression</rdfs:label>
    </owl:Class>
    


    <!-- http://www.w3id.org/efro/efro#FullTimeProgram -->

    <owl:Class rdf:about="http://www.w3id.org/efro/efro#FullTimeProgram">
        <owl:equivalentClass>
            <owl:Class>
                <owl:intersectionOf rdf:parseType="Collection">
                    <rdf:Description rdf:about="http://www.w3id.org/efro/efro#StudyProgramme"/>
                    <owl:Restriction>
                        <owl:onProperty rdf:resource="http://www.w3id.org/efro/efro#hasHoursPlanned"/>
                        <owl:someValuesFrom>
                            <rdfs:Datatype>
                                <owl:onDatatype rdf:resource="http://www.w3.org/2001/XMLSchema#integer"/>
                                <owl:withRestrictions rdf:parseType="Collection">
                                    <rdf:Description>
                                        <xsd:minInclusive rdf:datatype="http://www.w3.org/2001/XMLSchema#integer">540</xsd:minInclusive>
                                    </rdf:Description>
                                </owl:withRestrictions>
                            </rdfs:Datatype>
                        </owl:someValuesFrom>
                    </owl:Restriction>
                </owl:intersectionOf>
            </owl:Class>
        </owl:equivalentClass>
        <rdfs:subClassOf rdf:resource="http://www.w3id.org/efro/efro#StudyProgramme"/>
        <dcterms:description>A study program requiring 540 or more planned hours over an academic year, meeting the criteria for full-time funding.</dcterms:description>
        <rdfs:label>FullTimeProgram</rdfs:label>
        <skos:example>A full-time A Level program for 16-19 students​.</skos:example>
    </owl:Class>
    


    <!-- http://www.w3id.org/efro/efro#FullTimeStudent -->

    <owl:Class rdf:about="http://www.w3id.org/efro/efro#FullTimeStudent">
        <rdfs:subClassOf rdf:resource="http://www.w3id.org/efro/efro#Student"/>
        <owl:disjointWith rdf:resource="http://www.w3id.org/efro/efro#PartTimeStudent"/>
        <dcterms:description>A student enrolled in a study program with 540 or more planned hours over an academic year, qualifying as full-time under ESFA funding rules.</dcterms:description>
        <rdfs:label>FullTimeStudent</rdfs:label>
        <skos:example>A student enrolled in a full-time T Level program​.</skos:example>
    </owl:Class>
    


    <!-- http://www.w3id.org/efro/efro#FundedInstitution -->

    <owl:Class rdf:about="http://www.w3id.org/efro/efro#FundedInstitution">
        <rdfs:subClassOf rdf:resource="http://www.w3id.org/efro/efro#Institution"/>
        <dcterms:description>An institution directly receiving funding from the ESFA to deliver educational programs that comply with the regulations outlined in the funding guidance.</dcterms:description>
        <rdfs:label>FundedInstitution</rdfs:label>
        <skos:example>FE colleges and sixth forms funded to provide study programs for students aged 16 to 19</skos:example>
    </owl:Class>
    


    <!-- http://www.w3id.org/efro/efro#FundedStatus -->

    <owl:Class rdf:about="http://www.w3id.org/efro/efro#FundedStatus">
        <rdfs:subClassOf rdf:resource="http://www.w3id.org/efro/efro#FundingStatus"/>
        <owl:disjointWith rdf:resource="http://www.w3id.org/efro/efro#NonFundedStatus"/>
        <dcterms:description>Indicates that the student or program is fully eligible for ESFA funding.</dcterms:description>
        <rdfs:label>FundedStatus</rdfs:label>
        <skos:example>A 16-19-year-old student meeting all funding criteria for a full-time program.</skos:example>
    </owl:Class>
    


    <!-- http://www.w3id.org/efro/efro#FundedStudent -->

    <owl:Class rdf:about="http://www.w3id.org/efro/efro#FundedStudent">
        <owl:equivalentClass>
            <owl:Class>
                <owl:intersectionOf rdf:parseType="Collection">
                    <rdf:Description rdf:about="http://www.w3id.org/efro/efro#Student"/>
                    <owl:Restriction>
                        <owl:onProperty rdf:resource="http://www.w3id.org/efro/efro#relatedToFundingStatus"/>
                        <owl:someValuesFrom rdf:resource="http://www.w3id.org/efro/efro#FundedStatus"/>
                    </owl:Restriction>
                </owl:intersectionOf>
            </owl:Class>
        </owl:equivalentClass>
        <rdfs:subClassOf rdf:resource="http://www.w3id.org/efro/efro#Student"/>
        <dcterms:description>A student who meets the criteria for ESFA funding and is included in funding claims submitted by an institution.</dcterms:description>
        <rdfs:label>FundedStudent</rdfs:label>
        <skos:example>A 17-year-old enrolled in a vocational qualification funded through the 16-19 study program budget​.</skos:example>
    </owl:Class>
    


    <!-- http://www.w3id.org/efro/efro#FundingAdjustment -->

    <owl:Class rdf:about="http://www.w3id.org/efro/efro#FundingAdjustment">
        <rdfs:subClassOf rdf:resource="http://www.w3id.org/efro/efro#FundingElement"/>
        <dcterms:description>Adjustments applied to the allocated funding based on compliance, attendance, or completion criteria. These adjustments may result in increases or reductions in funding based on specific conditions outlined in the ESFA guidance.</dcterms:description>
        <rdfs:label>FundingAdjustment</rdfs:label>
    </owl:Class>
    


    <!-- http://www.w3id.org/efro/efro#FundingBand -->

    <owl:Class rdf:about="http://www.w3id.org/efro/efro#FundingBand">
        <rdfs:subClassOf rdf:resource="http://www.w3id.org/efro/efro#FundingComponent"/>
        <dcterms:description>A predefined range of funding amounts based on the type and level of the qualification being delivered. Funding bands ensure consistency in funding allocations for similar programs.</dcterms:description>
        <rdfs:label>FundingBand</rdfs:label>
        <skos:example>Funding bands for apprenticeships, where the maximum band reflects the funding cap for that qualification.</skos:example>
    </owl:Class>
    


    <!-- http://www.w3id.org/efro/efro#FundingClaimReport -->

    <owl:Class rdf:about="http://www.w3id.org/efro/efro#FundingClaimReport">
        <rdfs:subClassOf rdf:resource="http://www.w3id.org/efro/efro#ReportDocument"/>
        <dcterms:description>A report summarizing the funding claims made by an institution, including planned hours, attendance, and eligible activities. This report is critical for validating funding received from the ESFA.</dcterms:description>
        <rdfs:label>FundingClaimReport</rdfs:label>
        <skos:example>Reports submitted during funding returns to justify the institution’s funding allocation.</skos:example>
    </owl:Class>
    


    <!-- http://www.w3id.org/efro/efro#FundingComponent -->

    <owl:Class rdf:about="http://www.w3id.org/efro/efro#FundingComponent">
        <rdfs:subClassOf rdf:resource="http://www.w3id.org/efro/efro#FundingElement"/>
        <dcterms:description>Specific elements or criteria that determine the amount of funding allocated to a program or institution. These components are used to calculate and validate funding claims.</dcterms:description>
        <rdfs:label>FundingComponent</rdfs:label>
    </owl:Class>
    


    <!-- http://www.w3id.org/efro/efro#FundingCondition -->

    <owl:Class rdf:about="http://www.w3id.org/efro/efro#FundingCondition">
        <rdfs:subClassOf rdf:resource="http://www.w3id.org/efro/efro#FundingElement"/>
        <dcterms:description>Specific conditions or rules that must be met to qualify for and retain funding. These conditions ensure institutions comply with ESFA funding regulations.</dcterms:description>
        <rdfs:label>FundingCondition</rdfs:label>
    </owl:Class>
    


    <!-- http://www.w3id.org/efro/efro#FundingElement -->

    <owl:Class rdf:about="http://www.w3id.org/efro/efro#FundingElement">
        <dcterms:description>Represents any concept, component, or adjustment directly associated with the allocation, distribution, or compliance of educational funding.</dcterms:description>
        <rdfs:label>FundingElement</rdfs:label>
    </owl:Class>
    


    <!-- http://www.w3id.org/efro/efro#FundingEvidenceDocument -->

    <owl:Class rdf:about="http://www.w3id.org/efro/efro#FundingEvidenceDocument">
        <rdfs:subClassOf rdf:resource="http://www.w3id.org/efro/efro#ComplianceDocument"/>
        <dcterms:description>A document used to support funding claims by providing evidence of student eligibility, attendance, planned hours, and study program delivery.</dcterms:description>
        <rdfs:label>FundingEvidenceDocument</rdfs:label>
        <skos:example>Learning agreements, enrollment forms, and timetables used as funding evidence during compliance audits.</skos:example>
    </owl:Class>
    


    <!-- http://www.w3id.org/efro/efro#FundingImpact -->

    <owl:Class rdf:about="http://www.w3id.org/efro/efro#FundingImpact">
        <rdfs:label>Funding Impact</rdfs:label>
    </owl:Class>
    


    <!-- http://www.w3id.org/efro/efro#FundingObligation -->

    <owl:Class rdf:about="http://www.w3id.org/efro/efro#FundingObligation">
        <rdfs:subClassOf rdf:resource="http://www.w3id.org/efro/efro#Obligation"/>
        <rdfs:subClassOf>
            <owl:Restriction>
                <owl:onProperty rdf:resource="http://www.w3id.org/efro/efro#hasHoursPlanned"/>
                <owl:maxQualifiedCardinality rdf:datatype="http://www.w3.org/2001/XMLSchema#nonNegativeInteger">1</owl:maxQualifiedCardinality>
                <owl:onDataRange rdf:resource="http://www.w3.org/2001/XMLSchema#integer"/>
            </owl:Restriction>
        </rdfs:subClassOf>
        <dcterms:description>A duty to meet specific conditions to access or retain funding. Institutions must ensure compliance with funding rules, such as delivering eligible qualifications and avoiding double funding.</dcterms:description>
        <rdfs:label>FundingObligation</rdfs:label>
        <skos:example>Obligations to demonstrate student participation, maintain evidence for planned hours, and ensure timely withdrawals for students who leave programs.</skos:example>
    </owl:Class>
    


    <!-- http://www.w3id.org/efro/efro#FundingOverlap -->

    <owl:Class rdf:about="http://www.w3id.org/efro/efro#FundingOverlap">
        <rdfs:subClassOf rdf:resource="http://www.w3id.org/efro/efro#FundingCondition"/>
        <dcterms:description>A condition addressing potential overlaps in funding claims, ensuring that institutions do not claim funding for overlapping study periods or activities.</dcterms:description>
        <rdfs:label>FundingOverlap</rdfs:label>
        <skos:example>Overlaps in planned hours between two study programs for the same studen.</skos:example>
    </owl:Class>
    


    <!-- http://www.w3id.org/efro/efro#FundingQualifyingPeriod -->

    <owl:Class rdf:about="http://www.w3id.org/efro/efro#FundingQualifyingPeriod">
        <rdfs:subClassOf rdf:resource="http://www.w3id.org/efro/efro#FundingCondition"/>
        <dcterms:description>A minimum period that students must participate in a study program to qualify for funding.</dcterms:description>
        <rdfs:label>FundingQualifyingPeriod</rdfs:label>
        <skos:example>Students must attend for a minimum number of days (e.g., 6 weeks) to qualify for ESFA funding.</skos:example>
    </owl:Class>
    


    <!-- http://www.w3id.org/efro/efro#FundingRate -->

    <owl:Class rdf:about="http://www.w3id.org/efro/efro#FundingRate">
        <rdfs:subClassOf rdf:resource="http://www.w3id.org/efro/efro#FundingComponent"/>
        <dcterms:description>The rate of funding allocated per qualification, student, or activity. Funding rates are determined based on qualification types, planned hours, and delivery models.</dcterms:description>
        <rdfs:label>FundingRate</rdfs:label>
        <skos:example>The rate per hour for study programs or specific funding rates for high-needs students​.</skos:example>
    </owl:Class>
    


    <!-- http://www.w3id.org/efro/efro#FundingReduction -->

    <owl:Class rdf:about="http://www.w3id.org/efro/efro#FundingReduction">
        <rdfs:subClassOf rdf:resource="http://www.w3id.org/efro/efro#FundingAdjustment"/>
        <dcterms:description>An adjustment reducing the allocated funding due to non-compliance, insufficient attendance, or failure to meet required criteria.</dcterms:description>
        <rdfs:label>FundingReduction</rdfs:label>
        <skos:example>A reduction applied if students do not meet the minimum threshold for planned hours or fail to qualify for funding.</skos:example>
    </owl:Class>
    


    <!-- http://www.w3id.org/efro/efro#FundingRegulations -->

    <owl:Class rdf:about="http://www.w3id.org/efro/efro#FundingRegulations">
        <rdfs:label>Funding Regulations</rdfs:label>
    </owl:Class>
    


    <!-- http://www.w3id.org/efro/efro#FundingStartCriteria -->

    <owl:Class rdf:about="http://www.w3id.org/efro/efro#FundingStartCriteria">
        <rdfs:subClassOf rdf:resource="http://www.w3id.org/efro/efro#FundingCondition"/>
        <dcterms:description>Criteria that must be met at the start of a program to establish eligibility for funding.</dcterms:description>
        <rdfs:label>FundingStartCriteria</rdfs:label>
        <skos:example>Students must meet age, residency, and program type criteria at the beginning of their study​.</skos:example>
    </owl:Class>
    


    <!-- http://www.w3id.org/efro/efro#FundingStartStatus -->

    <owl:Class rdf:about="http://www.w3id.org/efro/efro#FundingStartStatus">
        <rdfs:subClassOf rdf:resource="http://www.w3id.org/efro/efro#FundingStatus"/>
        <dcterms:description xml:lang="en">Defines the funding eligibility of a student at the beginning of their study programme.
The funding start status is determined by the student&apos;s enrollment date and whether they meet the qualifying period of attendance required to receive funding​.
This status also ensures that students are only funded at one institution at a time to prevent duplicate funding claims.</dcterms:description>
        <rdfs:label>FundingStartStatus</rdfs:label>
    </owl:Class>
    


    <!-- http://www.w3id.org/efro/efro#FundingStatus -->

    <owl:Class rdf:about="http://www.w3id.org/efro/efro#FundingStatus">
        <rdfs:subClassOf rdf:resource="http://www.w3id.org/efro/efro#Status"/>
        <dcterms:description>Represents the funding eligibility of a student or program based on compliance with ESFA rules.</dcterms:description>
        <rdfs:label>FundingStatus</rdfs:label>
    </owl:Class>
    


    <!-- http://www.w3id.org/efro/efro#FundingType -->

    <owl:Class rdf:about="http://www.w3id.org/efro/efro#FundingType">
        <rdfs:subClassOf rdf:resource="http://www.w3id.org/efro/efro#FundingElement"/>
        <dcterms:description>The type of funding allocated based on the program, qualification, or support being delivered. Funding types ensure alignment with ESFA rules for various educational pathways.</dcterms:description>
        <rdfs:label>FundingType</rdfs:label>
    </owl:Class>
    


    <!-- http://www.w3id.org/efro/efro#FundingYear -->

    <owl:Class rdf:about="http://www.w3id.org/efro/efro#FundingYear">
        <rdfs:subClassOf rdf:resource="http://www.w3id.org/efro/efro#TimePeriod"/>
        <dcterms:description>The 12-month period during which funding allocations and claims are calculated, typically aligned with the fiscal year.</dcterms:description>
        <rdfs:label>FundingYear</rdfs:label>
        <skos:example>ESFA funding allocations for the 2024/25 funding year​.</skos:example>
    </owl:Class>
    


    <!-- http://www.w3id.org/efro/efro#GeneralAdministrativeActivity -->

    <owl:Class rdf:about="http://www.w3id.org/efro/efro#GeneralAdministrativeActivity">
        <rdfs:subClassOf rdf:resource="http://www.w3id.org/efro/efro#AdministrativeActivity"/>
        <dcterms:description xml:lang="en">Activities that provide overall administrative support to the institution, ensuring smooth operations and adherence to ESFA guidelines.</dcterms:description>
        <rdfs:label>GeneralAdministrativeActivity</rdfs:label>
        <skos:example xml:lang="en">Scheduling student sessions, maintaining compliance records, and submitting data returns​.</skos:example>
    </owl:Class>
    


    <!-- http://www.w3id.org/efro/efro#GeneralAssistanceActivity -->

    <owl:Class rdf:about="http://www.w3id.org/efro/efro#GeneralAssistanceActivity">
        <rdfs:subClassOf rdf:resource="http://www.w3id.org/efro/efro#Activity"/>
        <rdfs:comment>Activities that provide general assistance or support but are not part of guided learning.</rdfs:comment>
        <rdfs:label>GeneralAssistanceActivity</rdfs:label>
    </owl:Class>
    


    <!-- http://www.w3id.org/efro/efro#GuidedLearning -->

    <owl:Class rdf:about="http://www.w3id.org/efro/efro#GuidedLearning">
        <rdfs:subClassOf rdf:resource="http://www.w3id.org/efro/efro#LearningMode"/>
        <dcterms:description>Planned learning hours under the direct supervision of a tutor or instructor.</dcterms:description>
        <rdfs:label>GuidedLearning</rdfs:label>
        <skos:example>Classroom teaching sessions and practical workshops​.</skos:example>
    </owl:Class>
    


    <!-- http://www.w3id.org/efro/efro#InitialASLevel -->

    <owl:Class rdf:about="http://www.w3id.org/efro/efro#InitialASLevel">
        <rdfs:subClassOf rdf:resource="http://www.w3id.org/efro/efro#Qualification"/>
        <dcterms:description>An AS Level qualification pursued at the start of a study program.</dcterms:description>
        <rdfs:label>InitialASLevel</rdfs:label>
        <skos:example>AS Level Chemistry taken as an initial qualification during a two-year program.</skos:example>
    </owl:Class>
    


    <!-- http://www.w3id.org/efro/efro#InitialPlannedHours -->

    <owl:Class rdf:about="http://www.w3id.org/efro/efro#InitialPlannedHours">
        <rdfs:subClassOf rdf:resource="http://www.w3id.org/efro/efro#PlannedHours"/>
        <dcterms:description>The originally planned hours recorded at the start of a study program.</dcterms:description>
        <rdfs:label>InitialPlannedHours</rdfs:label>
        <skos:example>Timetabled hours based on the initial agreement between the student and institution​.</skos:example>
    </owl:Class>
    


    <!-- http://www.w3id.org/efro/efro#Institution -->

    <owl:Class rdf:about="http://www.w3id.org/efro/efro#Institution">
        <rdfs:subClassOf rdf:resource="http://www.w3id.org/efro/efro#EducationalEntity"/>
        <dcterms:description>An educational organization that delivers funded programs or training to students, including schools, colleges, and academies.</dcterms:description>
        <rdfs:label>Institution</rdfs:label>
    </owl:Class>
    


    <!-- http://www.w3id.org/efro/efro#LastAttendanceActivity -->

    <owl:Class rdf:about="http://www.w3id.org/efro/efro#LastAttendanceActivity">
        <rdfs:subClassOf rdf:resource="http://www.w3id.org/efro/efro#AttendanceActivity"/>
        <dcterms:description>The last recorded attendance activity for a student, marking their most recent engagement.</dcterms:description>
        <rdfs:label>LastAttendanceActivity</rdfs:label>
        <skos:example>Used for calculating funding adjustments after a withdrawal.</skos:example>
    </owl:Class>
    


    <!-- http://www.w3id.org/efro/efro#LastAttendanceDate -->

    <owl:Class rdf:about="http://www.w3id.org/efro/efro#LastAttendanceDate">
        <rdfs:subClassOf rdf:resource="http://www.w3id.org/efro/efro#TimePoint"/>
        <dcterms:description>The most recent date on which a student attended their study program. This date is used to determine withdrawal or early completion status.</dcterms:description>
        <rdfs:label>LastAttendanceDate</rdfs:label>
        <skos:example>A student’s funding eligibility ends based on their last recorded attendance date if they withdraw.</skos:example>
    </owl:Class>
    


    <!-- http://www.w3id.org/efro/efro#LastExam -->

    <owl:Class rdf:about="http://www.w3id.org/efro/efro#LastExam">
        <rdfs:subClassOf rdf:resource="http://www.w3id.org/efro/efro#AssessmentActivity"/>
        <dcterms:description>Represents the final or most recent exam undertaken by a student in a study program.</dcterms:description>
        <rdfs:label>LastExam</rdfs:label>
        <skos:example>The last exam completed before a withdrawal or completion​.</skos:example>
    </owl:Class>
    


    <!-- http://www.w3id.org/efro/efro#LastMarkedAssignment -->

    <owl:Class rdf:about="http://www.w3id.org/efro/efro#LastMarkedAssignment">
        <rdfs:subClassOf rdf:resource="http://www.w3id.org/efro/efro#AssessmentActivity"/>
        <dcterms:description>An assignment activity that represents the most recently evaluated and graded assignment for a student.</dcterms:description>
        <rdfs:label>LastMarkedAssignment</rdfs:label>
        <skos:example>A student’s final marked project before program completion.</skos:example>
    </owl:Class>
    


    <!-- http://www.w3id.org/efro/efro#Learning -->

    <owl:Class rdf:about="http://www.w3id.org/efro/efro#Learning">
        <dcterms:description>Represents all aspects of educational and training activities, including the aims, aspects, modes, qualifications, and study programs. It serves as a broad category encompassing the fundamental components of the educational process.</dcterms:description>
        <rdfs:label>Learning</rdfs:label>
    </owl:Class>
    


    <!-- http://www.w3id.org/efro/efro#LearningAim -->

    <owl:Class rdf:about="http://www.w3id.org/efro/efro#LearningAim">
        <rdfs:subClassOf rdf:resource="http://purl.org/vocab/aiiso/schema#KnowledgeGrouping"/>
        <dcterms:description>Refers to the specific educational or training objectives for a student, which may include qualifications or skills development. These aims guide the structure of study programs and funding eligibility.</dcterms:description>
        <rdfs:label>LearningAim</rdfs:label>
    </owl:Class>
    


    <!-- http://www.w3id.org/efro/efro#LearningAspect -->

    <owl:Class rdf:about="http://www.w3id.org/efro/efro#LearningAspect">
        <rdfs:subClassOf rdf:resource="http://www.w3id.org/efro/efro#Learning"/>
        <dcterms:description>Represents the measurable components of a learning aim, such as attendance, planned hours, and timetabled activities, which are essential for funding and compliance.</dcterms:description>
        <rdfs:label>LearningAspect</rdfs:label>
    </owl:Class>
    


    <!-- http://www.w3id.org/efro/efro#LearningMode -->

    <owl:Class rdf:about="http://www.w3id.org/efro/efro#LearningMode">
        <owl:equivalentClass>
            <owl:Class>
                <owl:unionOf rdf:parseType="Collection">
                    <rdf:Description rdf:about="http://www.w3id.org/efro/efro#DistanceLearningProvision"/>
                    <rdf:Description rdf:about="http://www.w3id.org/efro/efro#GuidedLearning"/>
                    <rdf:Description rdf:about="http://www.w3id.org/efro/efro#OpenLearningProvision"/>
                    <rdf:Description rdf:about="http://www.w3id.org/efro/efro#TraditionalProvision"/>
                </owl:unionOf>
            </owl:Class>
        </owl:equivalentClass>
        <rdfs:subClassOf rdf:resource="http://www.w3id.org/efro/efro#Learning"/>
        <dcterms:description>The mode of delivery for learning activities, indicating whether the program is delivered in person, online, or in other formats.</dcterms:description>
        <rdfs:label>LearningMode</rdfs:label>
    </owl:Class>
    


    <!-- http://www.w3id.org/efro/efro#LocalAuthority -->

    <owl:Class rdf:about="http://www.w3id.org/efro/efro#LocalAuthority">
        <rdfs:subClassOf rdf:resource="http://www.w3id.org/efro/efro#Authority"/>
        <dcterms:description>A regional administrative body responsible for funding and regulating educational institutions, typically for maintained schools and programs within their jurisdiction.</dcterms:description>
        <rdfs:label>LocalAuthority</rdfs:label>
        <skos:example>Local authorities provide funding to schools and oversee compliance with ESFA regulations for young people’s education</skos:example>
    </owl:Class>
    


    <!-- http://www.w3id.org/efro/efro#NewStart -->

    <owl:Class rdf:about="http://www.w3id.org/efro/efro#NewStart">
        <rdfs:subClassOf rdf:resource="http://www.w3id.org/efro/efro#EnrollmentActivity"/>
        <dcterms:description>The enrollment of a student starting a new program or qualification aim.</dcterms:description>
        <rdfs:label>NewStart</rdfs:label>
        <skos:example>A new enrollment after transferring institutions​.</skos:example>
    </owl:Class>
    


    <!-- http://www.w3id.org/efro/efro#NonAttendanceActivity -->

    <owl:Class rdf:about="http://www.w3id.org/efro/efro#NonAttendanceActivity">
        <rdfs:subClassOf rdf:resource="http://www.w3id.org/efro/efro#AttendanceActivity"/>
        <dcterms:description>Records events where students fail to attend scheduled activities and addresses their reasons for absence.</dcterms:description>
        <rdfs:label>NonAttendanceActivity</rdfs:label>
        <skos:example>Logs documenting student absences due to personal reasons​.</skos:example>
    </owl:Class>
    


    <!-- http://www.w3id.org/efro/efro#NonAttendanceReason -->

    <owl:Class rdf:about="http://www.w3id.org/efro/efro#NonAttendanceReason">
        <rdfs:subClassOf rdf:resource="http://www.w3id.org/efro/efro#WithdrawalReason"/>
        <dcterms:description>A reason for a student’s failure to attend required sessions or activities, which may impact funding eligibility or compliance.</dcterms:description>
        <rdfs:label>NonAttendanceReason</rdfs:label>
        <skos:example>Absences due to illness, family emergencies, or personal issues.</skos:example>
    </owl:Class>
    


    <!-- http://www.w3id.org/efro/efro#NonFundedStatus -->

    <owl:Class rdf:about="http://www.w3id.org/efro/efro#NonFundedStatus">
        <rdfs:subClassOf rdf:resource="http://www.w3id.org/efro/efro#FundingStatus"/>
        <dcterms:description>Represents a student or program that does not qualify for ESFA funding due to ineligibility or non-compliance.</dcterms:description>
        <rdfs:label>NonFundedStatus</rdfs:label>
        <skos:example>A program exceeding the funding cap or students not meeting residency requirements.</skos:example>
    </owl:Class>
    


    <!-- http://www.w3id.org/efro/efro#NonQualificationAim -->

    <owl:Class rdf:about="http://www.w3id.org/efro/efro#NonQualificationAim">
        <rdfs:subClassOf rdf:resource="http://www.w3id.org/efro/efro#LearningAim"/>
        <dcterms:description>Learning aims that do not lead directly to a formal qualification but support personal or professional development.</dcterms:description>
        <rdfs:label>NonQualificationAim</rdfs:label>
        <skos:example>Enrichment activities, work placements, or employability skills sessions that are part of the study program​.</skos:example>
    </owl:Class>
    


    <!-- http://www.w3id.org/efro/efro#NotCompletedStatus -->

    <owl:Class rdf:about="http://www.w3id.org/efro/efro#NotCompletedStatus">
        <rdfs:subClassOf rdf:resource="http://www.w3id.org/efro/efro#CompletionStatus"/>
        <dcterms:description>Status indicating that the student did not complete their study program, potentially impacting funding claims.</dcterms:description>
        <rdfs:label>NotCompletedStatus</rdfs:label>
        <skos:example>A student withdrawing midway due to personal or attendance-related issues.</skos:example>
    </owl:Class>
    


    <!-- http://www.w3id.org/efro/efro#Obligation -->

    <owl:Class rdf:about="http://www.w3id.org/efro/efro#Obligation">
        <dcterms:description>Represents a duty or requirement placed on individuals or institutions to comply with rules, funding conditions, or reporting requirements as outlined in the ESFA guidance.</dcterms:description>
        <rdfs:label>Obligation</rdfs:label>
    </owl:Class>
    


    <!-- http://www.w3id.org/efro/efro#OpenLearningProvision -->

    <owl:Class rdf:about="http://www.w3id.org/efro/efro#OpenLearningProvision">
        <rdfs:subClassOf rdf:resource="http://www.w3id.org/efro/efro#LearningMode"/>
        <dcterms:description>Learning delivered in an open format, allowing flexibility in attendance and participation.</dcterms:description>
        <rdfs:label>OpenLearningProvision</rdfs:label>
        <skos:example>Self-paced online courses​.</skos:example>
    </owl:Class>
    


    <!-- http://www.w3id.org/efro/efro#PartTimeProgram -->

    <owl:Class rdf:about="http://www.w3id.org/efro/efro#PartTimeProgram">
        <rdfs:subClassOf rdf:resource="http://www.w3id.org/efro/efro#StudyProgramme"/>
        <dcterms:description>A study program with fewer than 540 planned hours, designed for part-time learners.</dcterms:description>
        <rdfs:label>PartTimeProgram</rdfs:label>
        <skos:example>Part-time vocational qualifications delivered to adult learners​.</skos:example>
    </owl:Class>
    


    <!-- http://www.w3id.org/efro/efro#PartTimeStudent -->

    <owl:Class rdf:about="http://www.w3id.org/efro/efro#PartTimeStudent">
        <rdfs:subClassOf rdf:resource="http://www.w3id.org/efro/efro#Student"/>
        <owl:disjointWith>
            <owl:Class>
                <owl:unionOf rdf:parseType="Collection">
                    <rdf:Description rdf:about="http://www.w3id.org/efro/efro#FullTimeStudent"/>
                    <rdf:Description rdf:about="http://www.w3id.org/efro/efro#TimeRelated"/>
                </owl:unionOf>
            </owl:Class>
        </owl:disjointWith>
        <dcterms:description>A student enrolled in a study program with fewer than 540 planned hours over an academic year, qualifying as part-time under ESFA funding rules.</dcterms:description>
        <rdfs:label>PartTimeStudent</rdfs:label>
        <skos:example>n adult learner attending evening classes for a vocational qualification.</skos:example>
    </owl:Class>
    


    <!-- http://www.w3id.org/efro/efro#Participant -->

    <owl:Class rdf:about="http://www.w3id.org/efro/efro#Participant">
        <rdfs:subClassOf rdf:resource="http://www.w3id.org/efro/efro#Person"/>
        <rdfs:subClassOf rdf:resource="http://xmlns.com/foaf/0.1/Person"/>
        <dcterms:description>An individual engaged in an educational or training program, including apprentices, trainees, or young people.</dcterms:description>
        <rdfs:label>Participant</rdfs:label>
    </owl:Class>
    


    <!-- http://www.w3id.org/efro/efro#ParticipationStatus -->

    <owl:Class rdf:about="http://www.w3id.org/efro/efro#ParticipationStatus">
        <rdfs:subClassOf rdf:resource="http://www.w3id.org/efro/efro#Status"/>
        <dcterms:description>Reflects the engagement level of a student in their study program or activities.</dcterms:description>
        <rdfs:label>ParticipationStatus</rdfs:label>
    </owl:Class>
    


    <!-- http://www.w3id.org/efro/efro#Person -->

    <owl:Class rdf:about="http://www.w3id.org/efro/efro#Person">
        <owl:equivalentClass rdf:resource="http://xmlns.com/foaf/0.1/Person"/>
        <rdfs:subClassOf rdf:resource="http://xmlns.com/foaf/0.1/Agent"/>
        <dcterms:description>Represents any individual involved in educational activities, including students, staff, and participants in funded programs.</dcterms:description>
        <rdfs:label>Person</rdfs:label>
    </owl:Class>
    


    <!-- http://www.w3id.org/efro/efro#PersonalReason -->

    <owl:Class rdf:about="http://www.w3id.org/efro/efro#PersonalReason">
        <rdfs:subClassOf rdf:resource="http://www.w3id.org/efro/efro#WithdrawalReason"/>
        <dcterms:description>A reason related to personal circumstances, such as health, family responsibilities, or financial challenges, which may lead to non-attendance, withdrawal, or progression changes.</dcterms:description>
        <rdfs:label>PersonalReason</rdfs:label>
        <skos:example>Withdrawal from a study program due to personal health issues​.</skos:example>
    </owl:Class>
    


    <!-- http://www.w3id.org/efro/efro#PlannedHours -->

    <owl:Class rdf:about="http://www.w3id.org/efro/efro#PlannedHours">
        <rdfs:subClassOf rdf:resource="http://www.w3id.org/efro/efro#LearningAspect"/>
        <dcterms:description>The total hours planned for the delivery of a study program, including qualification and non-qualification hours.</dcterms:description>
        <rdfs:label>PlannedHours</rdfs:label>
        <skos:example>Timetabled hours documented for ESFA funding compliance.</skos:example>
    </owl:Class>
    


    <!-- http://www.w3id.org/efro/efro#PlannedHoursRecord -->

    <owl:Class rdf:about="http://www.w3id.org/efro/efro#PlannedHoursRecord">
        <rdfs:subClassOf rdf:resource="http://www.w3id.org/efro/efro#RecordDocument"/>
        <dcterms:description>A document detailing the planned learning hours for a student, including both qualification and non-qualification hours. This record ensures alignment with ESFA&apos;s funding conditions and planned hours requirements.</dcterms:description>
        <rdfs:label>PlannedHoursRecord</rdfs:label>
        <skos:example>Timetables or schedules used to record and verify planned hours submitted in data return</skos:example>
    </owl:Class>
    


    <!-- http://www.w3id.org/efro/efro#ProgrammeAim -->

    <owl:Class rdf:about="http://www.w3id.org/efro/efro#ProgrammeAim">
        <rdfs:subClassOf rdf:resource="http://www.w3id.org/efro/efro#LearningAim"/>
        <rdfs:label>Programme Aim</rdfs:label>
    </owl:Class>
    


    <!-- http://www.w3id.org/efro/efro#ProgrammeCompletionActivity -->

    <owl:Class rdf:about="http://www.w3id.org/efro/efro#ProgrammeCompletionActivity">
        <rdfs:subClassOf rdf:resource="http://www.w3id.org/efro/efro#CompletionActivity"/>
        <dcterms:description>Activities marking the official completion of a study program or learning aim.</dcterms:description>
        <rdfs:label>ProgrammeCompletionActivity</rdfs:label>
        <skos:example>Finalizing the records for students who meet all qualification criteria​.</skos:example>
    </owl:Class>
    


    <!-- http://www.w3id.org/efro/efro#ProgrammeStart -->

    <owl:Class rdf:about="http://www.w3id.org/efro/efro#ProgrammeStart">
        <rdfs:subClassOf rdf:resource="http://www.w3id.org/efro/efro#EnrollmentActivity"/>
        <dcterms:description>The activity marking the initiation of a specific study program for a student.</dcterms:description>
        <rdfs:label>ProgrammeStart</rdfs:label>
        <skos:example>Official start dates recorded for funding compliance.</skos:example>
    </owl:Class>
    


    <!-- http://www.w3id.org/efro/efro#ProgrammeStartDate -->

    <owl:Class rdf:about="http://www.w3id.org/efro/efro#ProgrammeStartDate">
        <rdfs:subClassOf rdf:resource="http://www.w3id.org/efro/efro#TimePoint"/>
        <dcterms:description>The official start date of a study program, marking the beginning of planned hours and eligibility for funding.</dcterms:description>
        <rdfs:label>ProgrammeStartDate</rdfs:label>
        <skos:example>Program start dates must match the information provided in ILR returns to avoid discrepancies during audits​.</skos:example>
    </owl:Class>
    


    <!-- http://www.w3id.org/efro/efro#ProgressReport -->

    <owl:Class rdf:about="http://www.w3id.org/efro/efro#ProgressReport">
        <rdfs:subClassOf rdf:resource="http://www.w3id.org/efro/efro#ReportDocument"/>
        <dcterms:description>A document detailing a student’s academic progress, attendance, and completion status for specific study programs. These reports may be used for funding audits, compliance checks, or student support.</dcterms:description>
        <rdfs:label>ProgressReport</rdfs:label>
        <skos:example>Reports showing students’ achievement in meeting their learning aims and progression to higher-level study or employment.</skos:example>
    </owl:Class>
    


    <!-- http://www.w3id.org/efro/efro#ProgressionActivity -->

    <owl:Class rdf:about="http://www.w3id.org/efro/efro#ProgressionActivity">
        <rdfs:subClassOf rdf:resource="http://www.w3id.org/efro/efro#AssessmentActivity"/>
        <dcterms:description>Activities aimed at tracking or enabling a student’s academic or professional progression.</dcterms:description>
        <rdfs:label>ProgressionActivity</rdfs:label>
    </owl:Class>
    


    <!-- http://www.w3id.org/efro/efro#ProgressionReason -->

    <owl:Class rdf:about="http://www.w3id.org/efro/efro#ProgressionReason">
        <rdfs:subClassOf rdf:resource="http://www.w3id.org/efro/efro#WithdrawalReason"/>
        <dcterms:description>A reason explaining a student&apos;s progression within or beyond their current study program.</dcterms:description>
        <rdfs:label>ProgressionReason</rdfs:label>
        <skos:example>Progression to a higher qualification, an apprenticeship, or sustainable employment​.</skos:example>
    </owl:Class>
    


    <!-- http://www.w3id.org/efro/efro#ProgressionStatus -->

    <owl:Class rdf:about="http://www.w3id.org/efro/efro#ProgressionStatus">
        <rdfs:subClassOf rdf:resource="http://www.w3id.org/efro/efro#Status"/>
        <dcterms:description>Reflects the progression state of a student within or beyond their current study program.</dcterms:description>
        <rdfs:label>ProgressionStatus</rdfs:label>
    </owl:Class>
    


    <!-- http://www.w3id.org/efro/efro#ProgressionType -->

    <owl:Class rdf:about="http://www.w3id.org/efro/efro#ProgressionType">
        <rdfs:subClassOf rdf:resource="http://www.w3id.org/efro/efro#ProgressionActivity"/>
        <dcterms:description xml:lang="en">Categorizes different types of educational and career progression pathways for students.</dcterms:description>
        <rdfs:label>ProgressionType</rdfs:label>
    </owl:Class>
    


    <!-- http://www.w3id.org/efro/efro#Qualification -->

    <owl:Class rdf:about="http://www.w3id.org/efro/efro#Qualification">
        <rdfs:subClassOf rdf:resource="http://purl.org/vocab/aiiso/schema#KnowledgeGrouping"/>
        <dcterms:description>Refers to formal certifications awarded upon completion of a recognized learning aim.</dcterms:description>
        <rdfs:label>Qualification</rdfs:label>
    </owl:Class>
    


    <!-- http://www.w3id.org/efro/efro#QualificationAim -->

    <owl:Class rdf:about="http://www.w3id.org/efro/efro#QualificationAim">
        <rdfs:subClassOf rdf:resource="http://www.w3id.org/efro/efro#LearningAim"/>
        <dcterms:description>Learning aims that lead to a recognized qualification, such as academic or vocational certifications.</dcterms:description>
        <rdfs:label>QualificationAim</rdfs:label>
        <skos:example>A Level, vocational qualifications, or apprenticeship standards included in the ESFA’s list of eligible qualifications.</skos:example>
    </owl:Class>
    


    <!-- http://www.w3id.org/efro/efro#QualifyingAttendanceActivity -->

    <owl:Class rdf:about="http://www.w3id.org/efro/efro#QualifyingAttendanceActivity">
        <rdfs:subClassOf rdf:resource="http://www.w3id.org/efro/efro#AttendanceActivity"/>
        <dcterms:description>Attendance activities that meet the criteria for funding eligibility and compliance, such as qualifying hours or required participation levels.</dcterms:description>
        <rdfs:label>QualifyingAttendanceActivity</rdfs:label>
        <skos:example>A student must attend six weeks of sessions to qualify for funding.</skos:example>
    </owl:Class>
    


    <!-- http://www.w3id.org/efro/efro#QualifyingPeriod -->

    <owl:Class rdf:about="http://www.w3id.org/efro/efro#QualifyingPeriod">
        <rdfs:subClassOf rdf:resource="http://www.w3id.org/efro/efro#TimePeriod"/>
        <dcterms:description>A minimum duration a student must attend to qualify for funding. Often, this refers to the six-week attendance rule.</dcterms:description>
        <rdfs:label>QualifyingPeriod</rdfs:label>
        <skos:example>A student must attend their program for at least six weeks to qualify for funding eligibility​.</skos:example>
    </owl:Class>
    


    <!-- http://www.w3id.org/efro/efro#QualityAssuranceRecord -->

    <owl:Class rdf:about="http://www.w3id.org/efro/efro#QualityAssuranceRecord">
        <rdfs:subClassOf rdf:resource="http://www.w3id.org/efro/efro#ComplianceDocument"/>
        <dcterms:description>Records that provide evidence of adherence to quality standards in delivering study programs, attendance monitoring, and institutional processes. These documents demonstrate efforts to meet educational objectives and maintain service quality.</dcterms:description>
        <rdfs:label>QualityAssuranceRecord</rdfs:label>
        <skos:example>Records ensuring accurate data in ILR returns or evidence of robust attendance tracking systems.</skos:example>
    </owl:Class>
    


    <!-- http://www.w3id.org/efro/efro#ReEnrollmentActivity -->

    <owl:Class rdf:about="http://www.w3id.org/efro/efro#ReEnrollmentActivity">
        <rdfs:subClassOf rdf:resource="http://www.w3id.org/efro/efro#EnrollmentActivity"/>
        <rdfs:label>ReEnrollment Activity</rdfs:label>
    </owl:Class>
    


    <!-- http://www.w3id.org/efro/efro#Reason -->

    <owl:Class rdf:about="http://www.w3id.org/efro/efro#Reason">
        <dcterms:description>Represents the justification or cause for an action, event, or decision related to education and training, such as withdrawal, non-attendance, or progression.</dcterms:description>
        <rdfs:label>Reason</rdfs:label>
    </owl:Class>
    


    <!-- http://www.w3id.org/efro/efro#RecordDocument -->

    <owl:Class rdf:about="http://www.w3id.org/efro/efro#RecordDocument">
        <rdfs:subClassOf rdf:resource="http://www.w3id.org/efro/efro#Document"/>
        <dcterms:description>A category of documents used to log and maintain detailed information for compliance, attendance, and funding-related activities.</dcterms:description>
        <rdfs:label>RecordDocument</rdfs:label>
    </owl:Class>
    


    <!-- http://www.w3id.org/efro/efro#RecordFundingValue -->

    <owl:Class rdf:about="http://www.w3id.org/efro/efro#RecordFundingValue">
        <rdfs:subClassOf rdf:resource="http://www.w3id.org/efro/efro#RecordingActivity"/>
        <dcterms:description>An activity that involves documenting the funding value associated with a specific student or program.</dcterms:description>
        <rdfs:label>RecordFundingValue</rdfs:label>
        <skos:example>Recording the funding rate in relation to planned hours.</skos:example>
    </owl:Class>
    


    <!-- http://www.w3id.org/efro/efro#RecordedPlannedHours -->

    <owl:Class rdf:about="http://www.w3id.org/efro/efro#RecordedPlannedHours">
        <rdfs:subClassOf rdf:resource="http://www.w3id.org/efro/efro#PlannedHours"/>
        <dcterms:description>The official record of planned hours submitted in funding claims or ILR returns.</dcterms:description>
        <rdfs:label>RecordedPlannedHours</rdfs:label>
        <skos:example>Hours documented for audit purposes​.</skos:example>
    </owl:Class>
    


    <!-- http://www.w3id.org/efro/efro#RecordingActivity -->

    <owl:Class rdf:about="http://www.w3id.org/efro/efro#RecordingActivity">
        <rdfs:subClassOf rdf:resource="http://www.w3id.org/efro/efro#Activity"/>
        <dcterms:description>Covers the documentation and recording of data required for compliance, attendance, and funding purposes.</dcterms:description>
        <rdfs:label>RecordingActivity</rdfs:label>
    </owl:Class>
    


    <!-- http://www.w3id.org/efro/efro#RecordingPlannedHours -->

    <owl:Class rdf:about="http://www.w3id.org/efro/efro#RecordingPlannedHours">
        <rdfs:subClassOf rdf:resource="http://www.w3id.org/efro/efro#RecordingActivity"/>
        <dcterms:description>The activity of recording the planned study or attendance hours for a program, as required for compliance.</dcterms:description>
        <rdfs:label>RecordingPlannedHours</rdfs:label>
        <skos:example>Timetables recorded at the start of the academic year</skos:example>
    </owl:Class>
    


    <!-- http://www.w3id.org/efro/efro#RegulatoryBody -->

    <owl:Class rdf:about="http://www.w3id.org/efro/efro#RegulatoryBody">
        <rdfs:subClassOf rdf:resource="http://www.w3id.org/efro/efro#Authority"/>
        <dcterms:description>A body responsible for creating, implementing, and monitoring compliance with regulations related to education and funding.</dcterms:description>
        <rdfs:label>RegulatoryBody</rdfs:label>
        <skos:example>The ESFA, which enforces funding rules and monitors compliance through audits and guidelines, is a regulatory body​</skos:example>
    </owl:Class>
    


    <!-- http://www.w3id.org/efro/efro#ReplacementActivity -->

    <owl:Class rdf:about="http://www.w3id.org/efro/efro#ReplacementActivity">
        <rdfs:subClassOf rdf:resource="http://www.w3id.org/efro/efro#LearningAim"/>
        <dcterms:description>Activities undertaken to replace a withdrawn or discontinued learning aim.</dcterms:description>
        <rdfs:label>ReplacementActivity</rdfs:label>
        <skos:example>A student switches to a similar qualification after withdrawing from their original learning aim​.</skos:example>
    </owl:Class>
    


    <!-- http://www.w3id.org/efro/efro#ReportDocument -->

    <owl:Class rdf:about="http://www.w3id.org/efro/efro#ReportDocument">
        <rdfs:subClassOf rdf:resource="http://purl.org/cerif/frapo/Output"/>
        <rdfs:subClassOf rdf:resource="http://www.w3id.org/efro/efro#Document"/>
        <dcterms:description>A document summarizing key institutional activities, compliance metrics, or funding-related outcomes. These reports are typically submitted to or reviewed by the ESFA.</dcterms:description>
        <rdfs:label>ReportDocument</rdfs:label>
    </owl:Class>
    


    <!-- http://www.w3id.org/efro/efro#ReportingObligation -->

    <owl:Class rdf:about="http://www.w3id.org/efro/efro#ReportingObligation">
        <rdfs:subClassOf rdf:resource="http://www.w3id.org/efro/efro#Obligation"/>
        <dcterms:description>A requirement to submit accurate and timely data to the ESFA, including Individualized Learner Records (ILR) and evidence of compliance.</dcterms:description>
        <rdfs:label>ReportingObligation</rdfs:label>
        <skos:example>Submission of ILR data to report attendance, withdrawals, and funding claims for audit purposes​.</skos:example>
    </owl:Class>
    


    <!-- http://www.w3id.org/efro/efro#RetainedForFundingStatus -->

    <owl:Class rdf:about="http://www.w3id.org/efro/efro#RetainedForFundingStatus">
        <rdfs:subClassOf rdf:resource="http://www.w3id.org/efro/efro#FundingStatus"/>
        <dcterms:description>Indicates that the student’s funding status is retained due to their compliance with attendance and program criteria.</dcterms:description>
        <rdfs:label>RetainedForFundingStatus</rdfs:label>
        <skos:example>Retention factors applied for students completing their planned hours.</skos:example>
    </owl:Class>
    


    <!-- http://www.w3id.org/efro/efro#RetainedStatus -->

    <owl:Class rdf:about="http://www.w3id.org/efro/efro#RetainedStatus">
        <rdfs:subClassOf rdf:resource="http://www.w3id.org/efro/efro#ParticipationStatus"/>
        <dcterms:description>Represents that the student remains retained within the study program and meets retention criteria for funding.</dcterms:description>
        <rdfs:label>RetainedStatus</rdfs:label>
        <skos:example>Students continuing to the next term after meeting engagement thresholds​.</skos:example>
    </owl:Class>
    


    <!-- http://www.w3id.org/efro/efro#RetentionFactor -->

    <owl:Class rdf:about="http://www.w3id.org/efro/efro#RetentionFactor">
        <rdfs:subClassOf rdf:resource="http://www.w3id.org/efro/efro#FundingComponent"/>
        <dcterms:description>A multiplier applied to funding calculations to account for student retention. Institutions are incentivized to retain students until the completion of their study programs.</dcterms:description>
        <rdfs:label>RetentionFactor</rdfs:label>
        <skos:example>Retention factors are used to adjust funding based on whether students complete the full planned program.</skos:example>
    </owl:Class>
    


    <!-- http://www.w3id.org/efro/efro#SameInstitution -->

    <owl:Class rdf:about="http://www.w3id.org/efro/efro#SameInstitution">
        <rdfs:subClassOf rdf:resource="http://www.w3id.org/efro/efro#Institution"/>
        <dcterms:description>Refers to the scenario where a student remains enrolled in the same educational institution for the entire duration of their program.</dcterms:description>
        <rdfs:label>SameInstitution</rdfs:label>
        <skos:example>Continuity of a student’s enrollment in a single institution ensures alignment with funding guidelines without duplication​</skos:example>
    </owl:Class>
    


    <!-- http://www.w3id.org/efro/efro#SixWeekPeriod -->

    <owl:Class rdf:about="http://www.w3id.org/efro/efro#SixWeekPeriod">
        <rdfs:subClassOf rdf:resource="http://www.w3id.org/efro/efro#TimePeriod"/>
        <dcterms:description>A specific six-week duration used to measure qualifying attendance or compliance with funding rules.</dcterms:description>
        <rdfs:label>SixWeekPeriod</rdfs:label>
        <skos:example>Institutions must confirm attendance records for students retained during the first six weeks of their program​.</skos:example>
    </owl:Class>
    


    <!-- http://www.w3id.org/efro/efro#SixWeeksEarlyCompletion -->

    <owl:Class rdf:about="http://www.w3id.org/efro/efro#SixWeeksEarlyCompletion">
        <rdfs:subClassOf rdf:resource="http://www.w3id.org/efro/efro#TimeCondition"/>
        <dcterms:description>Indicates early completion of a program within six weeks of the planned end date. Funding adjustments may apply in such cases.</dcterms:description>
        <rdfs:label>SixWeeksEarlyCompletion</rdfs:label>
        <skos:example>A student completing all their assessments six weeks before the scheduled end date of their program​.</skos:example>
    </owl:Class>
    


    <!-- http://www.w3id.org/efro/efro#SkillsProgressionActivity -->

    <owl:Class rdf:about="http://www.w3id.org/efro/efro#SkillsProgressionActivity">
        <rdfs:subClassOf rdf:resource="http://www.w3id.org/efro/efro#ProgressionActivity"/>
        <dcterms:description>Activities aimed at developing specific skills to improve employability or academic readiness.</dcterms:description>
        <rdfs:label>SkillsProgressionActivity</rdfs:label>
    </owl:Class>
    


    <!-- http://www.w3id.org/efro/efro#Staff -->

    <owl:Class rdf:about="http://www.w3id.org/efro/efro#Staff">
        <rdfs:subClassOf rdf:resource="http://www.w3id.org/efro/efro#Person"/>
        <rdfs:subClassOf rdf:resource="http://xmlns.com/foaf/0.1/Person"/>
        <dcterms:description>Represents individuals employed by an institution to support educational delivery, compliance, and administration.</dcterms:description>
        <rdfs:label>Staff</rdfs:label>
    </owl:Class>
    


    <!-- http://www.w3id.org/efro/efro#Status -->

    <owl:Class rdf:about="http://www.w3id.org/efro/efro#Status">
        <owl:equivalentClass>
            <owl:Class>
                <owl:unionOf rdf:parseType="Collection">
                    <rdf:Description rdf:about="http://www.w3id.org/efro/efro#CompletionStatus"/>
                    <rdf:Description rdf:about="http://www.w3id.org/efro/efro#EnrollmentStatus"/>
                    <rdf:Description rdf:about="http://www.w3id.org/efro/efro#FundingStatus"/>
                    <rdf:Description rdf:about="http://www.w3id.org/efro/efro#ProgressionStatus"/>
                </owl:unionOf>
            </owl:Class>
        </owl:equivalentClass>
        <dcterms:description>Represents the state or condition of a student, program, or funding claim at a specific point in time, influencing eligibility, compliance, and progression.</dcterms:description>
        <rdfs:label>Status</rdfs:label>
    </owl:Class>
    


    <!-- http://www.w3id.org/efro/efro#StopFunding -->

    <owl:Class rdf:about="http://www.w3id.org/efro/efro#StopFunding">
        <rdfs:subClassOf rdf:resource="http://www.w3id.org/efro/efro#FundingImpact"/>
        <rdfs:label>Stop Funding</rdfs:label>
    </owl:Class>
    


    <!-- http://www.w3id.org/efro/efro#Student -->

    <owl:Class rdf:about="http://www.w3id.org/efro/efro#Student">
        <owl:equivalentClass>
            <owl:Class>
                <owl:unionOf rdf:parseType="Collection">
                    <rdf:Description rdf:about="http://www.w3id.org/efro/efro#FullTimeStudent"/>
                    <rdf:Description rdf:about="http://www.w3id.org/efro/efro#PartTimeStudent"/>
                    <rdf:Description rdf:about="http://www.w3id.org/efro/efro#WithdrawnStudent"/>
                </owl:unionOf>
            </owl:Class>
        </owl:equivalentClass>
        <rdfs:subClassOf rdf:resource="http://www.w3id.org/efro/efro#Person"/>
        <rdfs:subClassOf rdf:resource="http://xmlns.com/foaf/0.1/Person"/>
        <dcterms:description>Represents an individual enrolled in a study program or training course at an educational institution.</dcterms:description>
        <rdfs:label>Student</rdfs:label>
    </owl:Class>
    


    <!-- http://www.w3id.org/efro/efro#StudentAttendance -->

    <owl:Class rdf:about="http://www.w3id.org/efro/efro#StudentAttendance">
        <rdfs:subClassOf rdf:resource="http://www.w3id.org/efro/efro#AttendanceActivity"/>
        <dcterms:description>An overarching activity encompassing the tracking and management of all attendance-related actions for students.</dcterms:description>
        <rdfs:label>StudentAttendance</rdfs:label>
        <skos:example>Comprehensive attendance tracking for ILR submissions.</skos:example>
    </owl:Class>
    


    <!-- http://www.w3id.org/efro/efro#StudyProgramme -->

    <owl:Class rdf:about="http://www.w3id.org/efro/efro#StudyProgramme">
        <rdfs:subClassOf rdf:resource="http://purl.org/vocab/aiiso/schema#Programme"/>
        <dcterms:description>A structured educational program combining qualification and non-qualification aims, designed to meet the needs of students and prepare them for progression to further education, training, or employment.</dcterms:description>
        <rdfs:label>StudyProgramme</rdfs:label>
    </owl:Class>
    


    <!-- http://www.w3id.org/efro/efro#SuccessfulCompletionActivity -->

    <owl:Class rdf:about="http://www.w3id.org/efro/efro#SuccessfulCompletionActivity">
        <rdfs:subClassOf rdf:resource="http://www.w3id.org/efro/efro#CompletionActivity"/>
        <dcterms:description>Activities indicating that a student has fully met all requirements of a program or qualification aim.</dcterms:description>
        <rdfs:label>SuccessfulCompletionActivity</rdfs:label>
        <skos:example>A completed qualification aim logged in the ILR.</skos:example>
    </owl:Class>
    


    <!-- http://www.w3id.org/efro/efro#SuccessfulCompletionStatus -->

    <owl:Class rdf:about="http://www.w3id.org/efro/efro#SuccessfulCompletionStatus">
        <rdfs:subClassOf rdf:resource="http://www.w3id.org/efro/efro#AchievementStatus"/>
        <dcterms:description>Represents the successful fulfillment of all learning aims, including qualification and non-qualification components.</dcterms:description>
        <rdfs:label>SuccessfulCompletionStatus</rdfs:label>
        <skos:example>Achieving an A Level qualification with full attendance and assessments completed successfully.</skos:example>
    </owl:Class>
    


    <!-- http://www.w3id.org/efro/efro#SuccessfulProgression -->

    <owl:Class rdf:about="http://www.w3id.org/efro/efro#SuccessfulProgression">
        <rdfs:subClassOf rdf:resource="http://www.w3id.org/efro/efro#ProgressionStatus"/>
        <dcterms:description>Indicates that the student has successfully progressed to a higher-level qualification, apprenticeship, or employment.</dcterms:description>
        <rdfs:label>SuccessfulProgression</rdfs:label>
        <skos:example>A student completing their study program and enrolling in a Level 3 apprenticeship​.</skos:example>
    </owl:Class>
    


    <!-- http://www.w3id.org/efro/efro#SummerTerm -->

    <owl:Class rdf:about="http://www.w3id.org/efro/efro#SummerTerm">
        <rdfs:subClassOf rdf:resource="http://www.w3id.org/efro/efro#TimePeriod"/>
        <dcterms:description>The term occurring during the summer months, which may include additional or supplemental learning activities.</dcterms:description>
        <rdfs:label>SummerTerm</rdfs:label>
        <skos:example>Summer term activities, such as exam preparation or catch-up sessions, may be included in planned hours.</skos:example>
    </owl:Class>
    


    <!-- http://www.w3id.org/efro/efro#SupportActivity -->

    <owl:Class rdf:about="http://www.w3id.org/efro/efro#SupportActivity">
        <rdfs:subClassOf rdf:resource="http://www.w3id.org/efro/efro#AdministrativeActivity"/>
        <dcterms:description xml:lang="en">Activities designed to provide operational or administrative support for students, staff, and institutional processes.</dcterms:description>
        <rdfs:label>SupportActivity</rdfs:label>
        <skos:example xml:lang="en">Assistance in managing compliance documentation or helping students address attendance-related issues.</skos:example>
    </owl:Class>
    


    <!-- http://www.w3id.org/efro/efro#SustainableEmploymentProgression -->

    <owl:Class rdf:about="http://www.w3id.org/efro/efro#SustainableEmploymentProgression">
        <rdfs:subClassOf rdf:resource="http://www.w3id.org/efro/efro#ProgressionType"/>
        <dcterms:description xml:lang="en">Represents a student&apos;s transition from education to long-term employment.</dcterms:description>
        <rdfs:label>SustainableEmploymentProgression</rdfs:label>
    </owl:Class>
    


    <!-- http://www.w3id.org/efro/efro#SustainableEmploymentStatus -->

    <owl:Class rdf:about="http://www.w3id.org/efro/efro#SustainableEmploymentStatus">
        <rdfs:subClassOf rdf:resource="http://www.w3id.org/efro/efro#AchievementStatus"/>
        <dcterms:description>Indicates that a student has progressed into sustained employment upon completing their study program.</dcterms:description>
        <rdfs:label>SustainableEmploymentStatus</rdfs:label>
        <skos:example>A graduate securing full-time employment after completing a traineeship program​.</skos:example>
    </owl:Class>
    


    <!-- http://www.w3id.org/efro/efro#TeachingStaff -->

    <owl:Class rdf:about="http://www.w3id.org/efro/efro#TeachingStaff">
        <rdfs:subClassOf rdf:resource="http://www.w3id.org/efro/efro#Staff"/>
        <dcterms:description>Staff directly responsible for delivering educational content and supporting students in achieving their learning aims.</dcterms:description>
        <rdfs:label>TeachingStaff</rdfs:label>
        <skos:example>A tutor delivering guided learning sessions for A Level students.</skos:example>
    </owl:Class>
    


    <!-- http://www.w3id.org/efro/efro#TelephoneContact -->

    <owl:Class rdf:about="http://www.w3id.org/efro/efro#TelephoneContact">
        <rdfs:subClassOf rdf:resource="http://www.w3id.org/efro/efro#GeneralAssistanceActivity"/>
        <dcterms:description>Activities involving contacting students or guardians via phone to confirm attendance or address absences.</dcterms:description>
        <rdfs:label>TelephoneContact</rdfs:label>
        <skos:example>Follow-ups for non-attendance compliance.</skos:example>
    </owl:Class>
    


    <!-- http://www.w3id.org/efro/efro#TimeCondition -->

    <owl:Class rdf:about="http://www.w3id.org/efro/efro#TimeCondition">
        <rdfs:subClassOf rdf:resource="http://www.w3id.org/efro/efro#TimeRelated"/>
        <dcterms:description>Defines time-related rules or criteria that must be met to maintain funding compliance or eligibility.</dcterms:description>
        <rdfs:label>TimeCondition</rdfs:label>
    </owl:Class>
    


    <!-- http://www.w3id.org/efro/efro#TimePeriod -->

    <owl:Class rdf:about="http://www.w3id.org/efro/efro#TimePeriod">
        <rdfs:subClassOf rdf:resource="http://www.w3id.org/efro/efro#TimeRelated"/>
        <dcterms:description>Represents a defined duration associated with educational or funding activities, compliance, or tracking.</dcterms:description>
        <rdfs:label>TimePeriod</rdfs:label>
    </owl:Class>
    


    <!-- http://www.w3id.org/efro/efro#TimePoint -->

    <owl:Class rdf:about="http://www.w3id.org/efro/efro#TimePoint">
        <rdfs:subClassOf rdf:resource="http://www.w3id.org/efro/efro#TimeRelated"/>
        <dcterms:description>Represents specific moments or dates within an academic or funding year that are critical for compliance, reporting, or funding calculations.</dcterms:description>
        <rdfs:label>TimePoint</rdfs:label>
    </owl:Class>
    


    <!-- http://www.w3id.org/efro/efro#TimeRelated -->

    <owl:Class rdf:about="http://www.w3id.org/efro/efro#TimeRelated">
        <dcterms:description>Represents concepts related to time in the context of funding compliance, attendance tracking, and program delivery. This includes time-based conditions, periods, and specific points relevant to funding and student progress.</dcterms:description>
        <rdfs:label>TimeRelated</rdfs:label>
    </owl:Class>
    


    <!-- http://www.w3id.org/efro/efro#TimetabledHours -->

    <owl:Class rdf:about="http://www.w3id.org/efro/efro#TimetabledHours">
        <rdfs:subClassOf rdf:resource="http://www.w3id.org/efro/efro#LearningAspect"/>
        <dcterms:description>Hours scheduled for the delivery of learning activities, including both qualification and non-qualification aims.</dcterms:description>
        <rdfs:label>TimetabledHours</rdfs:label>
        <skos:example>Weekly timetables showing planned sessions for students​.</skos:example>
    </owl:Class>
    


    <!-- http://www.w3id.org/efro/efro#TotalHoursForYear -->

    <owl:Class rdf:about="http://www.w3id.org/efro/efro#TotalHoursForYear">
        <rdfs:subClassOf rdf:resource="http://www.w3id.org/efro/efro#LearningAspect"/>
        <dcterms:description>The sum of all planned hours for a student’s study program over an academic year.</dcterms:description>
        <rdfs:label>TotalHoursForYear</rdfs:label>
        <skos:example>540 planned hours for full-time 16-19 study programs.</skos:example>
    </owl:Class>
    


    <!-- http://www.w3id.org/efro/efro#TraditionalProvision -->

    <owl:Class rdf:about="http://www.w3id.org/efro/efro#TraditionalProvision">
        <rdfs:subClassOf rdf:resource="http://www.w3id.org/efro/efro#LearningMode"/>
        <dcterms:description>Learning delivered through traditional in-person teaching methods.</dcterms:description>
        <rdfs:label>TraditionalProvision</rdfs:label>
        <skos:example>Lectures and classroom-based teaching.</skos:example>
    </owl:Class>
    


    <!-- http://www.w3id.org/efro/efro#Trainee -->

    <owl:Class rdf:about="http://www.w3id.org/efro/efro#Trainee">
        <rdfs:subClassOf rdf:resource="http://www.w3id.org/efro/efro#Participant"/>
        <dcterms:description>A participant enrolled in a traineeship program designed to develop employability skills and prepare them for employment or an apprenticeship.</dcterms:description>
        <rdfs:label>Trainee</rdfs:label>
        <skos:example>A young person in a 6-month traineeship program with work placement and training components​.</skos:example>
    </owl:Class>
    


    <!-- http://www.w3id.org/efro/efro#Traineeship -->

    <owl:Class rdf:about="http://www.w3id.org/efro/efro#Traineeship">
        <rdfs:subClassOf rdf:resource="http://www.w3id.org/efro/efro#StudyProgramme"/>
        <dcterms:description>A study program designed to prepare students for employment or further education, combining work placements with skills training.</dcterms:description>
        <rdfs:label>Traineeship</rdfs:label>
        <skos:example>A 6-month traineeship for students aged 16-24 focusing on employability skills​.</skos:example>
    </owl:Class>
    


    <!-- http://www.w3id.org/efro/efro#TraineeshipFunding -->

    <owl:Class rdf:about="http://www.w3id.org/efro/efro#TraineeshipFunding">
        <rdfs:subClassOf rdf:resource="http://www.w3id.org/efro/efro#FundingType"/>
        <dcterms:description>Funding specifically allocated for traineeships, which focus on preparing students for employment or apprenticeships by developing skills and providing work experience.</dcterms:description>
        <rdfs:label>TraineeshipFunding</rdfs:label>
        <skos:example>Traineeship funding based on planned hours and eligible activities​.</skos:example>
    </owl:Class>
    


    <!-- http://www.w3id.org/efro/efro#TrainingProvider -->

    <owl:Class rdf:about="http://www.w3id.org/efro/efro#TrainingProvider">
        <rdfs:subClassOf rdf:resource="http://www.w3id.org/efro/efro#EducationProvider"/>
        <dcterms:description>An organization delivering vocational training, skills development, or workforce preparation programs. Training providers may receive ESFA funding for delivering specific qualifications or employability skills.</dcterms:description>
        <rdfs:label>TrainingProvider</rdfs:label>
        <skos:example>Training providers offering technical qualifications approved on the ESFA list of funded qualifications.</skos:example>
    </owl:Class>
    


    <!-- http://www.w3id.org/efro/efro#TransferActivity -->

    <owl:Class rdf:about="http://www.w3id.org/efro/efro#TransferActivity">
        <rdfs:subClassOf rdf:resource="http://www.w3id.org/efro/efro#EnrollmentActivity"/>
        <dcterms:description>An enrollment activity involving the transfer of a student from one study program or institution to another.</dcterms:description>
        <rdfs:label>TransferActivity</rdfs:label>
        <skos:example>Updating ILR records when a student switches courses​.</skos:example>
    </owl:Class>
    


    <!-- http://www.w3id.org/efro/efro#TransferredStatus -->

    <owl:Class rdf:about="http://www.w3id.org/efro/efro#TransferredStatus">
        <rdfs:subClassOf rdf:resource="http://www.w3id.org/efro/efro#EnrollmentStatus"/>
        <dcterms:description>Indicates that a student has transferred to another study program or institution.</dcterms:description>
        <rdfs:label>TransferredStatus</rdfs:label>
        <skos:example>A student transferring from one provider to another during the program​.</skos:example>
    </owl:Class>
    


    <!-- http://www.w3id.org/efro/efro#TwoWeeksEarlyCompletion -->

    <owl:Class rdf:about="http://www.w3id.org/efro/efro#TwoWeeksEarlyCompletion">
        <rdfs:subClassOf rdf:resource="http://www.w3id.org/efro/efro#TimeCondition"/>
        <dcterms:description>Refers to a program completed two weeks earlier than planned. While less common than six-week adjustments, funding may still need recalibration.</dcterms:description>
        <rdfs:label>TwoWeeksEarlyCompletion</rdfs:label>
        <skos:example>A student achieving their qualification two weeks ahead of the planned completion date​.</skos:example>
    </owl:Class>
    


    <!-- http://www.w3id.org/efro/efro#UpdatePlannedHours -->

    <owl:Class rdf:about="http://www.w3id.org/efro/efro#UpdatePlannedHours">
        <rdfs:subClassOf rdf:resource="http://www.w3id.org/efro/efro#RecordingActivity"/>
        <dcterms:description>An activity involving updates to the recorded planned hours, reflecting changes in the program structure or student participation.</dcterms:description>
        <rdfs:label>UpdatePlannedHours</rdfs:label>
        <skos:example>Updating planned hours after a reduction in a student’s timetable​.</skos:example>
    </owl:Class>
    


    <!-- http://www.w3id.org/efro/efro#VocationalQualification -->

    <owl:Class rdf:about="http://www.w3id.org/efro/efro#VocationalQualification">
        <rdfs:subClassOf rdf:resource="http://www.w3id.org/efro/efro#Qualification"/>
        <dcterms:description>Qualifications focused on practical skills and workplace readiness.</dcterms:description>
        <rdfs:label>VocationalQualification</rdfs:label>
        <skos:example>BTEC or NVQ qualifications included in ESFA funding eligibility​.</skos:example>
    </owl:Class>
    


    <!-- http://www.w3id.org/efro/efro#VocationalTrainingProgression -->

    <owl:Class rdf:about="http://www.w3id.org/efro/efro#VocationalTrainingProgression">
        <rdfs:subClassOf rdf:resource="http://www.w3id.org/efro/efro#ProgressionType"/>
        <dcterms:description xml:lang="en">Covers transitions into alternative training programmes, such as skill-based certifications, employer-sponsored training, or workforce development initiatives.</dcterms:description>
        <rdfs:label>VocationalTrainingProgression</rdfs:label>
    </owl:Class>
    


    <!-- http://www.w3id.org/efro/efro#WholeYear -->

    <owl:Class rdf:about="http://www.w3id.org/efro/efro#WholeYear">
        <rdfs:subClassOf rdf:resource="http://www.w3id.org/efro/efro#TimePeriod"/>
        <dcterms:description>Represents the entire academic or funding year as a single time period.</dcterms:description>
        <rdfs:label>WholeYear</rdfs:label>
        <skos:example>Institutions must report total planned hours and attendance for the whole year in ILR submissions​.</skos:example>
    </owl:Class>
    


    <!-- http://www.w3id.org/efro/efro#WithdrawalActivity -->

    <owl:Class rdf:about="http://www.w3id.org/efro/efro#WithdrawalActivity">
        <rdfs:subClassOf rdf:resource="http://www.w3id.org/efro/efro#Activity"/>
        <dcterms:description>Activities associated with the process of withdrawing a student from a program or institution.</dcterms:description>
        <rdfs:label>WithdrawalActivity</rdfs:label>
    </owl:Class>
    


    <!-- http://www.w3id.org/efro/efro#WithdrawalAdjustment -->

    <owl:Class rdf:about="http://www.w3id.org/efro/efro#WithdrawalAdjustment">
        <rdfs:subClassOf rdf:resource="http://www.w3id.org/efro/efro#FundingAdjustment"/>
        <dcterms:description>An adjustment made when a student withdraws from their program. Funding is recalculated based on the student&apos;s attendance and engagement prior to withdrawal.</dcterms:description>
        <rdfs:label>WithdrawalAdjustment</rdfs:label>
        <skos:example>Partial funding claims made for students who withdraw early, based on the eligible learning complete.</skos:example>
    </owl:Class>
    


    <!-- http://www.w3id.org/efro/efro#WithdrawalDateActivity -->

    <owl:Class rdf:about="http://www.w3id.org/efro/efro#WithdrawalDateActivity">
        <rdfs:subClassOf rdf:resource="http://www.w3id.org/efro/efro#WithdrawalActivity"/>
        <dcterms:description>Recording the specific date of a student’s withdrawal from a program or institution.</dcterms:description>
        <rdfs:label>WithdrawalDateActivity</rdfs:label>
        <skos:example>Used to calculate funding adjustments.</skos:example>
    </owl:Class>
    


    <!-- http://www.w3id.org/efro/efro#WithdrawalFromLearningAim -->

    <owl:Class rdf:about="http://www.w3id.org/efro/efro#WithdrawalFromLearningAim">
        <rdfs:subClassOf rdf:resource="http://www.w3id.org/efro/efro#WithdrawalActivity"/>
        <dcterms:description>An activity where a student withdraws from a specific learning aim or course within a study program.</dcterms:description>
        <rdfs:label>WithdrawalFromLearningAim</rdfs:label>
        <skos:example>A student exits a single course while continuing other studies​.</skos:example>
    </owl:Class>
    


    <!-- http://www.w3id.org/efro/efro#WithdrawalFromStudyProgramme -->

    <owl:Class rdf:about="http://www.w3id.org/efro/efro#WithdrawalFromStudyProgramme">
        <rdfs:subClassOf rdf:resource="http://www.w3id.org/efro/efro#WithdrawalActivity"/>
        <dcterms:description>An activity involving the withdrawal of a student from an entire study program.</dcterms:description>
        <rdfs:label>WithdrawalFromStudyProgramme</rdfs:label>
        <skos:example>Transitioning from a study program to a different one within the same institution​.</skos:example>
    </owl:Class>
    


    <!-- http://www.w3id.org/efro/efro#WithdrawalFromWholeProgramme -->

    <owl:Class rdf:about="http://www.w3id.org/efro/efro#WithdrawalFromWholeProgramme">
        <rdfs:subClassOf rdf:resource="http://www.w3id.org/efro/efro#WithdrawalActivity"/>
        <dcterms:description>An activity marking the withdrawal of a student from all programs and courses at the institution.</dcterms:description>
        <rdfs:label>WithdrawalFromWholeProgramme</rdfs:label>
        <skos:example>A complete exit from education recorded in the ILR​.</skos:example>
    </owl:Class>
    


    <!-- http://www.w3id.org/efro/efro#WithdrawalProcess -->

    <owl:Class rdf:about="http://www.w3id.org/efro/efro#WithdrawalProcess">
        <rdfs:subClassOf rdf:resource="http://www.w3id.org/efro/efro#WithdrawalActivity"/>
        <dcterms:description>The administrative and procedural activities involved in managing and recording a student&apos;s withdrawal.</dcterms:description>
        <rdfs:label>WithdrawalProcess</rdfs:label>
        <skos:example>Completing and submitting withdrawal forms as evidence for audits.</skos:example>
    </owl:Class>
    


    <!-- http://www.w3id.org/efro/efro#WithdrawalReason -->

    <owl:Class rdf:about="http://www.w3id.org/efro/efro#WithdrawalReason">
        <owl:equivalentClass>
            <owl:Class>
                <owl:unionOf rdf:parseType="Collection">
                    <rdf:Description rdf:about="http://www.w3id.org/efro/efro#NonAttendanceReason"/>
                    <rdf:Description rdf:about="http://www.w3id.org/efro/efro#PersonalReason"/>
                    <rdf:Description rdf:about="http://www.w3id.org/efro/efro#ProgressionReason"/>
                </owl:unionOf>
            </owl:Class>
        </owl:equivalentClass>
        <rdfs:subClassOf rdf:resource="http://www.w3id.org/efro/efro#Reason"/>
        <dcterms:description>A specific reason provided for a student withdrawing from a study program or qualification.</dcterms:description>
        <rdfs:label>WithdrawalReason</rdfs:label>
        <skos:example>Withdrawal due to employment opportunities, health issues, or transferring to another institution.</skos:example>
    </owl:Class>
    


    <!-- http://www.w3id.org/efro/efro#WithdrawalRecord -->

    <owl:Class rdf:about="http://www.w3id.org/efro/efro#WithdrawalRecord">
        <rdfs:subClassOf rdf:resource="http://www.w3id.org/efro/efro#RecordDocument"/>
        <dcterms:description>A document recording the details of a student&apos;s withdrawal from a study program, including the date, reason, and evidence of proper process adherence.</dcterms:description>
        <rdfs:label>WithdrawalRecord</rdfs:label>
        <skos:example>Withdrawal forms or records submitted as part of the ILR or school census data returns.</skos:example>
    </owl:Class>
    


    <!-- http://www.w3id.org/efro/efro#WithdrawnQualification -->

    <owl:Class rdf:about="http://www.w3id.org/efro/efro#WithdrawnQualification">
        <rdfs:subClassOf rdf:resource="http://www.w3id.org/efro/efro#LearningAim"/>
        <dcterms:description>A learning aim or qualification that a student has formally withdrawn from before completion.</dcterms:description>
        <rdfs:label>WithdrawnQualification</rdfs:label>
        <skos:example>Withdrawal due to personal reasons or a change in the study program, with funding adjustments made accordingly​.</skos:example>
    </owl:Class>
    


    <!-- http://www.w3id.org/efro/efro#WithdrawnStatus -->

    <owl:Class rdf:about="http://www.w3id.org/efro/efro#WithdrawnStatus">
        <rdfs:subClassOf rdf:resource="http://www.w3id.org/efro/efro#EnrollmentStatus"/>
        <dcterms:description>Status indicating that a student has formally withdrawn from their study program.</dcterms:description>
        <rdfs:label>WithdrawnStatus</rdfs:label>
        <skos:example>A withdrawn student is subject to funding adjustments based on their attendance before withdrawal​.</skos:example>
    </owl:Class>
    


    <!-- http://www.w3id.org/efro/efro#WithdrawnStudent -->

    <owl:Class rdf:about="http://www.w3id.org/efro/efro#WithdrawnStudent">
        <owl:equivalentClass>
            <owl:Class>
                <owl:intersectionOf rdf:parseType="Collection">
                    <rdf:Description rdf:about="http://www.w3id.org/efro/efro#Student"/>
                    <owl:Restriction>
                        <owl:onProperty rdf:resource="http://www.w3id.org/efro/efro#hasStatus"/>
                        <owl:someValuesFrom rdf:resource="http://www.w3id.org/efro/efro#WithdrawnStatus"/>
                    </owl:Restriction>
                </owl:intersectionOf>
            </owl:Class>
        </owl:equivalentClass>
        <rdfs:subClassOf rdf:resource="http://www.w3id.org/efro/efro#Student"/>
        <dcterms:description>A student who has withdrawn from their study program before completion, requiring adjustments to the institution’s funding claims.</dcterms:description>
        <rdfs:label>WithdrawnStudent</rdfs:label>
        <skos:example>A student who leaves their program after completing 6 weeks but before achieving their qualification​</skos:example>
    </owl:Class>
    


    <!-- http://www.w3id.org/efro/efro#YoungPerson -->

    <owl:Class rdf:about="http://www.w3id.org/efro/efro#YoungPerson">
        <rdfs:subClassOf rdf:resource="http://www.w3id.org/efro/efro#Participant"/>
        <dcterms:description>A participant aged 16-19 (or up to 24 with an Education, Health, and Care Plan) engaged in a study program or traineeship.</dcterms:description>
        <rdfs:label>YoungPerson</rdfs:label>
        <skos:example>A young person undertaking a T Level program.</skos:example>
    </owl:Class>
    


    <!-- 
    ///////////////////////////////////////////////////////////////////////////////////////
    //
    // General axioms
    //
    ///////////////////////////////////////////////////////////////////////////////////////
     -->

    <rdf:Description>
        <rdf:type rdf:resource="http://www.w3.org/2002/07/owl#AllDisjointClasses"/>
        <owl:members rdf:parseType="Collection">
            <rdf:Description rdf:about="http://www.w3id.org/efro/efro#ActualAttendanceActivity"/>
            <rdf:Description rdf:about="http://www.w3id.org/efro/efro#LastAttendanceActivity"/>
            <rdf:Description rdf:about="http://www.w3id.org/efro/efro#NonAttendanceActivity"/>
            <rdf:Description rdf:about="http://www.w3id.org/efro/efro#QualifyingAttendanceActivity"/>
            <rdf:Description rdf:about="http://www.w3id.org/efro/efro#StudentAttendance"/>
            <rdf:Description rdf:about="http://www.w3id.org/efro/efro#TelephoneContact"/>
        </owl:members>
    </rdf:Description>
</rdf:RDF>



<!-- Generated by the OWL API (version 4.5.29.2024-05-13T12:11:03Z) https://github.com/owlcs/owlapi -->

